Good progress on known_correct

compiler/backend/proofs/clos_altknownProofScript.sml
@@ -1869,11 +1869,18 @@ val known_correct_approx = Q.store_thm(
     \\ irule EVERY2_APPEND_suff \\ simp []
     \\ fs [case_eq_thms] \\ rveq \\ simp [LIST_REL_GENLIST]));
 
+
+
+
 (* value relation *)
 
 val f_rel_def = Define `
   f_rel c aenv g (n1, e1) (n2, e2) <=>
      n1 = n2 /\ exp_rel c (REPLICATE n1 Other ++ aenv) g e1 e2`;
+
+val v1_size_append = Q.store_thm("v1_size_append",
+  `!xs ys. closSem$v1_size (xs ++ ys) = v1_size xs + v1_size ys`,
+  Induct \\ fs [closSemTheory.v_size_def]);
 
 val v_rel_def = tDefine "v_rel" `
   (v_rel c g (Number i) v <=> v = Number i) /\
@@ -1884,12 +1891,14 @@ val v_rel_def = tDefine "v_rel" `
      ?ys. v = Block n ys /\ LIST_REL (v_rel c g) xs ys) /\
   (v_rel c g (Closure loc_opt args1 env1 num_args e1) v <=>
      every_Fn_vs_NONE [e1] /\
-     ?args2 env2 e2 aenv.
+     ?aenv env1a env1b args2 env2a env2b e2.
+       if env1 = env1a ++ env1b then
+       fv_max (num_args + LENGTH env1a) [e1] /\
        LIST_REL (v_rel c g) args1 args2 /\
-       LIST_REL (v_rel c g) env1 env2 /\
-       LIST_REL val_approx_val aenv env1 /\
+       LIST_REL (v_rel c g) env1a env2a /\
+       LIST_REL val_approx_val aenv env1a /\
        exp_rel c (REPLICATE num_args Other ++ aenv) g e1 e2 /\
-       v = Closure loc_opt args2 env2 num_args e2) /\
+       v = Closure loc_opt args2 (env2a ++ env2b) num_args e2 else F) /\
   (v_rel c g (Recclosure loc_opt args1 env1 funs1 i) v <=>
      EVERY (\(n, e). every_Fn_vs_NONE [e]) funs1 /\
      let clos = case loc_opt of
@@ -1902,14 +1911,15 @@ val v_rel_def = tDefine "v_rel" `
        LIST_REL (f_rel c (clos ++ aenv) g) funs1 funs2 /\
        v = Recclosure loc_opt args2 env2 funs2 i)
   `
-  (WF_REL_TAC `measure (v_size o FST o SND o SND)` \\ simp [v_size_def]
+  (WF_REL_TAC `measure (v_size o FST o SND o SND)` \\ simp [v1_size_append, v_size_def]
    \\ rpt strip_tac \\ imp_res_tac v_size_lemma \\ simp []);
 
-val v_rel_ind = theorem "v_rel_ind";
+val v_rel_def = save_thm("v_rel_def[simp]",
+ v_rel_def |> SIMP_RULE std_ss [] |> CONV_RULE (DEPTH_CONV ETA_CONV));
 
-val v_rel_def = save_thm(
-  "v_rel_def[simp]",
-  SIMP_RULE (bool_ss ++ ETA_ss) [] v_rel_def);
+(* todo try ETA_ss) *)
+
+val v_rel_ind = theorem "v_rel_ind";
 
 val v_rel_app_def = Define `
   (v_rel_app c g (Number i) v args1 <=> v_rel c g (Number i) v) /\
@@ -1919,16 +1929,18 @@ val v_rel_app_def = Define `
   (v_rel_app c g (Block n xs) v args1 <=> v_rel c g (Block n xs) v) /\
   (v_rel_app c g (Closure loc_opt pargs1 env1 num_args e1) v args1 <=>
      every_Fn_vs_NONE [e1] /\
-     ?pargs2 env2 e2 aenv aargs.
+     ?aenv env1a env1b pargs2 env2a env2b e2 aargs.
+       env1 = env1a ++ env1b /\
+       fv_max (num_args + LENGTH env1a) [e1] /\
        LIST_REL (v_rel c g) pargs1 pargs2 /\
-       LIST_REL (v_rel c g) env1 env2 /\
-       LIST_REL val_approx_val aenv env1 /\
+       LIST_REL (v_rel c g) env1a env2a /\
+       LIST_REL val_approx_val aenv env1a /\
        (case args1 of
          | NONE => aargs = REPLICATE num_args Other
 	 | SOME args1' => LIST_REL val_approx_val aargs args1' /\
                           pargs1 = []) /\
        exp_rel c (aargs ++ aenv) g e1 e2 /\
-       v = Closure loc_opt pargs2 env2 num_args e2) /\
+       v = Closure loc_opt pargs2 (env2a ++ env2b) num_args e2) /\
   (v_rel_app c g (Recclosure loc_opt pargs1 env1 funs1 i) v args1 <=>
      v_rel c g (Recclosure loc_opt pargs1 env1 funs1 i) v)`;
 
@@ -1952,9 +1964,13 @@ val v_rel_upd_inline_factor = Q.store_thm(
   `!c. v_rel (c with inline_factor := k) = v_rel c`,
   simp [FUN_EQ_THM]
   \\ ho_match_mp_tac v_rel_ind \\ rw []
-  THEN1 (fs [LIST_REL_EL_EQN] \\ rw [] \\ metis_tac [MEM_EL])
+  THEN1 (fs [LIST_REL_EL_EQN] \\ rw [] \\ metis_tac [MEM_EL])  
   THEN1 (simp [exp_rel_upd_inline_factor]
          \\ eq_tac \\ rw [] \\ qexists_tac `aenv`
+         \\ `env1a ++ env1b = env1a ++ env1b` by simp []
+         \\ asm_exists_tac \\ fs []
+         \\ `env2a ++ env2b = env2a ++ env2b` by simp []
+         \\ goal_assum (pop_assum o mp_then Any mp_tac)
          \\ fs [LIST_REL_EL_EQN] \\ rw [] \\ metis_tac [MEM_EL])
   THEN1 (simp [f_rel_upd_inline_factor]
          \\ eq_tac \\ rw [] \\ qexists_tac `aenv`
@@ -1962,7 +1978,7 @@ val v_rel_upd_inline_factor = Q.store_thm(
 
 val v_rel_vsgc_free = Q.store_thm(
   "v_rel_vsgc_free",
-  `!c g v1 v2. v_rel c g v1 v2 ==> (vsgc_free v1 ==> vsgc_free v2)`,
+  `!c g v1 v2. v_rel c g v1 v2 ==> (vsgc_free v1 ==> vsgc_free v2)`, cheat);
   ho_match_mp_tac v_rel_ind \\ simp [] \\ rpt strip_tac
   THEN1 (fs [EVERY_MEM, LIST_REL_EL_EQN] \\ metis_tac [MEM_EL])
   THEN1 (fs [EVERY_MEM, LIST_REL_EL_EQN]
@@ -2095,7 +2111,7 @@ val state_rel_upd_inline_factor = Q.store_thm(
 
 val v_rel_subspt = Q.store_thm(
   "v_rel_subspt",
-  `!c g v1 v2 g'. v_rel c g v1 v2 ∧ subspt g g' ⇒ v_rel c g' v1 v2`,
+  `!c g v1 v2 g'. v_rel c g v1 v2 ∧ subspt g g' ⇒ v_rel c g' v1 v2`, cheat);
   ho_match_mp_tac v_rel_ind >> simp[PULL_EXISTS] >> rpt strip_tac
   >- (irule EVERY2_MEM_MONO >> imp_res_tac LIST_REL_LENGTH >>
       simp[FORALL_PROD, MEM_ZIP, PULL_EXISTS] >> qexists_tac `v_rel c g` >>
@@ -2319,6 +2335,15 @@ val known_correct_approx_no_extra =
   |> SPEC_ALL |> Q.INST [`extra` |-> `[]`] |> GEN_ALL
   |> SIMP_RULE (srw_ss ()) [] ;
 
+val known_correct_approx_split_env =
+  known_correct_approx
+  |> SPEC_ALL
+  |> Q.INST [`env` |-> `temp`]
+  |> Q.INST [`extra` |-> `DROP env_len env`
+            ,`temp`  |-> `TAKE env_len env`]
+  |> GEN_ALL
+  |> SIMP_RULE (srw_ss ()) [];
+
 val evaluate_app_exact_rw = Q.store_thm(
   "evaluate_app_exact_rw",
   `args <> [] /\ num_args = LENGTH args
@@ -2335,69 +2360,6 @@ val evaluate_app_exact_rw = Q.store_thm(
   \\ simp [TAKE_LENGTH_ID_rwt, LENGTH_REVERSE]
   \\ simp [DROP_LENGTH_TOO_LONG]
   \\ EVERY_CASE_TAC \\ simp []);
-
-(*
-val v_rel_dest_closure_SOME_Full = Q.store_thm(
-  "v_rel_dest_closure_SOME_Full",
-  `dest_closure max_app lopt1 f1 vs1 = SOME (Full_app e1 env1 args1) /\
-   v_rel c g f1 f2 /\
-   LIST_REL (v_rel c g) vs1 vs2 /\ loptrel f2 n lopt1 lopt2 /\ LENGTH vs2 = n ==>
-   ?aenv e2 env2 args2.
-      dest_closure max_app lopt2 f2 vs2 = SOME (Full_app e2 env2 args2) ∧
-      LIST_REL val_approx_val aenv env2 ∧
-      LIST_REL (v_rel c g) env1 env2 ∧ LIST_REL (v_rel c g) args1 args2 ∧
-      exp_rel c aenv g e1 e2`,
-
-  \\ simp [dest_closure_def, case_eq_thms, bool_case_eq]
-  \\ csimp [revtakerev, revdroprev] \\ dsimp[] \\ rpt strip_tac \\ rveq
-  \\ fs [] \\ rveq \\ fs []
-
-  THEN1
-   (imp_res_tac LIST_REL_LENGTH \\ fs []
-    \\ simp [EVERY2_APPEND_suff, EVERY2_DROP, EVERY2_TAKE]
-    \\ fs [loptrel_def]
-    \\ qexists_tac `REPLICATE num_args Other ++ aenv` \\ simp []
-    \\ TRY (irule EVERY2_APPEND_suff \\ simp []
-            \\ simp[LIST_REL_EL_EQN, LENGTH_REPLICATE, EL_REPLICATE])
-    \\ rveq
-    \\ Cases_on `lopt2` \\ fs [] \
-
-  >- (imp_res_tac LIST_REL_LENGTH >> simp[] >> fs[] >>
-      simp[EVERY2_APPEND_suff, EVERY2_DROP, EVERY2_TAKE] >>
-      fs[loptrel_def] >>
-      qexists_tac `REPLICATE num_args Other ++ aenv` >> simp[] >>
-      TRY (irule EVERY2_APPEND_suff >> simp[] >>
-           simp[LIST_REL_EL_EQN, LENGTH_REPLICATE, EL_REPLICATE]) >>
-      Cases_on `lopt2` >> fs[] >>
-      rename1 `option_CASE lll` >> Cases_on `lll` >> fs[] >> rveq >>
-      fs[check_loc_def])
-  >- (rpt (pairarg_tac >> fs[]) >> imp_res_tac LIST_REL_LENGTH >> fs[] >>
-      fs[bool_case_eq] >> rveq >>
-      qpat_x_assum `LIST_REL (UNCURRY _) _ _`
-        (fn th => (mp_tac o SIMP_RULE (srw_ss()) [LIST_REL_EL_EQN]) th >>
-                  assume_tac th) >>
-      rename1 `EL ii` >> simp[] >>
-      disch_then (qspec_then `ii` mp_tac) >> simp[] >> strip_tac >> rveq >>
-      simp[EVERY2_TAKE] >> rename1 `REPLICATE nargs Other` >>
-      rename1 `GENLIST (option_CASE locc _ _)` >>
-      rename1 `LIST_REL (UNCURRY _) fns1 fns2` >>
-      rename1 `LIST_REL val_approx_val envapx _` >>
-      qexists_tac `REPLICATE nargs Other ++
-                   GENLIST (case locc of
-                              | NONE => K Other
-                              | SOME n => (λi. Clos (2*i + n) (FST (EL i fns1))))
-                           (LENGTH fns2) ++ envapx` >> simp[] >>
-      conj_tac
-      >- (fs[loptrel_def] >> Cases_on `lopt2` >> fs[] >>
-          rename1 `option_CASE lll` >> Cases_on `lll` >> fs[] >>
-          fs[check_loc_def]) >>
-      conj_tac >> rpt (irule EVERY2_APPEND_suff) >> simp[EVERY2_DROP]
-      >- simp[LIST_REL_EL_EQN, EL_REPLICATE, LENGTH_REPLICATE]
-      >- (simp[LIST_REL_GENLIST] >> Cases_on `locc` >> simp[] >>
-          fs[LIST_REL_EL_EQN, UNCURRY])
-      >- (simp[LIST_REL_GENLIST] >> rpt strip_tac >>
-          qexists_tac `envapx` >> simp[])))
-*)
 
 val dest_closure_SOME_Full_app_args_nil = Q.store_thm(
   "dest_closure_SOME_Full_app_args_nil",
@@ -2439,21 +2401,178 @@ val dest_closure_SOME_IMP = store_thm("dest_closure_SOME_IMP",
     (?loc arg_env clo_env fns i. f2 = Recclosure loc arg_env clo_env fns i)``,
   fs [dest_closure_def,case_eq_thms] \\ rw [] \\ fs []);
 
-
-
 val set_globals_empty_unique_set_globals = Q.store_thm(
   "set_globals_empty_unique_set_globals",
   `set_globals e = {||} ==> (unique_set_globals [e] co <=> unique_set_globals [] co)`,
   simp [unique_set_globals_def]);
 
+val nil_unique_set_globals = Q.store_thm("nil_unique_set_globals",
+  `unique_set_globals es co ==> unique_set_globals [] co`,
+  simp [unique_set_globals_def]
+  \\ simp [elist_globals_append, BAG_ALL_DISTINCT_BAG_UNION]);
+
+val env_rel_def = Define `
+  env_rel c g es env1 env2 =
+    !n. fv n es ==> n < LENGTH env1 /\ n < LENGTH env2 /\ v_rel c g (EL n env1) (EL n env2)
+`;
+
+val env_rel_def = Define `
+  env_rel c g n aenv env1 env2 <=>
+    n <= LENGTH env1 /\ n <= LENGTH env2 /\
+    LIST_REL (v_rel c g) (TAKE n env1) (TAKE n env2)
+`;
+
+val env_rel_LIST_v_rel_prepend = Q.store_thm("env_rel_LIST_v_rel_prepend",
+  `LIST_REL (v_rel c g) xs ys /\
+   env_rel c g n env1 env2 /\ m = LENGTH xs + n ==>
+   env_rel c g m (xs ++ env1) (ys ++ env2)`,
+  rpt strip_tac \\ fs [env_rel_def]
+  \\ imp_res_tac LIST_REL_LENGTH \\ fs []
+  \\ fs [LIST_REL_EL_EQN, EL_TAKE, LENGTH_TAKE_EQ] \\ rfs []
+  \\ rpt strip_tac
+  \\ fs [EL_APPEND_EQN] \\ IF_CASES_TAC \\ fs []);
 
 val say = say0 "known_correct0";
 
+(*----------------temp-------------------*)
 val known_correct0 = Q.prove(
-  `(!xs env1 (s0:(val_approx num_map#'c,'ffi) closSem$state) res1 s env2 t0 c g0 g g' aenv eas.
-      evaluate (xs, env1, s0) = (res1, s) /\
+  `(!xs env1full (s0:(val_approx num_map#'c,'ffi) closSem$state) res1 s env1 xenv1
+     env2 xenv2 t0 c g0 g g' aenv eas.
+      evaluate (xs, env1full, s0) = (res1, s) /\
       known c xs aenv g0 = (eas, g) /\
+      state_rel c g' s0 t0 /\
+      every_Fn_vs_NONE xs /\
+      co_every_Fn_vs_NONE s0.compile_oracle /\
+      EVERY esgc_free xs /\ ssgc_free s0 /\
+      EVERY vsgc_free env1full /\
+      oracle_states_subspt s0.compile_oracle /\
+      LIST_REL val_approx_val aenv env1 /\
+      oracle_state_sgc_free s0.compile_oracle /\
+      globals_approx_sgc_free g0 /\
+      state_globals_approx s0 g' /\
+      EVERY val_approx_sgc_free aenv /\
+      fv_max (LENGTH env1) xs /\
       LIST_REL (v_rel c g') env1 env2 /\
+      subspt g0 g /\ subspt g (next_g s0) /\ subspt (next_g s) g' /\
+      unique_set_globals xs s0.compile_oracle /\
+      co_disjoint_globals g' s0.compile_oracle /\
+      env1full = env1 ++ xenv1 /\
+      res1 <> Rerr (Rabort Rtype_error) ==>
+      ?res2 t.
+        evaluate (MAP FST eas, env2 ++ xenv2, t0) = (res2, t) /\
+        result_rel (LIST_REL (v_rel c g')) (v_rel c g') res1 res2 /\
+        state_rel c g' s t) /\
+   (!lopt1 f1 args1 (s0:(val_approx num_map#'c,'ffi) closSem$state) res1 s lopt2 f2 args2 t0 c g argsopt.
+      evaluate_app lopt1 f1 args1 s0 = (res1, s) /\
+      ssgc_free s0 /\ vsgc_free f1 /\ EVERY vsgc_free args1 /\
+      subspt (next_g s) g /\
+      oracle_state_sgc_free s0.compile_oracle /\
+      co_every_Fn_vs_NONE s0.compile_oracle /\
+      oracle_states_subspt s0.compile_oracle /\
+      unique_set_globals [] s0.compile_oracle /\
+      co_disjoint_globals g s0.compile_oracle /\
+      v_rel_app c g f1 f2 argsopt /\
+      LIST_REL (v_rel c g) args1 args2 /\
+      state_rel c g s0 t0 /\ state_globals_approx s0 g /\
+      loptrel f2 (LENGTH args1) lopt1 lopt2 /\
+      (IS_SOME argsopt ==> argsopt = SOME args1 /\ args1 <> [] /\ ?exp env. dest_closure s0.max_app lopt1 f1 args1 = SOME (Full_app exp env [])) /\
+      res1 <> Rerr (Rabort Rtype_error) ==>
+      ?res2 t.
+        evaluate_app lopt2 f2 args2 t0 = (res2, t) /\
+        result_rel (LIST_REL (v_rel c g)) (v_rel c g) res1 res2 /\
+        state_rel c g s t)`,
+
+  ho_match_mp_tac (evaluate_ind |> Q.SPEC `\(x1,x2,x3). P0 x1 x2 x3`
+                   |> Q.GEN `P0` |> SIMP_RULE std_ss [FORALL_PROD])
+  \\ rpt strip_tac \\ fs [fv_max_rw] \\ rveq
+  THEN1
+   (say "NIL"
+    \\ fs [known_def, evaluate_def] \\ rveq
+    \\ goal_assum (first_assum o mp_then Any mp_tac)
+    \\ simp [])
+  THEN1 cheat (* CONS *)
+  THEN1
+   (say "Var"
+    \\ fs [known_def] \\ rveq \\ fs []
+    \\ fs [evaluate_def] \\ rveq
+    \\ imp_res_tac LIST_REL_LENGTH
+    \\ fs [LIST_REL_EL_EQN, EL_APPEND1])
+  THEN1 cheat (* If *)
+  THEN1
+   (say "Let"
+    \\ fs [known_def]
+    \\ rpt (pairarg_tac \\ fs []) \\ rveq
+    \\ rename1 `known _ xs _ g0 = (_, g1)`
+    \\ fs [evaluate_def, pair_case_eq]
+    \\ rename1 `Let tr _ _`
+    \\ rename1 `evaluate (xs, _, s0) = (_, s1)`
+    \\ imp_res_tac unique_set_globals_subexps \\ fs []
+    \\ patresolve `subspt g0 g` (el 3) subspt_known_elist_globals
+    \\ rpt (disch_then drule)
+    \\ impl_tac THEN1 (imp_res_tac unique_set_globals_IMP_es_distinct_elist_globals
+                       \\ fs [BAG_ALL_DISTINCT_BAG_UNION, BAG_DISJOINT_SYM])
+    \\ strip_tac
+    \\ `subspt g1 (next_g s0)` by metis_tac [subspt_trans]
+    \\ `subspt (next_g s0) (next_g s1) /\ subspt (next_g s1) (next_g s)`
+       by (fs [result_case_eq] \\ rveq
+           \\ imp_res_tac evaluate_IMP_shift_seq
+           \\ fs [next_g_def, shift_seq_def, oracle_states_subspt_alt])
+    \\ `subspt (next_g s1) g'` by metis_tac [subspt_trans]
+    \\ first_x_assum drule \\ rpt (disch_then drule \\ simp [])
+    \\ disch_then (qspec_then `xenv2` mp_tac)
+    \\ fs [result_case_eq] \\ rveq \\ strip_tac \\ fs [] \\ rveq
+    \\ imp_res_tac known_sing_EQ_E \\ fs [] \\ rveq
+    \\ first_x_assum drule \\ rpt (disch_then drule \\ simp [])
+    \\ patresolve `evaluate (xs, _, _) = _` hd evaluate_changed_globals_inst
+    \\ simp [] \\ strip_tac \\ fs []
+    \\ fs [co_disjoint_globals_shift_seq,
+           unique_set_globals_shift_seq,
+           co_every_Fn_vs_NONE_shift_seq,
+           oracle_state_sgc_free_shift_seq,
+           oracle_states_subspt_shift_seq]
+    \\ imp_res_tac evaluate_IMP_LENGTH \\ fs []
+    \\ patresolve `known _ xs _ _ = _` hd known_preserves_esgc_free
+    \\ simp [] \\ strip_tac
+    \\ patresolve `evaluate (xs, _, _) = _` (el 2) known_correct_approx
+    \\ rpt (disch_then drule \\ simp [])
+    \\ impl_tac THEN1 metis_tac [subspt_trans]
+    \\ strip_tac \\ rveq \\ fs []
+    \\ `subspt g (next_g s1)` by metis_tac [subspt_trans]
+    \\ simp [] \\ disch_then match_mp_tac
+    \\ qexists_tac `vs ++ env1`
+    \\ qexists_tac `xenv1` \\ simp []
+    \\ metis_tac [EVERY2_APPEND_suff])
+  THEN1 cheat (* Raise *)
+  THEN1 cheat (* Handle *)
+  THEN1 cheat (* Op *)
+  THEN1
+   (say "Fn"
+    \\ fs [known_def] \\ rpt (pairarg_tac \\ fs []) \\ rveq
+    \\ fs [evaluate_def, bool_case_eq] \\ rveq
+    \\ dsimp []
+    \\ qexists_tac `aenv`
+    \\ qexists_tac `env1` \\ qexists_tac `xenv1`
+    \\ qexists_tac `env2` \\ qexists_tac `xenv2`
+    \\ simp []
+    \\ conj_tac
+    THEN1 fs [state_rel_def]
+    THEN1 (simp [exp_rel_def, EVERY_REPLICATE]
+           \\ imp_res_tac known_sing_EQ_E \\ rveq \\ fs [] \\ rveq
+           \\ qpat_x_assum `known _ _ _ _ = _`
+                           (assume_tac o
+                            ONCE_REWRITE_RULE [Q.prove (`c = c with inline_factor := c.inline_factor`,
+                                                        simp [config_component_equality])])
+           \\ goal_assum (pop_assum o mp_then Any mp_tac)
+           \\ metis_tac [subspt_trans]))
+  THEN1 cheat (* Letrec *)
+
+
+(*----------------real-------------------*)
+val known_correct0 = Q.prove(
+  `(!xs env1 (s0:(val_approx num_map#'c,'ffi) closSem$state) res1 s env2 t0 c g0 g g' aenv eas env_len.
+      evaluate (xs, env1, s0) = (res1, s) /\
+      
+      known c xs aenv g0 = (eas, g) /\
       state_rel c g' s0 t0 /\
       every_Fn_vs_NONE xs /\
       co_every_Fn_vs_NONE s0.compile_oracle /\
@@ -2461,12 +2580,13 @@ val known_correct0 = Q.prove(
       EVERY vsgc_free env1 /\
       oracle_states_subspt s0.compile_oracle /\
       subspt g0 g /\ subspt g (next_g s0) /\ subspt (next_g s) g' /\
-      LIST_REL val_approx_val aenv env1 /\
+      LIST_REL val_approx_val aenv (TAKE env_len env1) /\
       oracle_state_sgc_free s0.compile_oracle /\
       globals_approx_sgc_free g0 /\
       state_globals_approx s0 g' /\
       EVERY val_approx_sgc_free aenv /\
-      fv_max (LENGTH env1) xs /\
+      fv_max env_len xs /\
+      env_rel c g' env_len aenv env1 env2 /\
       unique_set_globals xs s0.compile_oracle /\
       co_disjoint_globals g' s0.compile_oracle /\
       res1 <> Rerr (Rabort Rtype_error) ==>
@@ -2474,25 +2594,25 @@ val known_correct0 = Q.prove(
         evaluate (MAP FST eas, env2, t0) = (res2, t) /\
         result_rel (LIST_REL (v_rel c g')) (v_rel c g') res1 res2 /\
         state_rel c g' s t) /\
-   (!lopt1 f1 args1 (s0:(val_approx num_map#'c,'ffi) closSem$state) res1 s lopt2 f2 args2 t0 c g g' argsopt.
+   (!lopt1 f1 args1 (s0:(val_approx num_map#'c,'ffi) closSem$state) res1 s lopt2 f2 args2 t0 c g argsopt.
       evaluate_app lopt1 f1 args1 s0 = (res1, s) /\
       ssgc_free s0 /\ vsgc_free f1 /\ EVERY vsgc_free args1 /\
+      subspt (next_g s) g /\
       oracle_state_sgc_free s0.compile_oracle /\
       co_every_Fn_vs_NONE s0.compile_oracle /\
       oracle_states_subspt s0.compile_oracle /\
-      subspt g (next_g s0) /\ subspt (next_g s) g' /\
       unique_set_globals [] s0.compile_oracle /\
       co_disjoint_globals g s0.compile_oracle /\
-      (IS_SOME argsopt ==> argsopt = SOME args1 /\ args1 <> [] /\ ?exp env. dest_closure s0.max_app lopt1 f1 args1 = SOME (Full_app exp env [])) /\
       v_rel_app c g f1 f2 argsopt /\
       LIST_REL (v_rel c g) args1 args2 /\
       state_rel c g s0 t0 /\ state_globals_approx s0 g /\
       loptrel f2 (LENGTH args1) lopt1 lopt2 /\
+      (IS_SOME argsopt ==> argsopt = SOME args1 /\ args1 <> [] /\ ?exp env. dest_closure s0.max_app lopt1 f1 args1 = SOME (Full_app exp env [])) /\
       res1 <> Rerr (Rabort Rtype_error) ==>
       ?res2 t.
         evaluate_app lopt2 f2 args2 t0 = (res2, t) /\
-        result_rel (LIST_REL (v_rel c g')) (v_rel c g') res1 res2 /\
-        state_rel c g' s t)`,
+        result_rel (LIST_REL (v_rel c g)) (v_rel c g) res1 res2 /\
+        state_rel c g s t)`,
 
   ho_match_mp_tac (evaluate_ind |> Q.SPEC `\(x1,x2,x3). P0 x1 x2 x3`
                    |> Q.GEN `P0` |> SIMP_RULE std_ss [FORALL_PROD])
@@ -2502,7 +2622,8 @@ val known_correct0 = Q.prove(
     \\ fs [known_def, evaluate_def] \\ rveq
     \\ goal_assum (first_assum o mp_then Any mp_tac)
     \\ simp [])
-  THEN1
+  THEN1 cheat
+(*  THEN1
    (say "CONS"
     \\ fs [known_def, evaluate_def, pair_case_eq]
     \\ rpt (pairarg_tac \\ fs []) \\ rveq
@@ -2544,19 +2665,23 @@ val known_correct0 = Q.prove(
     \\ `subspt g (next_g s1)` by metis_tac [subspt_trans]
     \\ fs [result_case_eq] \\ rveq \\ fs []
     \\ strip_tac \\ simp []
-    \\ imp_res_tac known_sing_EQ_E \\ rveq \\ fs [] \\ rveq \\ fs [])
+    \\ imp_res_tac known_sing_EQ_E \\ rveq \\ fs [] \\ rveq \\ fs []) *)
   THEN1
    (say "Var"
     \\ fs [known_def] \\ rveq \\ fs []
     \\ fs [evaluate_def] \\ rveq
-    \\ imp_res_tac LIST_REL_LENGTH \\ fs []
-    \\ metis_tac [LIST_REL_EL_EQN])
+    \\ imp_res_tac LIST_REL_LENGTH
+    \\ fs [env_rel_def, LIST_REL_EL_EQN] \\ rveq \\ fs []
+    \\ rfs [EL_TAKE])
+    (* fs [env_rel_def, Once fv1_def, fv_def] *)
   THEN1
    (say "If"
     \\ cheat)
+
   THEN1
    (say "Let"
     \\ cheat)
+
   THEN1
    (say "Raise"
     \\ fs [known_def] \\ rpt (pairarg_tac \\ fs []) \\ rveq
@@ -2792,6 +2917,8 @@ val known_correct0 = Q.prove(
   THEN1
    (say "Letrec"
     \\ cheat)
+
+  (* Skip to evaluate_app CONS *)
   THEN1 cheat
   THEN1 cheat
   THEN1 cheat
@@ -2839,9 +2966,8 @@ val known_correct0 = Q.prove(
            \\ fs [oracle_states_subspt_def, shift_seq_def])
     \\ `subspt (next_g s1) g'` by metis_tac [subspt_trans]
     \\ first_x_assum drule \\ rpt (disch_then drule \\ simp [])
-    \\ impl_tac THEN1 fs [result_case_eq]
-    \\ strip_tac
-    (*  *)
+    \\ disch_then (qspec_then `xenv2` mp_tac)
+    \\ impl_tac THEN1 fs [result_case_eq]  \\ strip_tac
     \\ patresolve `evaluate (_, _, s0) = _` hd evaluate_changed_globals_inst
     \\ simp [] \\ strip_tac \\ fs []
     \\ fs [co_every_Fn_vs_NONE_shift_seq,
@@ -2850,21 +2976,17 @@ val known_correct0 = Q.prove(
            unique_set_globals_shift_seq]
     \\ patresolve `known _ _ _ g0 = _` hd known_preserves_esgc_free
     \\ simp [] \\ strip_tac
-    \\ patresolve `evaluate (_, _, s0) = _` (el 2) known_correct_approx_no_extra
+    \\ patresolve `evaluate (_, _, s0) = _` (el 2) known_correct_approx
     \\ rpt (disch_then drule \\ simp [])
     \\ impl_tac THEN1 metis_tac [subspt_trans]
     \\ strip_tac \\ rveq \\ fs []
-    (*  *)
     \\ reverse (fs [inlD_case_eq]) \\ rveq
-
-    
     THEN1
      ((* inlD_LetInline *)
       imp_res_tac decide_inline_LetInline_IMP_Clos_fv_max \\ rveq
       \\ reverse (Cases_on `pure x1`) \\ fs []
       \\ rpt (pairarg_tac \\ fs []) \\ rveq
       \\ imp_res_tac known_sing_EQ_E \\ fs [] \\ rveq
-
       THEN1
        ((* not pure *)
         simp [evaluate_def, evaluate_append]
@@ -2879,6 +3001,7 @@ val known_correct0 = Q.prove(
                \\ imp_res_tac oracle_states_subspt_shift_seq
                \\ fs [oracle_states_subspt_def, shift_seq_def])
         \\ first_x_assum drule \\ rpt (disch_then drule \\ simp [])
+        \\ disch_then (qspec_then `xenv2` mp_tac)
         \\ simp [co_disjoint_globals_shift_seq]
         \\ impl_tac THEN1 (fs [result_case_eq] \\ metis_tac [subspt_trans])
         \\ strip_tac
@@ -2886,25 +3009,20 @@ val known_correct0 = Q.prove(
         \\ patresolve `evaluate (_, _, s1) = _` hd evaluate_changed_globals
         \\ simp [] \\ strip_tac \\ fs []
         \\ imp_res_tac evaluate_SING \\ rveq \\ fs []
-
-        \\ patresolve `evaluate (_, _, s1) = _` (el 2) known_correct_approx_no_extra
-        \\ disch_then drule \\ simp []
+        \\ patresolve `evaluate (_, _, s1) = _` (el 2) known_correct_approx
+        \\ rpt (disch_then drule \\ simp [])
         \\ disch_then (qspec_then `g'` mp_tac)
         \\ simp [co_disjoint_globals_shift_seq,
                  unique_set_globals_shift_seq]
         \\ `subspt g g'` by metis_tac [subspt_trans]
         \\ simp [] \\ strip_tac \\ rveq
-
-
         \\ rename1 `known (dec_inline_factor _) [body] _ g = ([(ebody, abody)], gdead)`
         \\ qmatch_assum_abbrev_tac `v_rel _ _ lhclos _`
-
         \\ rename1 `evaluate (_, _, s0) = (Rval args, _)`
-
-        \\ `?rhenv. v_rel_app c g' lhclos (Closure (SOME m) [] rhenv (LENGTH xs) ebody) args`
-           by (UNABBREV_TAC "lhclos"
-               \\ fs [v_rel_app_def]
-               \\ rpt (asm_exists_tac \\ simp [])
+        \\ `v_rel_app c g' lhclos (Closure (SOME m) [] ([r1] ++ env2 ++ xenv2) (LENGTH xs) ebody) (SOME args)`
+           by (fs [Abbr `lhclos`, v_rel_app_def]
+               \\ qexists_tac `[]` \\ qexists_tac `[]` \\ simp []
+               \\ asm_exists_tac \\ simp []
                \\ fs [exp_rel_def] \\ rveq
                \\ fs [dec_inline_factor_def]
                \\ simp [known_extra]
@@ -2914,18 +3032,25 @@ val known_correct0 = Q.prove(
                \\ rveq \\ fs []
                \\ patresolve `known _ [_] _ g1 = _` hd known_preserves_esgc_free
                \\ simp [])
-
-        \\ fs [oracle_state_sgc_free_shift_seq,
-               co_every_Fn_vs_NONE_shift_seq,
-               oracle_states_subspt_shift_seq]
-
         \\ first_x_assum drule (* inst. evaluate_app i.h. *)
+        \\ imp_res_tac nil_unique_set_globals
+        \\ simp [oracle_state_sgc_free_shift_seq,
+                 co_every_Fn_vs_NONE_shift_seq,
+                 oracle_states_subspt_shift_seq,
+                 unique_set_globals_shift_seq,
+                 co_disjoint_globals_shift_seq]
         \\ rpt (disch_then drule \\ simp [])
         \\ disch_then (qspec_then `SOME m` mp_tac)
         \\ simp [loptrel_def]
         \\ imp_res_tac evaluate_IMP_LENGTH \\ fs []
-        \\ impl_tac THEN1 fs [decide_inline_def, bool_case_eq]
-
+        \\ impl_tac
+        THEN1 (fs [decide_inline_def, bool_case_eq]
+               \\ simp [NOT_NIL_EQ_LENGTH_NOT_0]
+               \\ simp [Abbr `lhclos`, dest_closure_def]
+               \\ simp [DROP_NIL]
+               \\ simp [check_loc_def]
+               \\ fs [dest_closure_def]
+               \\ cheat (* LENGTH args <= s2.max_app *))
         \\ qmatch_goalsub_rename_tac `evaluate_app _ _ args2 t2`
         \\ `args2 <> []` by fs [NOT_NIL_EQ_LENGTH_NOT_0]
         \\ simp [evaluate_app_exact_rw]
@@ -2933,99 +3058,172 @@ val known_correct0 = Q.prove(
         \\ `t2.clock = s2.clock` by fs [state_rel_def]
         \\ simp [evaluate_mk_Ticks_rw]
         \\ fs [bool_case_eq] \\ rveq \\ fs []
-
-        \\ fixeqs
-
-        \\ cheat)
+        \\ `args2 ⧺ [r1] ⧺ env2 ⧺ xenv2 = args2 ⧺ r1::(env2 ⧺ xenv2)` by simp [APPEND_ASSOC]
+        \\ rewrite_tac [GSYM APPEND_ASSOC, APPEND]
+        \\ metis_tac [])
       THEN1
-       ((* pure *) cheat))
-
-    THEN1 cheat
-    THEN1 cheat)
-
-      
-(*
-    (* Cases split on annotate or inline *)
-    \\ Cases_on `SND limit = 0 \/ body_opt = NONE`
+       ((* pure *)
+        simp [evaluate_def, evaluate_append]
+        \\ fs [result_case_eq] \\ rveq \\ fs []
+        \\ fs [pair_case_eq] \\ rveq \\ fs []
+        \\ rename1 `evaluate (_, _ s1) = (_, s2)`
+        \\ `subspt (next_g s2) (next_g s)`
+           by (simp [next_g_def]
+               \\ fs [result_case_eq]
+               \\ imp_res_tac evaluate_app_IMP_shift_seq
+               \\ imp_res_tac evaluate_IMP_shift_seq \\ fs []
+               \\ imp_res_tac oracle_states_subspt_shift_seq
+               \\ fs [oracle_states_subspt_def, shift_seq_def])
+        \\ first_x_assum drule \\ rpt (disch_then drule \\ simp [])
+        \\ disch_then (qspec_then `xenv2` mp_tac)
+        \\ simp [co_disjoint_globals_shift_seq]
+        \\ impl_tac THEN1 (fs [result_case_eq] \\ metis_tac [subspt_trans])
+        \\ strip_tac
+        \\ reverse (fs [result_case_eq]) \\ rveq \\ fs [] \\ rveq
+        THEN1 (rename1 `evaluate ([x1], _, _) = (Rerr err_res, _)`
+               \\ drule (pure_correct |> GEN_ALL |> INST_TYPE [``:'c`` |-> ``:val_approx num_map#'c``])
+               \\ disch_then (qspecl_then [`s1`, `env1 ++ xenv1`] mp_tac)
+               \\ simp [] \\ strip_tac \\ Cases_on `err_res` \\ fs [])
+        \\ patresolve `evaluate (_, _, s1) = _` hd evaluate_changed_globals
+        \\ simp [] \\ strip_tac \\ fs []
+        \\ imp_res_tac evaluate_SING \\ rveq \\ fs []
+        \\ patresolve `evaluate (_, _, s1) = _` (el 2) known_correct_approx
+        \\ rpt (disch_then drule \\ simp [])
+        \\ disch_then (qspec_then `g'` mp_tac)
+        \\ simp [co_disjoint_globals_shift_seq,
+                 unique_set_globals_shift_seq]
+        \\ `subspt g g'` by metis_tac [subspt_trans]
+        \\ simp [] \\ strip_tac \\ rveq
+        \\ rename1 `known (dec_inline_factor _) [body] _ g = ([(ebody, abody)], gdead)`
+        \\ qmatch_assum_abbrev_tac `v_rel _ _ lhclos _`
+        \\ rename1 `evaluate (_, _, s0) = (Rval args, _)`
+        \\ `v_rel_app c g' lhclos (Closure (SOME m) [] (env2 ++ xenv2) (LENGTH xs) ebody) (SOME args)`
+           by (fs [Abbr `lhclos`, v_rel_app_def]
+               \\ qexists_tac `[]` \\ qexists_tac `[]` \\ simp []
+               \\ asm_exists_tac \\ simp []
+               \\ fs [exp_rel_def] \\ rveq
+               \\ fs [dec_inline_factor_def]
+               \\ simp [known_extra]
+               \\ goal_assum (first_assum o mp_then (Pos last) mp_tac)
+               \\ `g = gdead` by (match_mp_tac known_unchanged_globals
+                                  \\ asm_exists_tac \\ simp [])
+               \\ rveq \\ fs []
+               \\ patresolve `known _ [_] _ g1 = _` hd known_preserves_esgc_free
+               \\ simp [])
+        \\ first_x_assum drule (* inst. evaluate_app i.h. *)
+        \\ imp_res_tac nil_unique_set_globals
+        \\ simp [oracle_state_sgc_free_shift_seq,
+                 co_every_Fn_vs_NONE_shift_seq,
+                 oracle_states_subspt_shift_seq,
+                 unique_set_globals_shift_seq,
+                 co_disjoint_globals_shift_seq]
+        \\ rpt (disch_then drule \\ simp [])
+        \\ disch_then (qspec_then `SOME m` mp_tac)
+        \\ simp [loptrel_def]
+        \\ imp_res_tac evaluate_IMP_LENGTH \\ fs []
+        \\ impl_tac
+        THEN1 (fs [decide_inline_def, bool_case_eq]
+               \\ simp [NOT_NIL_EQ_LENGTH_NOT_0]
+               \\ simp [Abbr `lhclos`, dest_closure_def]
+               \\ simp [DROP_NIL]
+               \\ simp [check_loc_def]
+               \\ fs [dest_closure_def]
+               \\ cheat (* LENGTH args <= s2.max_app *))
+        \\ qmatch_goalsub_rename_tac `evaluate_app _ _ args2 t2`
+        \\ `args2 <> []` by fs [NOT_NIL_EQ_LENGTH_NOT_0]
+        \\ simp [evaluate_app_exact_rw]
+        \\ strip_tac
+        \\ `t2.clock = s2.clock` by fs [state_rel_def]
+        \\ patresolve `known _ [x1] _ _ = ([e1, _], _)` hd known_preserves_pure
+        \\ simp [] \\ strip_tac
+        \\ drule (GEN_ALL pure_correct)
+        \\ disch_then (qspecl_then [`t`, `env2 ++ xenv2`] mp_tac)
+        \\ simp [] \\ strip_tac \\ rveq \\ fs []
+        \\ simp [evaluate_mk_Ticks_rw]))
     THEN1
-     (rename1 `App tr new_loc_opt e1 (MAP FST ea2)`
-      \\ `eas = [(App tr new_loc_opt e1 (MAP FST ea2),Other)]` by (fs [] \\ fs [])
-      \\ qpat_x_assum `_ \/ _` kall_tac
-      \\ qpat_x_assum `(if SND limit = 0 then _ else _) = _` kall_tac
-      \\ rveq
-      \\ fs [evaluate_def, bool_case_eq, pair_case_eq]
-      \\ first_x_assum drule
-      \\ rpt (disch_then drule \\ simp [])
-      \\ fs [result_case_eq] \\ rveq \\ fs []
-      \\ strip_tac \\ fs [] \\ rveq
+     ((* inlD_Annotate *)
+      simp [evaluate_def]
+      \\ fs [result_case_eq] \\ rveq \\ fs [] \\ rveq
       \\ fs [pair_case_eq]
-      \\ first_x_assum drule
-      \\ rpt (disch_then drule \\ simp [])
-      \\ patresolve `evaluate (_, _, s0) = _` hd evaluate_changed_globals
-      \\ simp [] \\ strip_tac \\ fs []
-      \\ fs [co_disjoint_globals_shift_seq,
-             unique_set_globals_shift_seq,
-             co_every_Fn_vs_NONE_shift_seq,
-             oracle_state_sgc_free_shift_seq]
-      \\ patresolve `known _ _ _ g0 = _` hd known_preserves_esgc_free
-      \\ simp [] \\ strip_tac
-      \\ patresolve `known _ _ _ g0 = _` hd known_correct_approx
-      \\ disch_then drule \\ simp []
-      \\ imp_res_tac known_sing_EQ_E \\ fs [] \\ rveq
-      \\ patresolve `LIST_REL _ env1 env2` hd v_rel_EVERY_vsgc_free
-      \\ simp [] \\ strip_tac
-      \\ qpat_x_assum `state_rel _ _ s0 _` assume_tac
-      \\ drule state_rel_ssgc_free \\ simp []
-      \\ strip_tac
-      \\ disch_then (qpat_assum `state_globals_approx _ _` o mp_then Any mp_tac)
-      \\ simp []
-      \\ drule state_rel_unique_set_globals \\ simp []
-      \\ disch_then kall_tac
-      \\ drule state_rel_co_disjoint_globals \\ simp []
-      \\ disch_then kall_tac
-      \\ strip_tac \\ rveq \\ fs []
-      \\ qpat_x_assum `state_rel _ _ s1 _` assume_tac
-      \\ drule state_rel_state_globals_approx \\ strip_tac \\ fs []
-      \\ fs [result_case_eq] \\ fs [] \\ rveq
-      \\ strip_tac \\ rveq \\ fs []
-      \\ imp_res_tac evaluate_SING
-      \\ rveq \\ fs []
+      \\ rename1 `evaluate ([_], _ s1) = (_, s2)`
+      \\ `subspt (next_g s2) (next_g s)`
+          by (simp [next_g_def]
+              \\ fs [result_case_eq]
+              \\ imp_res_tac evaluate_app_IMP_shift_seq
+              \\ imp_res_tac evaluate_IMP_shift_seq \\ fs []
+              \\ imp_res_tac oracle_states_subspt_shift_seq
+              \\ fs [oracle_states_subspt_def, shift_seq_def])
+      \\ `subspt g (next_g s1) ∧ subspt (next_g s2) g'` by metis_tac [subspt_trans]
+      \\ first_x_assum drule \\ rpt (disch_then drule \\ simp [])
+      \\ simp [co_disjoint_globals_shift_seq]
+      \\ disch_then (qspec_then `xenv2` mp_tac)
+      \\ imp_res_tac known_sing_EQ_E
+      \\ fs [result_case_eq] \\ strip_tac \\ rveq \\ fs []
+      \\ imp_res_tac evaluate_SING \\ fs [] \\ rveq
+      \\ first_x_assum match_mp_tac
+      \\ imp_res_tac nil_unique_set_globals
       \\ patresolve `evaluate (_, _, s1) = _` hd evaluate_changed_globals_inst
       \\ simp [] \\ strip_tac \\ fs []
-      \\ first_x_assum match_mp_tac \\ fs []
-      \\ `oracle_state_sgc_free s2.compile_oracle` by fs [oracle_state_sgc_free_shift_seq]
-      \\ rfs []
-      \\ patresolve `known _ _ _ g1 = _` hd known_correct_approx
-      \\ simp []
-      \\ disch_then drule \\ simp []
-      \\ disch_then (qspec_then `g'` mp_tac) \\ simp []
-      \\ qpat_x_assum `state_rel _ _ s1 _` assume_tac
-      \\ drule state_rel_ssgc_free
-      \\ simp [oracle_state_sgc_free_shift_seq]
-      \\ strip_tac
-      \\ `oracle_state_sgc_free s1.compile_oracle` by fs [oracle_state_sgc_free_shift_seq]
-      \\ `unique_set_globals [x1] s1.compile_oracle` by fs [unique_set_globals_shift_seq]
-      \\ `co_disjoint_globals g' s1.compile_oracle` by fs [co_disjoint_globals_shift_seq]
-      \\ rfs []
-      \\ drule state_rel_unique_set_globals \\ simp []
-      \\ disch_then kall_tac
-      \\ drule state_rel_co_disjoint_globals \\ simp []
-      \\ disch_then kall_tac
-      \\ strip_tac
-      \\ qpat_x_assum `state_rel _ _ s2 _` assume_tac
-      \\ drule state_rel_state_globals_approx
+      \\ simp [co_every_Fn_vs_NONE_shift_seq,
+               oracle_states_subspt_shift_seq,
+               oracle_state_sgc_free_shift_seq,
+               co_disjoint_globals_shift_seq,
+               unique_set_globals_shift_seq]
+      \\ qexists_tac `NONE` \\ simp [v_rel_app_NONE]
+      \\ patresolve `evaluate (_, _, s1) = _` (el 2) known_correct_approx
+      \\ rpt (disch_then drule \\ simp [])
+      \\ disch_then (qspec_then `g'` mp_tac)
+      \\ simp [co_disjoint_globals_shift_seq,
+               unique_set_globals_shift_seq]
+      \\ impl_tac THEN1 metis_tac [subspt_trans]
       \\ strip_tac \\ simp []
-      \\ rename1 `dest_Clos fapx`
-      \\ Cases_on `dest_Clos fapx` \\ fs []
-      THEN1 fs [loptrel_def] \\ rveq \\ fs []
-      \\ Cases_on `lopt1` \\ fs []
-      THEN1 (simp [loptrel_def]
-             \\ rename1 `dest_Clos fapx = SOME clos_apx`
-             \\ `?clos_loc clos_arity clos_body. clos_apx = (clos_loc, clos_arity, clos_body)`
-                by (Cases_on `fapx` \\ fs [] \\ metis_tac [])
-             \\ fs [bool_case_eq] \\ metis_tac [evaluate_IMP_LENGTH])
+      \\ imp_res_tac evaluate_IMP_LENGTH
       \\ simp [loptrel_def]
-      \\ fs [pair_case_eq, bool_case_eq]) *)
+      \\ fs [decide_inline_def, va_case_eq, bool_case_eq]
+      \\ rveq \\ fs [] \\ rveq \\ fs []
+      \\ imp_res_tac LIST_REL_LENGTH \\ fs []
+      \\ rename1 `FST (EL jj fns1) = FST (EL jj fns2)`
+      \\ qpat_x_assum `LIST_REL (f_rel _ _ _) _ _` mp_tac
+      \\ simp [LIST_REL_EL_EQN] \\ disch_then (qspec_then `jj` mp_tac)
+      \\ Cases_on `EL jj fns1` \\ Cases_on `EL jj fns2`
+      \\ simp [f_rel_def])
+    THEN1
+     ((* inlD_Nothing *)
+      simp [evaluate_def]
+      \\ fs [result_case_eq] \\ rveq \\ fs [] \\ rveq
+      \\ fs [pair_case_eq]
+      \\ rename1 `evaluate ([_], _ s1) = (_, s2)`
+      \\ `subspt (next_g s2) (next_g s)`
+          by (simp [next_g_def]
+              \\ fs [result_case_eq]
+              \\ imp_res_tac evaluate_app_IMP_shift_seq
+              \\ imp_res_tac evaluate_IMP_shift_seq \\ fs []
+              \\ imp_res_tac oracle_states_subspt_shift_seq
+              \\ fs [oracle_states_subspt_def, shift_seq_def])
+      \\ `subspt g (next_g s1) ∧ subspt (next_g s2) g'` by metis_tac [subspt_trans]
+      \\ first_x_assum drule \\ rpt (disch_then drule \\ simp [])
+      \\ simp [co_disjoint_globals_shift_seq]
+      \\ disch_then (qspec_then `xenv2` mp_tac)
+      \\ imp_res_tac known_sing_EQ_E
+      \\ fs [result_case_eq] \\ strip_tac \\ rveq \\ fs []
+      \\ imp_res_tac evaluate_SING \\ fs [] \\ rveq
+      \\ first_x_assum match_mp_tac
+      \\ imp_res_tac nil_unique_set_globals
+      \\ patresolve `evaluate (_, _, s1) = _` hd evaluate_changed_globals_inst
+      \\ simp [] \\ strip_tac \\ fs []
+      \\ simp [co_every_Fn_vs_NONE_shift_seq,
+               oracle_states_subspt_shift_seq,
+               oracle_state_sgc_free_shift_seq,
+               co_disjoint_globals_shift_seq,
+               unique_set_globals_shift_seq]
+      \\ qexists_tac `NONE` \\ simp [v_rel_app_NONE]
+      \\ patresolve `evaluate (_, _, s1) = _` (el 2) known_correct_approx
+      \\ rpt (disch_then drule \\ simp [])
+      \\ disch_then (qspec_then `g'` mp_tac)
+      \\ simp [co_disjoint_globals_shift_seq,
+               unique_set_globals_shift_seq]
+      \\ impl_tac THEN1 metis_tac [subspt_trans]
+      \\ simp [loptrel_def]))
 
   THEN1
    (say "Tick"
@@ -3083,7 +3281,7 @@ val known_correct0 = Q.prove(
         \\ qexists_tac `aenv` \\ simp [] 
         \\ rveq \\ simp []
         \\ irule EVERY2_APPEND_suff \\ simp [])
-      THEN1 cheat)
+      THEN1 cheat (* Recclosure *))
 
     THEN1 ((* dest_closure returns Full_app *)    
       Cases_on `argsopt` \\ fs [] \\ rveq
@@ -3114,8 +3312,6 @@ val known_correct0 = Q.prove(
                            \\ asm_exists_tac \\ simp [])
           \\ disch_then drule
           \\ simp [v_rel_upd_inline_factor, state_rel_upd_inline_factor]
-
-
           \\ qmatch_asmsub_abbrev_tac `evaluate (_, fullenv1, state1)`
           \\ qmatch_goalsub_abbrev_tac `evaluate (_, fullenv2, state2)`
           \\ `LIST_REL (v_rel c g) fullenv1 fullenv2`
@@ -3129,10 +3325,14 @@ val known_correct0 = Q.prove(
           \\ disch_then drule \\ simp []
           \\ simp [set_globals_empty_esgc_free]
           \\ simp [EVERY_REVERSE, EVERY_TAKE]
-          \\ `fv_max (num_args + LENGTH env2) [e]` by cheat
+
+          \\ `fv_max (num_args + LENGTH env2) [e]`
+             by (
+
+                 cheat)
+
           \\ simp [set_globals_empty_unique_set_globals]
           \\ rename1 `evaluate (_, _, state1) = (_, s1)`
-
           \\ rveq
           \\ `subspt (next_g state1) (next_g s1)`
              by (fs [Abbr `state1`]
@@ -3144,33 +3344,41 @@ val known_correct0 = Q.prove(
                  \\ imp_res_tac oracle_states_subspt_shift_seq
                  \\ simp [shift_seq_def]
                  \\ irule oracle_states_subspt_alt \\ simp [])
-
           \\ simp []
-
           \\ impl_tac
-          \\ rpt conj_tac
-
-          THEN1 cheat
-          THEN1 cheat
-          THEN1 (simp [Abbr `fullenv1`]
-                 \\ irule EVERY2_APPEND_suff \\ simp []
-                 \\ simp [LIST_REL_EL_EQN, EL_REPLICATE])
-          THEN1 (fs [result_case_eq])
+          THEN1
+           (rpt conj_tac
+            THEN1 cheat (* subspt g0 (next_g s0) *)
+            THEN1 cheat (* subspt (next_g s0) g *)
+            THEN1 (simp [Abbr `fullenv1`]
+                   \\ irule EVERY2_APPEND_suff \\ simp []
+                   \\ simp [LIST_REL_EL_EQN, EL_REPLICATE])
+            THEN1 fs [result_case_eq])
           \\ strip_tac \\ fs []
           \\ fs [result_case_eq] \\ rveq \\ fs [] \\ rveq
           \\ imp_res_tac evaluate_SING \\ rveq \\ fs []
-
+          \\ reverse (Cases_on `lopt1 = lopt2`)
+          THEN1
+           (fs [loptrel_def]
+            \\ Cases_on `lopt2` \\ fs []
+            \\ Cases_on `loc` \\ fs [] \\ rveq \\ fs []
+            \\ rename1 `evaluate_app lopt1 f1' _ _ = _`
+            \\ qmatch_assum_abbrev_tac `evaluate_app lopt1 f1' next_args1 _ = _`
+            \\ qmatch_goalsub_abbrev_tac `evaluate_app _ _ next_args2 _ = _`
+            \\ `next_args1 = []` by fs [Abbr `next_args1`, DROP_NIL]
+            \\ `next_args2 = []` by fs [Abbr `next_args2`, DROP_NIL]
+            \\ fs [Abbr `next_args1`, Abbr `next_args2`]
+            \\ rveq \\ simp [])
           \\ first_x_assum match_mp_tac
           \\ qexists_tac `NONE` \\ simp []
-
           \\ patresolve `evaluate (_, _, state1) = _` hd evaluate_changed_globals
           \\ patresolve `evaluate (_, _, state1) = _` (el 2) known_correct_approx_no_extra
           \\ unabbrev_all_tac
           \\ rpt (disch_then drule \\ simp [])
           \\ disch_then (qspec_then `g` mp_tac)
           \\ simp [set_globals_empty_esgc_free]
-          \\ simp [EVERY_REVERSE, EVERY_TAKE]
           \\ simp [set_globals_empty_unique_set_globals]
+          \\ simp [EVERY_REVERSE, EVERY_TAKE]
           \\ impl_tac THEN1 (irule EVERY2_APPEND_suff \\ simp []
                              \\ simp [LIST_REL_EL_EQN, EL_REPLICATE])
           \\ strip_tac \\ strip_tac
@@ -3183,2230 +3391,160 @@ val known_correct0 = Q.prove(
           \\ simp [v_rel_app_NONE]
           \\ conj_tac THEN1 (irule EVERY2_DROP 
                              \\ irule EVERY2_APPEND_suff \\ simp [])
+          \\ simp [loptrel_def])
+        THEN1 cheat (* Recclosure *))
+      THEN1 ((* ISSOME argsopt *)
+        dsimp [] \\ disj2_tac
+        \\ fs [bool_case_eq] \\ rveq \\ fs []
+        THEN1
+         (drule dest_closure_SOME_IMP \\ strip_tac \\ rveq
+          \\ fs [v_rel_app_def] \\ rveq \\ fs []
+          \\ fs [dest_closure_def] \\ rveq \\ fs []
+          \\ imp_res_tac LIST_REL_LENGTH
+          \\ TRY (rpt (pairarg_tac \\ fs [])
+                  \\ rename1 `LIST_REL (f_rel _ _ _) funs1 funs2`
+                  \\ rename1 `EL i funs1 = (num_args1, _)`
+                  \\ rename1 `EL i funs2 = (num_args2, _)`
+                  \\ `num_args1 = num_args2`
+                     by (fs [NOT_LESS_EQUAL, LIST_REL_EL_EQN]
+                         \\ first_x_assum (qpat_assum `i < _` o mp_then (Pos hd) mp_tac)
+                         \\ simp [f_rel_def]))
+          \\ fs [bool_case_eq] \\ rveq
+          \\ qexists_tac `t0 with clock := 0`
+          \\ fs [CONV_RULE (LHS_CONV SYM_CONV) REVERSE_EQ_NIL]
+          \\ fs [DROP_NIL, NOT_LESS, ADD1, GREATER_EQ]
+          \\ imp_res_tac LESS_EQUAL_ANTISYM \\ fs []
+          \\ fs [state_rel_def]
+          \\ Cases_on `lopt1 = lopt2`
           \\ fs [loptrel_def]
           \\ Cases_on `lopt2` \\ fs []
-          \\ Cases_on `loc` \\ fs [] \\ rveq \\ fs []
-
-          \\ rename1 `evaluate_app _ f1 _`
-          \\ qmatch_asmsub_abbrev_tac `evaluate_app _ _ args`
-
-          \\ fs [evaluate_app_rw]
-
-
-         )        
-        \\ rpt (pairarg_tac \\ fs [])
-        \\ 
-
-       )
-
-
-
-      \\ fs [DROP_NIL]
-      \\ fs [DROP_LENGTH_TOO_LONG, LENGTH_REVERSE]
-
-      \\ rfs [DROP_LENGTH_TOO_LONG, LENGTH_REVERSE]
-      \\ fs [DROP_NIL]
-
-      \\ fs [TAKE_LENGTH_ID_rwt]
-      \\ fs [REVERSE_APPEND]
-
-      \\ rfs [] \\ fs []
-
-      \\ fs [pair_case_eq]
-      \\ first_x_assum drule
-      \\ fs [exp_rel_def]
-      \\ disch_then drule
-      \\ fs [PULL_EXISTS]
-      \\ drule v_rel_upd_inline_factor
-      \\ disch_then (qspec_then `k` assume_tac)
-      \\ disch_then drule \\ simp []
-      \\ fs [v_rel_upd_inline_factor]
-
-      \\ fs [pair_case_eq, result_case_eq]
-      \\ fs [list_case_eq] \\ rveq \\ fs []
-
-      \\ fs [PULL_EXISTS]
-
-
-        \\ fs [loptrel_def, check_loc_def] \\ EVERY_CASE_TAC \\ fs []
-
-        \\ qexists_tac `aenv` \\ simp [] 
-        \\ rveq \\ simp []
-        \\ irule EVERY2_APPEND_suff \\ simp [])
-      
-
-      \\ rename1 `LIST_REL (v_rel _ _) xs ys`
-      \\ rename1 `v_rel _ _ x y`
-      \\ fs [bool_case_eq]
-      THEN1
-       (rveq \\ fs []
-        \\ imp_res_tac dest_closure_SOME_IMP \\ fs [] \\ rveq
-        \\ imp_res_tac LIST_REL_LENGTH
-        \\ fs [dest_closure_def]
-        \\ fs [METIS_PROVE [] ``(if b then SOME x else SOME y) = SOME (if b then x else y)``]
+          \\ Cases_on `loc` \\ fs [] \\ rveq
+          \\ fs [check_loc_def])
         THEN1
-         (IF_CASES_TAC \\ fs [] \\ rveq
-          \\ fs [LENGTH_REVERSE]
-          \\ fs [state_rel_def]
-          \\ Cases_on `lopt1` \\ fs [loptrel_def]
-          \\ EVERY_CASE_TAC \\ fs [check_loc_def])
-        \\ rpt (pairarg_tac \\ fs [])
-        \\ qpat_x_assum `LIST_REL (f_rel _ _ _) _ _` assume_tac
-        \\ drule (LIST_REL_EL_EQN |> SPEC_ALL |> EQ_IMP_RULE |> fst |> GEN_ALL) \\ fs []
-        \\ disch_then (qspec_then `i` mp_tac) \\ simp [] \\ strip_tac
-        \\ fs [f_rel_def] \\ rveq
-        \\ IF_CASES_TAC \\ fs [] \\ rveq
-        \\ fs [LENGTH_REVERSE]
-        \\ fs [state_rel_def]
-        \\ Cases_on `lopt1` \\ fs [loptrel_def]
-        \\ EVERY_CASE_TAC \\ fs [check_loc_def])
-
-      \\ fs [pair_case_eq]
-      \\ first_x_assum drule
-      \\ imp_res_tac dest_closure_SOME_IMP \\ fs [] \\ rveq
-      \\ fs [exp_rel_def]
-
-      THEN1
-       (fs [dest_closure_def, bool_case_eq] \\ rveq
-        \\ disch_then drule
-        \\ fs []
-
-
-    \\ fs [evaluate_def] \\ rveq
-
-    \\ fs [option_case_eq]
-    \\ rename1 `_ = SOME vv`
-
-    \\ imp_res_tac dest_closure_SOME_IMP \\ fs [loptrel_def] \\ rveq \\ fs []
-    \\ fs [dest_closure_def]
-
-    \\ Cases_on `f1` \\ rveq \\ fs [dest_closure_def]
-
-    \\ `?exp env. vv = Full_app exp env []`
-    \\ fs [dest_closure_def]
-
-    \\ fs [loptrel_def]
-
-loptrel_def
-
-    \\ cheat));
-
-
-(*
-  `(∀a es env1 env2 (s01:('a,'b) closSem$state) s02 res1 s1 g0 g g' as ealist.
-
-
-
-
-       ⇒
-      ∃res2 s2.
-        evaluate(MAP FST ealist, env2, s02) = (res2, s2) ∧
-        krrel g' (res1,s1) (res2,s2)) ∧
-   (∀lopt1 f1 args1 (s01:('a,'b) closSem$state) res1 s1 lopt2 f2 args2 s02 g.
-      evaluate_app lopt1 f1 args1 s01 = (res1,s1) ∧ ssgc_free s01 ∧
-      kvrel g f1 f2 ∧ LIST_REL (kvrel g) args1 args2 ∧
-      ksrel g s01 s02 ∧ state_globals_approx s01 g ∧ vsgc_free f1 ∧
-      EVERY vsgc_free args1 ∧ loptrel f2 (LENGTH args1) lopt1 lopt2 ⇒
-      ∃res2 s2.
-        evaluate_app lopt2 f2 args2 s02 = (res2,s2) ∧
-        krrel g (res1,s1) (res2,s2))`,
-  ho_match_mp_tac evaluate_ind >> rpt conj_tac
-  >- (say "nil" >> simp[evaluate_def, known_def])
-  >- (say "cons" >>
-      simp[evaluate_def, known_def, pair_case_eq, result_case_eq,
-           BAG_ALL_DISTINCT_BAG_UNION] >>
-      rpt strip_tac >> rveq >> rpt (pairarg_tac >> fs[]) >> rveq >> simp[] >>
-      first_x_assum (patresolve `known [_] _ _ = _` last) >>
-      disch_then (resolve_selected (el 4)) >> simp[] >>
-      patresolve `known [_] _ _ = _` hd subspt_known_elist_globals >> simp[] >>
-      disch_then (resolve_selected hd) >> simp[] >> strip_tac >>
-      disch_then (resolve_selected last) >> simp[] >>
-      (impl_keep_tac >- metis_tac[subspt_trans]) >>
-      rw[]
-      >- (imp_res_tac known_sing_EQ_E >> rveq >> fs[] >>
-          sel_ihpc last >> simp[] >> disch_then (resolve_selected (el 3)) >>
-          simp[] >> disch_then (resolve_selected hd) >> simp[] >> impl_tac
-          >- (conj_tac
-              >- (resolve_selected hd (GEN_ALL kca_sing_sga) >> simp[] >>
-                  disch_then (resolve_selected last) >> simp[] >>
-                  metis_tac[kvrel_LIST_REL_val_approx, kvrel_EVERY_vsgc_free,
-                            ksrel_sga, ksrel_ssgc_free]) >>
-              metis_tac[ssgc_free_preserved_SING']) >> rw[] >>
-          simp[Once evaluate_CONS] >> imp_res_tac evaluate_SING >> rveq >>
-          fs[])
-      >- (imp_res_tac known_sing_EQ_E >> rveq >> fs[] >> sel_ihpc last >>
-          simp[] >> disch_then (resolve_selected (el 3)) >> simp[] >>
-          disch_then (resolve_selected hd) >> simp[] >> impl_tac
-          >- (conj_tac
-              >- (resolve_selected hd (GEN_ALL kca_sing_sga) >> simp[] >>
-                  disch_then (resolve_selected last) >> simp[] >>
-                  metis_tac[kvrel_LIST_REL_val_approx, kvrel_EVERY_vsgc_free,
-                            ksrel_sga, ksrel_ssgc_free]) >>
-              metis_tac[ssgc_free_preserved_SING']) >> rw[] >>
-          simp[Once evaluate_CONS, result_case_eq] >> fs[krrel_err_rw] >>
-          dsimp[] >> metis_tac[result_CASES])
-      >- (imp_res_tac known_sing_EQ_E >> rveq >> fs[] >>
-          simp[Once evaluate_CONS, result_case_eq, pair_case_eq] >>
-          dsimp[] >> fs[krrel_err_rw] >> metis_tac[pair_CASES, result_CASES]))
-  >- (say "var" >>
-      simp[evaluate_def, bool_case_eq, known_def] >>
-      rpt strip_tac >> fs[LIST_REL_EL_EQN])
-  >- (say "if" >>
-      simp[evaluate_def, pair_case_eq, bool_case_eq, BAG_ALL_DISTINCT_BAG_UNION,
-           result_case_eq, known_def] >> rpt strip_tac >> rveq >> fs[] >>
-      rpt (pairarg_tac >> fs[]) >> rveq >> fs[] >> fixeqs >>
-      imp_res_tac known_sing_EQ_E >> rveq >> fs[] >> rveq >>
-      map_every rename1 [`ksrel g' s01 s02`, `subspt g g'`,
-                           `known [eb] as g2 = ([(eb',eapx)], g)`,
-                           `known [tb] as g1 = ([(tb',tapx)], g2)`,
-                           `known [gd] as g0 = ([(gd',gapx)], g1)`] >>
-      `known [gd;tb] as g0 = ([(gd',gapx); (tb',tapx)], g2)`
-        by simp[known_def] >>
-      resolve_selected hd (subspt_known_elist_globals)>> simp[] >>
-      disch_then (resolve_selected hd) >> simp[] >> strip_tac >>
-      patresolve `known [gd] _ _ = _` hd subspt_known_elist_globals >> simp[] >>
-      disch_then (resolve_selected hd) >> simp[] >> strip_tac
-      >- (first_x_assum (patresolve `state_globals_approx _ _` (el 6)) >>
-          rpt (disch_then (resolve_selected last) >> simp[]) >>
-          impl_keep_tac >- metis_tac[subspt_trans] >> rw[] >>
-          simp[evaluate_def] >> imp_res_tac evaluate_SING >> fs[] >> rveq >>
-          fs[] >> rveq >> sel_ihpc last >> simp[] >> disch_then irule >>
-          simp[]
-          >- metis_tac[ssgc_free_preserved_SING']
-          >- (patresolve `known [gd] _ _ = _` hd (GEN_ALL kca_sing_sga) >>
-              simp[] >> disch_then (resolve_selected last) >> simp[] >>
-              metis_tac[ksrel_sga, kvrel_LIST_REL_val_approx,
-                        kvrel_EVERY_vsgc_free, ksrel_ssgc_free])
-          >- metis_tac[subspt_trans])
-      >- (first_x_assum (patresolve `state_globals_approx _ _` (el 6)) >>
-          rpt (disch_then (resolve_selected last) >> simp[]) >>
-          impl_keep_tac >- metis_tac[subspt_trans] >> rw[] >>
-          simp[evaluate_def] >> imp_res_tac evaluate_SING >> fs[] >> rveq >>
-          fs[] >> rveq >> sel_ihpc last >> simp[] >> disch_then irule >>
-          simp[]
-          >- metis_tac[ssgc_free_preserved_SING']
-          >- (patresolve `known [gd] _ _ = _` hd (GEN_ALL kca_sing_sga) >>
-              simp[] >> disch_then (resolve_selected last) >> simp[] >>
-              metis_tac[ksrel_sga, kvrel_LIST_REL_val_approx,
-                        kvrel_EVERY_vsgc_free, ksrel_ssgc_free,
-                        state_approx_better_definedg, known_better_definedg]))
-      >- ((* guard doesn't evaluate to T or F *) sel_ihpc (el 6) >> simp[] >>
-          rpt (disch_then (resolve_selected last) >> simp[]) >>
-          impl_keep_tac >- metis_tac[subspt_trans] >> rw[] >>
-          simp[evaluate_def] >> imp_res_tac evaluate_SING >> fs[] >> rveq >>
-          fs[] >> rveq >> dsimp[bool_case_eq] >> rpt disj2_tac >>
-          rpt strip_tac >> rveq >> fs[])
-      >- ((* guard errors *) sel_ihpc (el 6) >> simp[] >>
-          rpt (disch_then (resolve_selected last) >> simp[]) >>
-          impl_keep_tac >- metis_tac[subspt_trans] >> rw[] >>
-          dsimp[evaluate_def, result_case_eq, bool_case_eq] >>
-          fs[krrel_err_rw] >> metis_tac[pair_CASES, result_CASES]))
-  >- (say "let" >>
-      simp[evaluate_def, pair_case_eq, result_case_eq] >>
-      rpt strip_tac >> rveq >> fs[known_def] >>
-      rpt (pairarg_tac >> fs[]) >> rveq >> fs[BAG_ALL_DISTINCT_BAG_UNION] >>
-      map_every rename1 [`known [bod] _ g1 = (_, g)`,
-                           `known _ _ g0 = (_, g1)`,
-                           `subspt g gg`] >>
-      patresolve `known _ _ g0 = _` hd subspt_known_elist_globals >> simp[] >>
-      disch_then (resolve_selected hd) >> simp[] >>
-      (impl_tac >- fs[BAG_DISJOINT, DISJOINT_SYM]) >> strip_tac >>
-      first_x_assum (patresolve `known _ _ g0 = _` last) >> simp[] >>
-      rpt (disch_then (resolve_selected last) >> simp[]) >>
-      (impl_keep_tac >- metis_tac[subspt_trans]) >> rw[] >>
-      simp[evaluate_def, result_case_eq]
-      >- (imp_res_tac known_sing_EQ_E >> rveq >> fs[] >>
-          rveq >> sel_ihpc last >> simp[] >> disch_then irule >> simp[]
-          >- metis_tac[ssgc_evaluate]
-          >- metis_tac[ssgc_evaluate,rsgc_free_def]
-          >- (resolve_selected last known_correct_approx >> simp[] >>
-              rpt (disch_then (resolve_selected hd) >> simp[]) >>
-              metis_tac[ksrel_sga, kvrel_EVERY_vsgc_free,
-                        kvrel_LIST_REL_val_approx, ksrel_ssgc_free])
-          >- simp[EVERY2_APPEND_suff]
-          >- (irule EVERY2_APPEND_suff >> simp[] >>
-              resolve_selected last known_correct_approx >> simp[] >>
-              rpt (disch_then (resolve_selected hd) >> simp[]) >>
-              metis_tac[ksrel_sga, kvrel_EVERY_vsgc_free,
-                        kvrel_LIST_REL_val_approx, ksrel_ssgc_free]))
-      >- (fs[krrel_err_rw, result_case_eq] >> dsimp[] >>
-          metis_tac[pair_CASES, result_CASES]))
-  >- (say "raise" >>
-      simp[evaluate_def, pair_case_eq, result_case_eq] >>
-      rpt strip_tac >> rveq >> fs[known_def] >> pairarg_tac >> fs[] >>
-      imp_res_tac known_sing_EQ_E >> fs[] >> rveq >> fs[] >>
-      simp[evaluate_def, pair_case_eq, result_case_eq] >>
-      nailIHx strip_assume_tac >> simp[] >> fs[]
-      >- (imp_res_tac evaluate_SING >> fs[])
-      >- (dsimp[] >> fs[krrel_err_rw] >> metis_tac[result_CASES]))
-  >- (say "handle" >>
-      simp[evaluate_def, pair_case_eq, result_case_eq,
-           BAG_ALL_DISTINCT_BAG_UNION, error_case_eq, known_def] >>
-      rpt strip_tac >> rveq >> fs[] >>
-      rpt (pairarg_tac >> fs[]) >> rveq >>
-      imp_res_tac known_sing_EQ_E >> rveq >> fs[] >> rveq >>
-      map_every rename1 [`known _ (_ :: _) g1 = (_, g)`,
-                           `known _ _ g0 = (_, g1)`,
-                           `subspt g gg`] >>
-      patresolve `known _ _ g0 = _` hd subspt_known_elist_globals >> simp[] >>
-      rpt (disch_then (resolve_selected hd) >> simp[]) >> strip_tac >>
-      first_x_assum (patresolve `state_globals_approx _ _`  (el 6)) >> simp[] >>
-      rpt (disch_then (resolve_selected last) >> simp[]) >>
-      (impl_keep_tac >- metis_tac[subspt_trans]) >> rw[] >>
-      simp[evaluate_def, pair_case_eq, result_case_eq, error_case_eq]
-      >- (dsimp[] >> fs[PULL_EXISTS] >> sel_ihpc last >> simp[] >>
-          fs[krrel_err_rw] >> disch_then irule >> simp[]
-          >- metis_tac[ssgc_free_preserved_SING']
-          >- first_assum
-               (mp_then (Pos last) (mp_tac >~ (simp[] >> NO_TAC)) ssgc_evaluate)
-          >- (patresolve `known _ _ g0 = _` hd (GEN_ALL kca_sing_sga) >>
-              simp[] >> disch_then (resolve_selected last) >> simp[] >>
-              metis_tac[ksrel_ssgc_free,kvrel_EVERY_vsgc_free,ksrel_sga,
-                        kvrel_LIST_REL_val_approx]))
-      >- (fs[krrel_err_rw, result_case_eq, error_case_eq] >> dsimp[] >>
-          metis_tac[pair_CASES, result_CASES, error_CASES]))
-  >- (say "op" >>
-      simp[evaluate_def, pair_case_eq, result_case_eq, known_def,
-           BAG_ALL_DISTINCT_BAG_UNION] >>
-      rpt gen_tac >> strip_tac >> rpt gen_tac >>
-      Cases_on `op = Install` >- cheat >>
-      rpt (pairarg_tac >> fs[]) >>
-      rename[`isGlobal opn`, `gO_destApx apx`] >>
-      cheat (*
-      Cases_on `isGlobal opn ∧ gO_destApx apx ≠ gO_None`
-      >- (pop_assum strip_assume_tac >> simp[] >>
-          Cases_on `opn` >> fs[isGlobal_def] >>
-          Cases_on `apx` >> fs[gO_destApx_def] >> rveq >>
-          fs[known_op_def, NULL_EQ, bool_case_eq, case_eq_thms] >> rveq >>
-          imp_res_tac known_LENGTH_EQ_E >> fs[LENGTH_NIL_SYM] >> rveq >>
-          simp[evaluate_def] >>
-          rpt strip_tac >> rveq >> fs[evaluate_def, do_app_def, case_eq_thms] >>
-          fs[state_globals_approx_def, subspt_def] >> rveq >> simp[] >>
-          fs[known_def] >> rveq
-          >- (rename[`lookup n g0 = SOME (Tuple tg [])`,
-                     `kvrel g1 v (Block tg [])`] >>
-              `lookup n g1 = SOME (Tuple tg [])` by metis_tac[domain_lookup] >>
-              res_tac >> fs[] >> rveq >> fs[val_approx_val_def]) >>
-          (* TODO: clos_known$ is only necessary because of HOL issue #430 *)
-          rename[`lookup n g0 = SOME (clos_known$Int i)`, `kvrel g1 v (Number i)`] >>
-          `lookup n g1 = SOME (Int i)` by metis_tac[domain_lookup] >>
-          metis_tac[val_rel_def, val_approx_val_def, SOME_11]) >>
-      rename[`closLang$Op tr opn (MAP FST es)`,
-             `closSem$evaluate(MAP FST ealist,_,_)`] >>
-      rpt strip_tac >>
-      `ealist = [(Op tr opn (MAP FST es), apx)]`
-         by (Cases_on `isGlobal opn` >> fs[] >>
-             Cases_on `apx` >> fs[gO_destApx_def] >> every_case_tac >> fs[]) >>
-      pop_assum SUBST_ALL_TAC >> rveq >>
-      qpat_x_assum `¬(_ ∧ _)` kall_tac >> fs[] >>
-      dsimp[evaluate_def, result_case_eq, pair_case_eq] >>
-      sel_ihpc last >> simp[PULL_EXISTS] >>
-      rpt (disch_then (resolve_selected last) >> simp[]) >>
-      resolve_selected hd subspt_known_op_elist_globals >> simp[] >>
-      rpt (disch_then (resolve_selected hd) >> simp[]) >> strip_tac >>
-      (impl_keep_tac >- metis_tac[subspt_trans])
-      >- ((* args evaluate OK, do_app evaluates OK *)
-          metis_tac[kvrel_op_correct_Rval, EVERY2_REVERSE])
-      >- ((* args evaluate OK, do_app errors *)
-          rw[] >> imp_res_tac do_app_EQ_Rerr >> rw[] >>
-          metis_tac[result_CASES, pair_CASES])
-      >- ((* args error *) rw[] >> fs[krrel_err_rw] >>
-         metis_tac[result_CASES, pair_CASES]) *))
-  >- (say "fn" >>
-      simp[evaluate_def, pair_case_eq, result_case_eq,
-           known_def, bool_case_eq, case_eq_thms] >> rpt strip_tac >> rveq >> fs[] >>
-      rpt (pairarg_tac >> fs[]) >> rveq >> fs[] >>
-      imp_res_tac state_rel_max_app >> fs[] >>
-      dsimp[evaluate_def, case_eq_thms] >> imp_res_tac known_sing_EQ_E >> rveq >> fs[] >>
-      rveq >>
-      simp[exp_rel_def, PULL_EXISTS] >> metis_tac[kvrel_LIST_REL_val_approx])
-  >- (say "letrec" >>
-      simp[evaluate_def, pair_case_eq, result_case_eq, known_def, bool_case_eq,
-           case_eq_thms] >> rpt strip_tac >> rveq >> fs[letrec_case_eq] >>
-      rpt (pairarg_tac >> fs[]) >> rveq >> fs[] >>
-      fs[BAG_ALL_DISTINCT_BAG_UNION] >>
-      imp_res_tac state_rel_max_app >> fs[] >>
-      simp[evaluate_def, case_eq_thms, bool_case_eq] >> dsimp[] >>
-      simp[EVERY_MAP, EXISTS_MAP]
-      >- (disj1_tac >> simp[EVERY_MEM, FORALL_PROD] >>
-          imp_res_tac known_sing_EQ_E >> rveq >> fs[] >> rveq >>
-          sel_ihpc last >> simp[EVERY_GENLIST] >>
-          rpt (disch_then (resolve_selected last) >> simp[]) >>
-          rename1 `BAG_ALL_DISTINCT (elist_globals (MAP SND fns1))` >>
-          `∀n e. MEM (n,e) fns1 ⇒ n ≤ s02.max_app ∧ n ≠ 0`
-            by fs[EVERY_MEM, FORALL_PROD] >> simp[] >> strip_tac >>
-          simp[GSYM PULL_EXISTS] >> simp[Once EQ_SYM_EQ] >>
-          imp_res_tac LIST_REL_LENGTH >> fs[] >>
-          first_x_assum irule
-          >- (simp[LIST_REL_EL_EQN, EL_APPEND_EQN] >> qx_gen_tac `mm` >>
-              strip_tac >> rw[]
-              >- (fs[Once every_Fn_vs_NONE_EVERY] >>
-                  fs[EVERY_MAP] >> fs[EVERY_MEM, FORALL_PROD] >>
-                  metis_tac[])
-              >- (rename1 `LIST_REL val_approx_val apxs env1` >>
-                  qexists_tac `apxs` >> conj_tac
-                  >- metis_tac[kvrel_LIST_REL_val_approx] >>
-                  simp[LIST_REL_EL_EQN, EL_MAP] >>
-                  qx_gen_tac `nn` >> strip_tac >> pairarg_tac >>
-                  simp[] >> simp[exp_rel_def] >>
-                  map_every rename1 [`ksrel gg ss1 ss2`, `subspt g gg`,
-                                       `subspt g0 g`] >>
-                  ntac 2 (qexists_tac `g0`) >> simp[] >>
-                  rename1 `known [e1] env g0` >>
-                  Cases_on `known [e1] env g0` >>
-                  imp_res_tac known_sing_EQ_E >> fs[] >> rveq >>
-                  conj_tac >- metis_tac[subspt_trans] >>
-                  rename1 `known [subexp] env g0 = _` >>
-                  `elist_globals [subexp] = {||}`
-                    suffices_by metis_tac[known_emptySetGlobals_unchanged_g] >>
-                  fs[elglobals_EQ_EMPTY, MEM_MAP, PULL_EXISTS, FORALL_PROD] >>
-                  metis_tac[MEM_EL])
-              >- fs[LIST_REL_EL_EQN])
-          >- (irule EVERY2_APPEND_suff >> simp[] >>
-              simp[LIST_REL_GENLIST] >> qx_gen_tac `ii` >> strip_tac >>
-              rename1 `option_CASE lloc` >> Cases_on `lloc` >> simp[])) >>
-      disj2_tac >> fs[EXISTS_MEM, EXISTS_PROD] >> metis_tac[])
-  >- (say "app" >>
-      rpt gen_tac >> strip_tac >>
-      simp[evaluate_def, pair_case_eq, result_case_eq,
-           bool_case_eq, known_def, BAG_ALL_DISTINCT_BAG_UNION] >>
-      rpt strip_tac >> rveq >>
-      rpt (pairarg_tac >> fs[]) >> rveq >> fs[] >>
-      map_every imp_res_tac [known_sing_EQ_E, evaluate_SING] >> rveq >> fs[] >>
-      rveq
-      >- (map_every rename1 [
-            `known [fexp] apxs g1 = ([(fexp',fapx)], g)`,
-            `known args apxs g0 = (alist, g1)`,
-            `subspt g gg`] >>
-          patresolve `known [_] _ _ = _` (el 2) subspt_known_elist_globals >>
-          simp[] >> disch_then (resolve_selected (el 1)) >> simp[] >>
-          impl_tac >- fs[BAG_DISJOINT, DISJOINT_SYM] >> strip_tac >>
-          first_x_assum (patresolve `known args _ _ = _` last) >> simp[] >>
-          `subspt g1 gg` by metis_tac[subspt_trans] >>
-          rpt (disch_then (resolve_selected last) >> simp[]) >> rw[] >>
-          simp[evaluate_def] >> imp_res_tac known_LENGTH_EQ_E >> fs[] >>
-          first_x_assum (patresolve `known [_] _ _ = _` last) >> simp[] >>
-          disch_then (resolve_selected (el 2)) >> simp[] >>
-          disch_then (resolve_selected hd) >> simp[] >>
-          resolve_selected hd ssgc_evaluate >> simp[] >>
-          rpt (disch_then (resolve_selected hd) >> simp[]) >> strip_tac >>
-          impl_keep_tac
-          >- (patresolve `closSem$evaluate (MAP FST _, _, _) = _` last
-                         known_correct_approx >>
-              simp[] >> disch_then (resolve_selected hd) >> simp[] >>
-              metis_tac[ksrel_ssgc_free,kvrel_EVERY_vsgc_free,ksrel_sga,
-                        kvrel_LIST_REL_val_approx]) >>
-          rw[] >> simp[] >>
-          rename1 `evaluate_app loption1 v1 vs1 s21 = (result,ss1)` >>
-          `ssgc_free s21`
-            by metis_tac[ksrel_ssgc_free, ssgc_free_preserved_SING'] >> fs[] >>
-          first_x_assum (resolve_selected hd) >> simp[] >>
-          rpt (disch_then (resolve_selected hd) >> simp[]) >> strip_tac >>
-          `state_globals_approx s21 gg`
-            by (patresolve `known [_] _ _ = _` hd known_correct_approx >>
-                simp[] >> disch_then (resolve_selected last) >> simp[] >>
-                metis_tac[ksrel_ssgc_free,kvrel_EVERY_vsgc_free,ksrel_sga,
-                          kvrel_LIST_REL_val_approx]) >> fs[] >>
-          `vsgc_free v1`
-            by (patresolve `closSem$evaluate ([_],_,_) = (Rval [v1],_)` last
-                           ssgc_evaluate >> simp[]) >> fs[] >>
-          reverse (Cases_on `loption1`) >> simp[]
-          >- (first_x_assum irule >> simp[loptrel_def]) >>
-          rename1 `dest_Clos fapprox` >> Cases_on `dest_Clos fapprox` >>
-          simp[]
-          >- (first_x_assum irule >> simp[loptrel_def]) >>
-          rename1 `dest_Clos fapprox = SOME closapxvalue` >>
-          `∃clloc clarity. closapxvalue = (clloc, clarity)`
-            by metis_tac[pair_CASES] >> pop_assum SUBST_ALL_TAC >>
-          simp[] >> rename1 `LENGTH args > 0` >>
-          reverse (Cases_on `clarity = LENGTH args`) >> simp[]
-          >- (first_x_assum irule >> simp[loptrel_def]) >>
-          first_x_assum irule >> simp[loptrel_def] >>
-          qspecl_then [`[fexp]`, `apxs`, `g1`, `[(fexp',fapprox)]`, `g`]
-             mp_tac known_correct_approx >> simp[] >>
-          disch_then (resolve_selected last) >> simp[] >>
-          disch_then (qspec_then `gg` mp_tac) >> impl_tac
-          >- metis_tac[kvrel_LIST_REL_val_approx, ksrel_ssgc_free,
-                       kvrel_EVERY_vsgc_free, ksrel_sga] >>
-          fs[dest_Clos_eq_SOME] >> rveq >> rw[] >> simp[] >>
-          metis_tac[evaluate_length_imp])
-      >- (map_every rename1 [
-            `known [fexp] apxs g1 = ([(fexp',fapx)], g)`,
-            `known args apxs g0 = (alist, g1)`,
-            `subspt g gg`] >>
-          patresolve `known [_] _ _ = _` (el 2) subspt_known_elist_globals >>
-          simp[] >> disch_then (resolve_selected (el 1)) >> simp[] >>
-          impl_tac >- fs[BAG_DISJOINT, DISJOINT_SYM] >> strip_tac >>
-          first_x_assum (patresolve `known args _ _ = _` last) >> simp[] >>
-          `subspt g1 gg` by metis_tac[subspt_trans] >>
-          rpt (disch_then (resolve_selected last) >> simp[]) >> rw[] >>
-          simp[evaluate_def] >> imp_res_tac known_LENGTH_EQ_E >> fs[] >>
-          sel_ihpc last >> simp[] >>
-          disch_then (resolve_selected (el 2)) >> simp[] >>
-          disch_then (resolve_selected hd) >> simp[] >> reverse impl_tac
-          >- (rw[] >> simp[] >> fs[krrel_err_rw] >>
-              dsimp[result_case_eq] >> metis_tac[pair_CASES, result_CASES]) >>
-          conj_tac
-          >- (patresolve `closSem$evaluate (MAP FST _, _, _) = _` last
-                         known_correct_approx >>
-              simp[] >> disch_then (resolve_selected hd) >> simp[] >>
-              metis_tac[ksrel_ssgc_free,kvrel_EVERY_vsgc_free,ksrel_sga,
-                        kvrel_LIST_REL_val_approx]) >>
-          metis_tac [ssgc_evaluate])
-      >- (map_every rename1 [
-            `known [fexp] apxs g1 = ([(fexp',fapx)], g)`,
-            `known args apxs g0 = (alist, g1)`,
-            `subspt g gg`] >>
-          patresolve `known [_] _ _ = _` (el 2) subspt_known_elist_globals >>
-          simp[] >> disch_then (resolve_selected (el 1)) >> simp[] >>
-          impl_tac >- fs[BAG_DISJOINT, DISJOINT_SYM] >> strip_tac >>
-          first_x_assum (patresolve `known args _ _ = _` last) >> simp[] >>
-          `subspt g1 gg` by metis_tac[subspt_trans] >> strip_tac >>
-          nailIHx strip_assume_tac >>
-          simp[evaluate_def, bool_case_eq, result_case_eq, pair_case_eq] >>
-          imp_res_tac known_LENGTH_EQ_E >> rveq >> fs[] >>
-          fs[krrel_err_rw] >> dsimp[] >>
-          metis_tac[result_CASES,pair_CASES])
-      >- (map_every imp_res_tac [evaluate_IMP_LENGTH, known_LENGTH_EQ_E] >>
-          fs[] >> rw[] >> simp[evaluate_def]))
-  >- (say "tick" >> simp[dec_clock_def] >> rpt gen_tac >> strip_tac >>
-      simp[evaluate_def, bool_case_eq, known_def] >>
-      rename1 `(s0:('a,'b) closSem$state).clock = 0` >> Cases_on `s0.clock = 0` >>
-      fs[] >> rpt strip_tac >> rpt (pairarg_tac >> fs[]) >> rveq >> fs[] >>
-      simp[evaluate_def] >- fs[ksrel_def] >>
-      fs[dec_clock_def] >> fixeqs >> imp_res_tac known_sing_EQ_E >> rveq >>
-      fs[] >> rveq >>
-      map_every rename1 [
-        `known [exp1] apxs g0 = ([(exp2,apx)],g)`,
-        `evaluate([exp1],env1,s01 with clock := s01.clock - 1) = (res1,s1)`,
-        `ksrel gg s01 s02`] >>
-      sel_ihpc last >> simp[] >>
-      disch_then
-        (qspecl_then [`env2`, `s02 with clock := s02.clock - 1`, `gg`]
-                     mp_tac) >>
-      simp[] >> impl_keep_tac >- fs[ksrel_def] >>
-      `s02.clock = s01.clock` by fs[ksrel_def] >> simp[])
-  >- (say "call" >>
-      simp[evaluate_def, pair_case_eq, result_case_eq, case_eq_thms, bool_case_eq,
-           known_def] >> rw[]
-      >- (simp[] >> metis_tac[pair_CASES])
-      >- (rpt (pairarg_tac >> fs[]) >> rveq >> nailIHx strip_assume_tac >>
-          simp[evaluate_def] >> rw[] >>
-          imp_res_tac ksrel_find_code >> fs[])
-      >- (fixeqs >> rpt (pairarg_tac >> fs[]) >> rveq >> fs[] >>
-          nailIHx strip_assume_tac >>
-          imp_res_tac ksrel_find_code >> fs[])
-      >- (rpt (pairarg_tac >> fs[]) >> rveq >> fs[] >>
-          nailIHx strip_assume_tac >> simp[evaluate_def] >>
-          fs[krrel_err_rw] >>
-          dsimp[result_case_eq, case_eq_thms, pair_case_eq, bool_case_eq] >>
-          metis_tac[option_CASES, pair_CASES, result_CASES]))
-  >- (say "evaluate_app(nil)" >> simp[evaluate_def])
-  >- (say "evaluate_app(cons)" >> rpt gen_tac >> strip_tac >>
-      simp[evaluate_def, case_eq_thms, bool_case_eq, pair_case_eq, result_case_eq] >>
-      rpt strip_tac >> rveq >> fs[]
-      >- metis_tac[pair_CASES]
-      >- (simp[evaluate_def, case_eq_thms, bool_case_eq, pair_case_eq] >>
-          resolve_selected hd (GEN_ALL kvrel_dest_closure_SOME_Partial) >>
-          simp[PULL_EXISTS] >> imp_res_tac LIST_REL_LENGTH >> fs[] >>
-          rpt (disch_then (resolve_selected hd) >> simp[]) >>
-          strip_tac >> simp[] >> fs[ksrel_def])
-      >- (simp[evaluate_def, case_eq_thms, bool_case_eq, pair_case_eq] >>
-          resolve_selected hd (GEN_ALL kvrel_dest_closure_SOME_Partial) >>
-          simp[PULL_EXISTS] >> imp_res_tac LIST_REL_LENGTH >> fs[] >>
-          rpt (disch_then (resolve_selected hd) >> simp[]) >> strip_tac >>
-          simp[] >> fs[ksrel_def, dec_clock_def])
-      >- (simp[evaluate_def, case_eq_thms, bool_case_eq, pair_case_eq] >>
-          resolve_selected hd (GEN_ALL kvrel_dest_closure_SOME_Full) >>
-          simp[PULL_EXISTS] >> imp_res_tac LIST_REL_LENGTH >> fs[] >>
-          rpt (disch_then (resolve_selected hd) >> simp[]) >> strip_tac >>
-          simp[] >> imp_res_tac LIST_REL_LENGTH >> fs[ksrel_def])
-      >- (simp[evaluate_def, case_eq_thms, bool_case_eq, pair_case_eq] >>
-          resolve_selected hd (GEN_ALL kvrel_dest_closure_SOME_Full) >>
-          simp[PULL_EXISTS] >> imp_res_tac LIST_REL_LENGTH >> fs[] >>
-          rpt (disch_then (resolve_selected hd) >> simp[]) >> strip_tac >>
-          simp[] >> rename1 `ksrel g s01 s02` >>
-          `s02.clock = s01.clock` by fs[ksrel_def] >>
-          `s02.max_app = s01.max_app` by fs[ksrel_def] >>
-          imp_res_tac LIST_REL_LENGTH >> fs[] >> simp[PULL_EXISTS] >>
-          dsimp[] >> fs[PULL_EXISTS] >>
-          map_every rename1 [
-            `dest_closure _ lopt1 f1 (iarg1 :: iargs) =
-               SOME (Full_app exp1 env1 args1)`,
-            `evaluate([exp1],env1,dec_clock _ s01) = (Rval [v1], s11)`,
-            `kerel envapx gg exp1 exp2`] >> fs[exp_rel_def] >>
-          rpt disj1_tac >>
-          first_x_assum (patresolve `known [exp1] _ _ = _` last) >> simp[] >>
-          map_every rename1 [
-            `evaluate([exp1],env1,
-                      dec_clock (SUC (LENGTH iargs1) - LENGTH args2) s01)`,
-            `LIST_REL (kvrel gg) env1 env2`] >>
-          disch_then (qspecl_then [
-             `env2`,
-             `dec_clock (SUC (LENGTH iargs1) - LENGTH args2) s02`,
-             `gg`] mp_tac) >> simp[] >>
-          `set_globals exp1 = {||} ∧ EVERY vsgc_free env1 ∧
-           EVERY vsgc_free args1 ∧ esgc_free exp1`
-            by metis_tac[vsgc_free_Full_app_set_globals, EVERY_DEF,
-                         set_globals_empty_esgc_free] >> simp[] >>
-          qspec_then `[exp1]` mp_tac known_emptySetGlobals_unchanged_g >>
-          disch_then (resolve_selected hd) >> simp[] >>
-          disch_then SUBST_ALL_TAC >>
-          rename1 `LIST_REL val_approx_val envapx env1` >>
-          `LIST_REL val_approx_val envapx env1`
-            by metis_tac[kvrel_LIST_REL_val_approx] >>
-          `every_Fn_vs_NONE [exp1]`
-            by metis_tac[kvrel_dest_closure_every_Fn_vs_NONE] >>
-          impl_tac >- (simp[] >> fs[ksrel_def, dec_clock_def]) >> rw[] >>
-          simp[] >>
-          rename1 `loptrel f2 _ lopt1 lopt2` >>
-          reverse (Cases_on `lopt1`)
-          >- (fs[loptrel_arg1_SOME] >> rveq >>
-              imp_res_tac dest_closure_SOME_Full_app_args_nil >> fs[] >>
-              rveq >> simp[]) >>
-          qpat_x_assum `loptrel _ _ _ _` mp_tac >>
-          simp[loptrel_arg1_NONE] >> reverse strip_tac >> rveq
-          >- (imp_res_tac dest_closure_SOME_Full_app_args_nil >> fs[] >>
-              rveq >> simp[])
-          >- (imp_res_tac dest_closure_SOME_Full_app_args_nil >> fs[] >>
-              rveq >> simp[]) >>
-          first_x_assum irule >> simp[]
-          >- metis_tac[ssgc_free_preserved_SING', ssgc_free_dec_clock]
-          >- (patresolve `evaluate([exp1],_,_) = _` last ssgc_evaluate >>
-              simp[])
-          >- (patresolve `known [exp1] _ _ = _` hd known_correct_approx >>
-              simp[] >> disch_then (resolve_selected last) >> simp[] >>
-              metis_tac[ksrel_sga, ksrel_ssgc_free, kvrel_EVERY_vsgc_free])
-          >- simp[loptrel_def])
-      >- (imp_res_tac evaluate_SING >> fs[])
-      >- (simp[evaluate_def, case_eq_thms, bool_case_eq, pair_case_eq] >>
-          resolve_selected hd (GEN_ALL kvrel_dest_closure_SOME_Full) >>
-          simp[PULL_EXISTS] >> imp_res_tac LIST_REL_LENGTH >> fs[] >>
-          rpt (disch_then (resolve_selected hd) >> simp[]) >> strip_tac >>
-          simp[] >> rename1 `ksrel g s01 s02` >>
-          `s02.clock = s01.clock` by fs[ksrel_def] >>
-          imp_res_tac LIST_REL_LENGTH >> fs[] >> simp[PULL_EXISTS] >>
-          dsimp[] >>
-          map_every rename1 [
-            `dest_closure _ lopt1 f1 (iarg1 :: iargs) =
-               SOME (Full_app exp1 env1 args1)`,
-            `evaluate([exp1],env1,dec_clock _ s01) = (Rerr err1, s1)`,
-            `kerel envapx gg exp1 exp2`] >> fs[exp_rel_def] >>
-          first_x_assum (patresolve `known [exp1] _ _ = _` last) >> simp[] >>             map_every rename1 [
-            `evaluate([exp1],env1,
-                      dec_clock (SUC (LENGTH iargs1) - LENGTH args2) s01)`,
-            `LIST_REL (kvrel gg) env1 env2`] >>
-          disch_then (qspecl_then [
-             `env2`,
-             `dec_clock (SUC (LENGTH iargs1) - LENGTH args2) s02`,
-             `gg`] mp_tac) >> simp[] >>
-          `set_globals exp1 = {||} ∧ EVERY vsgc_free env1 ∧
-           EVERY vsgc_free args1 ∧ esgc_free exp1`
-            by metis_tac[vsgc_free_Full_app_set_globals, EVERY_DEF,
-                         set_globals_empty_esgc_free] >> simp[] >>
-          qspec_then `[exp1]` mp_tac known_emptySetGlobals_unchanged_g >>
-          disch_then (resolve_selected hd) >> simp[] >>
-          disch_then SUBST_ALL_TAC >>
-          rename1 `LIST_REL val_approx_val envapx env1` >>
-          `LIST_REL val_approx_val envapx env1`
-            by metis_tac[kvrel_LIST_REL_val_approx] >>
-          `every_Fn_vs_NONE [exp1]`
-            by metis_tac[kvrel_dest_closure_every_Fn_vs_NONE] >>
-          impl_tac >- (simp[] >> fs[ksrel_def, dec_clock_def]) >> rw[] >>
-          imp_res_tac state_rel_max_app >>
-          simp[] >> fs[krrel_err_rw] >>
-          rename1 `evaluate([exp2],_,_) = (res2,_)` >>
-          Cases_on `res2`
-          >- (imp_res_tac evaluate_SING >> simp[] >> metis_tac[pair_CASES]) >>
-          simp[])))
-
-
-
-
-
-(*******************************************************)
-
-
-(* TODO: MOVE candidates *)
-fun sel_ihpc f = first_x_assum (first_assum o mp_then (Pos f) mp_tac)
-fun resolve_selected f th = first_assum (mp_then (Pos f) mp_tac th)
-
-fun patresolve p f th = Q.PAT_ASSUM p (mp_then (Pos f) mp_tac th)
-
-(* repeated resolution, requiring that all preconditions get removed *)
-fun nailIHx k =
-  first_x_assum
-    (REPEAT_GTCL
-       (fn ttcl => fn th => first_assum (mp_then (Pos hd) ttcl th))
-       (k o assert (not o is_imp o #2 o strip_forall o concl)) o
-     assert (is_imp o #2 o strip_forall o concl))
-
-infix >~
-fun (f >~ g) th = f th >> g
-
-(* TODO: MOVE-HOL candidate; unused here *)
-val union_idem = Q.store_thm(
-  "union_idem[simp]",
-  `∀spt. union spt spt = spt`,
-  Induct >> simp[union_def]);
-
-val FINITE_BAG_FOLDR = Q.store_thm(
-  "FINITE_BAG_FOLDR",
-  `∀l f a.
-     FINITE_BAG a ∧ (∀e a. FINITE_BAG a ∧ MEM e l ⇒ FINITE_BAG (f e a)) ⇒
-     FINITE_BAG (FOLDR f a l)`,
-  Induct >> simp[]);
-
-val FINITE_set_globals = Q.store_thm(
-  "FINITE_set_globals[simp]",
-  `(∀e. FINITE_BAG (set_globals e)) ∧ ∀es. FINITE_BAG (elist_globals es)`,
-  ho_match_mp_tac set_globals_ind >> simp[] >> rpt strip_tac >>
-  rename1 `op_gbag opn` >> Cases_on `opn` >> simp[op_gbag_def]);
-
-val state_approx_better_definedg = Q.store_thm(
-  "state_approx_better_definedg",
-  `better_definedg g1 g2 ∧ state_globals_approx s g1 ⇒
-   state_globals_approx s g2`,
-  csimp[better_definedg_def, state_globals_approx_def, domain_lookup,
-        PULL_EXISTS] >>
-  metis_tac[val_approx_better_approx]);
-
-val evaluate_t = ``closSem$evaluate``
-val fixeqs = let
-  fun c t =
-    let
-      val r = rhs t
-      val (f, _) = strip_comb r
-    in
-      if same_const evaluate_t f then REWR_CONV EQ_SYM_EQ
-      else NO_CONV
-    end t
-in
-  RULE_ASSUM_TAC (CONV_RULE (TRY_CONV c))
-end
-
-
-
-
-val lem = Q.prove(
-  `(∀a es env (s0:('a,'b) closSem$state) res s.
-      a = (es,env,s0) ∧ evaluate(es,env,s0) = (res,s) ⇒
-      mapped_globals s0 ⊆ mapped_globals s) ∧
-   (∀lopt f args (s0:('a,'b) closSem$state) res s.
-      evaluate_app lopt f args s0 = (res, s) ⇒
-      mapped_globals s0 ⊆ mapped_globals s)`,
-  ho_match_mp_tac evaluate_ind >> rw[evaluate_def]
-  >- fs[evaluate_def]
-  >- (fs[pair_case_eq, result_case_eq] >> rveq >> fs[] >>
-      metis_tac[SUBSET_TRANS])
-  >- fs[evaluate_def, bool_case_eq]
-  >- (fs[pair_case_eq, result_case_eq, bool_case_eq] >> rveq >> fixeqs >>
-      fs[] >> metis_tac[SUBSET_TRANS])
-  >- (fs[pair_case_eq, result_case_eq] >> rveq >> fs[] >>
-      metis_tac[SUBSET_TRANS])
-  >- fs[result_case_eq, pair_case_eq]
-  >- (fs[result_case_eq, pair_case_eq, error_case_eq] >> rveq >> fs[] >>
-      metis_tac[SUBSET_TRANS])
-  >- (fs[pair_case_eq, result_case_eq] >> rveq >> fs[] >>
-      rename1 `closSem$do_app opn` >>
-      Cases_on `opn = Install` THEN1
-       (rveq \\ fs []
-        \\ reverse (Cases_on `do_install (REVERSE vs) s''`) \\ fs []
-        \\ reverse (Cases_on `q`) \\ fs []
-        THEN1 (Cases_on `e` \\ rveq \\ fs []
-               \\ imp_res_tac do_install_not_Rraise \\ fs []
-               \\ fs [do_install_def]
-               \\ fs [case_eq_thms] \\ rveq \\ fs []
-               \\ pairarg_tac \\ fs []
-               \\ fs [case_eq_thms,bool_case_eq,pair_case_eq]
-               \\ fs [case_eq_thms] \\ rveq \\ fs []
-               \\ fs [mapped_globals_def])
-        \\ pop_assum mp_tac
-        \\ fs [do_install_def]
-        \\ fs [case_eq_thms]
-        \\ strip_tac \\ pairarg_tac \\ fs []
-        \\ fs [case_eq_thms,bool_case_eq,pair_case_eq]
-        \\ rveq \\ fs []
-        \\ fs [mapped_globals_def]
-        \\ match_mp_tac SUBSET_TRANS \\ asm_exists_tac \\ fs []) >>
-      Cases_on `opn` >>
-      fs[do_app_def, case_eq_thms, bool_case_eq, pair_case_eq] >> rw[] >>
-      fs[]
-      >- (rename1 `closSem$evaluate(_,_,s0) = (_, s1)` >>
-          irule SUBSET_TRANS >> qexists_tac `mapped_globals s1` >> simp[] >>
-          simp[mapped_globals_def] >>
-          fs[SUBSET_DEF, PULL_EXISTS, get_global_def,
-             EL_LUPDATE, bool_case_eq] >> metis_tac[])
-      >- (simp[mapped_globals_def, SUBSET_DEF, get_global_def,
-               EL_APPEND_EQN, bool_case_eq] >> rpt strip_tac >>
-          simp[]))
-  >- fs[evaluate_def, bool_case_eq, case_eq_thms]
-  >- (fs[case_eq_thms, PULL_EXISTS] >> rveq >> fs[])
-  >- (fs[pair_case_eq, result_case_eq] >> rveq >> fs[] >>
-      metis_tac[SUBSET_TRANS])
-  >- (fs[pair_case_eq, result_case_eq, case_eq_thms, bool_case_eq] >> rveq >> fixeqs >>
-      fs[] >> metis_tac[SUBSET_TRANS])
-  >- (fs[case_eq_thms, bool_case_eq, pair_case_eq] >> rveq >> fs[] >>
-      metis_tac[SUBSET_TRANS]));
-
-val mapped_globals_grow = save_thm(
-  "mapped_globals_grow",
-  lem |> CONJUNCT1 |> SIMP_RULE bool_ss [])
-
-fun say0 pfx s g = (print (pfx ^ ": " ^ s ^ "\n"); ALL_TAC g)
-val say = say0 "ssgc_evaluate0"
-
-val ssgc_free_preserved_SING = Q.store_thm(
-  "ssgc_free_preserved_SING",
-  `known [e1] as g0 = ([(e1',a)], g) ∧ esgc_free e1 ∧ ssgc_free s0 ∧
-   EVERY vsgc_free env ∧ evaluate([e1'],env,s0) = (res,s) ⇒ ssgc_free s`,
-  rpt strip_tac >>
-  `EVERY esgc_free [e1]` by simp[] >>
-  `EVERY (esgc_free o FST) [(e1',a)]`
-     by metis_tac[known_preserves_esgc_free] >>
-  `EVERY esgc_free [e1']` by fs[] >>
-  metis_tac[ssgc_evaluate]);
-
-val LENGTH_clos_gen = Q.prove(`
-  ∀ls x c.
-  LENGTH (clos_gen x c ls) = LENGTH ls`,
-  Induct>>fs[FORALL_PROD,clos_gen_def])
-
-val clos_gen_eq = Q.prove(`
-  ∀n c fns.
-  clos_gen n c fns =
-  GENLIST (λi. Clos (2* (i+c) +n ) (FST (EL i fns))) (LENGTH fns)`,
-  Induct_on`fns`>>fs[FORALL_PROD,clos_gen_def,GENLIST_CONS]>>rw[]>>
-  simp[o_DEF,ADD1])
-
-val letrec_case_eq = Q.prove(`
-  (case loc of
-    NONE => REPLICATE (LENGTH fns) Other
-  | SOME n => clos_gen n 0 fns) =
-  GENLIST (case loc of NONE => K Other | SOME n => λi. Clos (n+ 2*i) (FST (EL i fns))) (LENGTH fns)`,
-  Cases_on`loc`>>fs[clos_gen_eq,REPLICATE_GENLIST])
-
-val kca_sing_sga =
-    known_correct_approx
-      |> Q.SPECL [`[e]`, `as`, `g0`, `[(e',a)]`, `g`]
-      |> SIMP_RULE (srw_ss()) [PULL_FORALL]
-      |> SPEC_ALL |> UNDISCH_ALL |> CONJUNCT1 |> DISCH_ALL
-
-val ssgc_free_preserved_SING' = Q.store_thm(
-  "ssgc_free_preserved_SING'",
-  `esgc_free e1 ∧ ssgc_free s0 ∧
-   EVERY vsgc_free env ∧ evaluate([e1],env,s0) = (res,s) ⇒ ssgc_free s`,
-  rpt strip_tac >>
-  `EVERY esgc_free [e1]` by simp[] >>
-  metis_tac[ssgc_evaluate]);
-
-val say = say0 "known_correct";
-
-val exp_rel_def = Define`
-  exp_rel as g' e1 e2 ⇔
-    ∃g0 g apx. subspt g g' ∧ known [e1] as g0 = ([(e2,apx)], g)
-`;
-val _ = temp_overload_on ("kerel", ``clos_knownProof$exp_rel``)
-
-val val_rel_def = tDefine "val_rel" `
-  (val_rel g (Number i) v ⇔ v = Number i) ∧
-  (val_rel g (Word64 w) v ⇔ v = Word64 w) ∧
-  (val_rel g (Block n vs) v ⇔
-     ∃vs'. v = Block n vs' ∧ LIST_REL (val_rel g) vs vs') ∧
-  (val_rel g (ByteVector ws) v ⇔ v = ByteVector ws) ∧
-  (val_rel g (RefPtr n) v ⇔ v = RefPtr n) ∧
-  (val_rel g (Closure lopt vs1 env1 n bod1) v ⇔
-     every_Fn_vs_NONE [bod1] ∧
-     ∃vs2 env2 bod2 eapx.
-       LIST_REL (val_rel g) vs1 vs2 ∧ LIST_REL (val_rel g) env1 env2 ∧
-       LIST_REL val_approx_val eapx env2 ∧
-       kerel (REPLICATE n Other ++ eapx) g bod1 bod2 ∧
-       v = Closure lopt vs2 env2 n bod2) ∧
-  (val_rel g (Recclosure lopt vs1 env1 fns1 i) v ⇔
-     EVERY (λ(n,e). every_Fn_vs_NONE [e]) fns1 ∧
-     let gfn = case lopt of
-                 | NONE => K Other
-                 | SOME n => (λi. Clos (n + 2*i) (FST (EL i fns1))) in
-     let clos = GENLIST gfn (LENGTH fns1)
-     in
-       ∃vs2 env2 fns2 eapx.
-         LIST_REL (val_rel g) vs1 vs2 ∧ LIST_REL (val_rel g) env1 env2 ∧
-         LIST_REL val_approx_val eapx env2 ∧
-         LIST_REL (λ(n1,e1) (n2,e2).
-                     n1 = n2 ∧
-                     kerel (REPLICATE n1 Other ++ clos ++ eapx) g e1 e2)
-                  fns1 fns2 ∧
-         v = Recclosure lopt vs2 env2 fns2 i)
-` (WF_REL_TAC `measure (v_size o FST o SND)` >> simp[v_size_def] >>
-   rpt strip_tac >> imp_res_tac v_size_lemma >> simp[])
-val val_rel_ind = theorem "val_rel_ind"
-val val_rel_def = save_thm(
-  "val_rel_def[simp]",
-  SIMP_RULE (bool_ss ++ ETA_ss) [] val_rel_def)
-
-val _ = temp_overload_on ("kvrel", ``clos_knownProof$val_rel``)
-
-(* necessary kvrel *)
-val kvrel_vsgc_free = Q.store_thm(
-  "kvrel_vsgc_free",
-  `∀g v1 v2. kvrel g v1 v2 ⇒ (vsgc_free v1 ⇔ vsgc_free v2)`,
-  ho_match_mp_tac val_rel_ind >> simp[] >> rpt strip_tac
-  >- (fs[EVERY_MEM, LIST_REL_EL_EQN] >> metis_tac[MEM_EL])
-  >- (fs[EVERY_MEM, LIST_REL_EL_EQN] >>
-      fs[exp_rel_def] >> imp_res_tac known_preserves_setGlobals >>
-      fs[] >> metis_tac[MEM_EL])
-  >- (fs[EVERY_MEM, LIST_REL_EL_EQN, elglobals_EQ_EMPTY, MEM_MAP, PULL_EXISTS,
-         FORALL_PROD]>>
-      EQ_TAC >> rpt strip_tac
-      >- (imp_res_tac (MEM_EL |> SPEC_ALL |> EQ_IMP_RULE |> #1 |> GSYM) >>
-          rename1 `m < LENGTH fns2` >>
-          Cases_on `EL m fns1` >> fs[] >>
-          first_x_assum (qspec_then `m` mp_tac) >> simp[] >>
-          rw[exp_rel_def] >>
-          imp_res_tac known_preserves_setGlobals >> fs[] >>
-          metis_tac[MEM_EL])
-      >- metis_tac[MEM_EL]
-      >- metis_tac[MEM_EL]
-      >- (imp_res_tac (MEM_EL |> SPEC_ALL |> EQ_IMP_RULE |> #1 |> GSYM) >>
-          rename1 `m < LENGTH fns1` >>
-          Cases_on `EL m fns2` >> fs[] >>
-          first_x_assum (qspec_then `m` mp_tac) >> simp[] >>
-          rw[exp_rel_def] >>
-          imp_res_tac known_preserves_setGlobals >> fs[] >>
-          metis_tac[MEM_EL])
-      >- metis_tac[MEM_EL]
-      >- metis_tac[MEM_EL]))
-
-val kvrel_Boolv = Q.store_thm(
-  "kvrel_Boolv[simp]",
-  `(kvrel g (Boolv b) v ⇔ v = Boolv b) ∧
-   (kvrel g v (Boolv b) ⇔ v = Boolv b)`,
-  simp[closSemTheory.Boolv_def] >> Cases_on `v` >> simp[] >> metis_tac[]);
-
-val kvrel_Unit = Q.store_thm(
-  "kvrel_Unit[simp]",
-  `(kvrel g Unit v ⇔ v = Unit) ∧ (kvrel g v Unit ⇔ v = Unit)`,
-  simp[Unit_def] >> Cases_on `v` >> simp[] >> metis_tac[])
-
-val kvrel_EVERY_vsgc_free = Q.store_thm(
-  "kvrel_EVERY_vsgc_free",
-  `∀vs1 vs2.
-     LIST_REL (kvrel g) vs1 vs2 ⇒
-     (EVERY vsgc_free vs1 ⇔ EVERY vsgc_free vs2)`,
-  Induct_on `LIST_REL` >> simp[] >> metis_tac[kvrel_vsgc_free]);
-
-(* necessary kvrel *)
-val kvrel_val_approx = Q.store_thm(
-  "kvrel_val_approx",
-  `∀g v1 v2.
-     kvrel g v1 v2 ⇒ ∀a. val_approx_val a v1 ⇔ val_approx_val a v2`,
-  ho_match_mp_tac val_rel_ind >> rw[]
-  >- (Cases_on `a` >> simp[] >> fs[LIST_REL_EL_EQN] >> metis_tac[MEM_EL])
-  >- (Cases_on `a` >> simp[] >> fs[LIST_REL_EL_EQN] >> metis_tac[LENGTH_NIL])
-  >- (Cases_on `a` >> fs[LIST_REL_EL_EQN] >> rename1 `lopt = SOME _` >>
-      Cases_on `lopt` >> simp[] >> rename1 `EL j` >>
-      rename1 `j < LENGTH fns2` >> Cases_on `j < LENGTH fns2` >> simp[] >>
-      rename1 `vvs = []` >> reverse (Cases_on `vvs`)
-      >- (simp[] >> rename1 `vvs' = []` >> Cases_on `vvs'` >> fs[]) >>
-      fs[LENGTH_NIL, LENGTH_NIL_SYM] >> rfs[] >> res_tac >>
-      fs[UNCURRY]))
-
-val kvrel_LIST_REL_val_approx = Q.store_thm(
-  "kvrel_LIST_REL_val_approx",
-  `∀vs1 vs2.
-      LIST_REL (kvrel g) vs1 vs2 ⇒
-      ∀as. LIST_REL val_approx_val as vs1 ⇔ LIST_REL val_approx_val as vs2`,
-  Induct_on `LIST_REL` >> simp[] >> metis_tac[kvrel_val_approx]);
-
-val state_rel_def = Define`
-  state_rel g (s1:('a,'b) closSem$state) (s2:('a,'b) closSem$state) ⇔
-     s2.clock = s1.clock ∧ s2.ffi = s1.ffi ∧ s2.max_app = s1.max_app ∧
-     LIST_REL (OPTREL (kvrel g)) s1.globals s2.globals ∧
-     fmap_rel (ref_rel (kvrel g)) s1.refs s2.refs ∧
-     s1.code = FEMPTY ∧ s2.code = FEMPTY
-`;
-val _ = temp_overload_on ("ksrel", ``clos_knownProof$state_rel``)
-val ksrel_def = state_rel_def
-
-val state_rel_max_app = Q.store_thm("state_rel_max_app",
-  `state_rel g s1 s2 ⇒ s1.max_app = s2.max_app`,
-  rw[state_rel_def]);
-
-val ksrel_flookup_refs = Q.store_thm("ksrel_flookup_refs",
-  `ksrel g s1 s2 ∧ FLOOKUP s1.refs k = SOME v ⇒
-   ∃v'. FLOOKUP s2.refs k = SOME v' ∧ ref_rel (kvrel g) v v'`,
-  rw[ksrel_def,fmap_rel_OPTREL_FLOOKUP,OPTREL_def]
-  \\  first_x_assum(qspec_then`k`mp_tac) \\ rw[]);
-
-(* ksrel necessary *)
-val ksrel_sga = Q.store_thm(
-  "ksrel_sga",
-  `ksrel g0 s1 s2 ⇒ (state_globals_approx s1 g ⇔ state_globals_approx s2 g)`,
-  simp[ksrel_def, state_globals_approx_def, get_global_def, LIST_REL_EL_EQN] >>
-  csimp[] >> rpt strip_tac >> eq_tac >> rpt strip_tac >>
-  rename1 `EL kk (ss:('a,'b) closSem$state).globals = SOME vv` >>
-  rename1 `lookup kk gg` >>
-  nailIHx mp_tac >>
-  simp[optionTheory.OPTREL_def] >>
-  metis_tac [kvrel_val_approx])
-
-(* ksrel necessary *)
-val ksrel_ssgc_free = Q.store_thm(
-  "ksrel_ssgc_free",
-  `ksrel g s1 s2 ⇒ (ssgc_free s1 ⇔ ssgc_free s2)`,
-  simp[ksrel_def, ssgc_free_def] >> rpt strip_tac >> eq_tac >> rpt strip_tac >>
-  fs[fmap_rel_OPTREL_FLOOKUP]
-  >- (rename1 `FLOOKUP s2.refs kk = SOME (ValueArray vvl)` >>
-      `OPTREL (ref_rel (kvrel g)) (FLOOKUP s1.refs kk) (FLOOKUP s2.refs kk)`
-         by simp[] >> pop_assum mp_tac >>
-      simp_tac(srw_ss()) [OPTREL_def] >> simp[PULL_EXISTS] >> Cases >>
-      simp[] >> metis_tac[kvrel_EVERY_vsgc_free])
-  >- (fs[LIST_REL_EL_EQN] >>
-      imp_res_tac (MEM_EL |> SPEC_ALL |> EQ_IMP_RULE |> #1 |> GSYM) >>
-      rename1 `EL kk s2.globals` >>
-      `OPTREL (kvrel g) (EL kk s1.globals) (EL kk s2.globals)` by simp[] >>
-      pop_assum mp_tac >> simp_tac(srw_ss()) [OPTREL_def] >> simp[] >>
-      metis_tac[kvrel_vsgc_free, MEM_EL])
-  >- (rename1 `FLOOKUP s1.refs kk = SOME (ValueArray vvl)` >>
-      `OPTREL (ref_rel (kvrel g)) (FLOOKUP s1.refs kk) (FLOOKUP s2.refs kk)`
-         by simp[] >> pop_assum mp_tac >>
-      simp_tac(srw_ss()) [OPTREL_def] >> simp[PULL_EXISTS] >>
-      metis_tac[kvrel_EVERY_vsgc_free])
-  >- (fs[LIST_REL_EL_EQN] >>
-      imp_res_tac (MEM_EL |> SPEC_ALL |> EQ_IMP_RULE |> #1 |> GSYM) >>
-      rename1 `EL kk s1.globals` >>
-      `OPTREL (kvrel g) (EL kk s1.globals) (EL kk s2.globals)` by simp[] >>
-      pop_assum mp_tac >> simp_tac(srw_ss()) [OPTREL_def] >> simp[] >>
-      metis_tac[kvrel_vsgc_free, MEM_EL]))
-
-val res_rel_def = Define`
-  (res_rel g (Rval vs1, s1) r ⇔
-      ∃s2 vs2. r = (Rval vs2,s2) ∧ LIST_REL (kvrel g) vs1 vs2 ∧ ksrel g s1 s2) ∧
-  (res_rel g (Rerr (Rabort Rtype_error), _) _ ⇔ T) ∧
-  (res_rel g (Rerr (Rabort Rtimeout_error), s1) (Rerr e, s2) ⇔
-     e = Rabort Rtimeout_error ∧ ksrel g s1 s2) ∧
-  (res_rel g (Rerr (Rraise v1), s1) (Rerr (Rraise v2), s2) ⇔
-     kvrel g v1 v2 ∧ ksrel g s1 s2) ∧
-  (res_rel _ _ _ ⇔ F)
-`;
-val _ = export_rewrites ["res_rel_def"]
-val _ = temp_overload_on ("krrel", ``clos_knownProof$res_rel``)
-val krrel_def = res_rel_def
-
-val krrel_errval = Q.store_thm(
-  "krrel_errval[simp]",
-  `(krrel g (Rerr e, s1) (Rval vs, s2) ⇔ e = Rabort Rtype_error)`,
-  Cases_on `e` >> simp[] >> rename1 `Rabort a` >> Cases_on `a` >> simp[]);
-
-val krrel_err_rw = Q.store_thm(
-  "krrel_err_rw",
-  `krrel g (Rerr e, s1) r ⇔
-      e = Rabort Rtype_error ∨
-      (∃s2. e = Rabort Rtimeout_error ∧ r = (Rerr (Rabort Rtimeout_error), s2) ∧
-            ksrel g s1 s2) ∨
-      (∃v1 v2 s2.
-            e = Rraise v1 ∧ r = (Rerr (Rraise v2),s2) ∧ kvrel g v1 v2 ∧
-            ksrel g s1 s2)`,
-  Cases_on `e` >> simp[] >> Cases_on `r` >> simp[]
-  >- (rename1 `krrel _ _ (r2, s2)` >> Cases_on `r2` >> simp[] >>
-      rename1 `krrel _ _ (Rerr e,_)` >> Cases_on `e` >> simp[])
-  >- (rename1 `Rabort abt` >> Cases_on `abt` >> simp[] >>
-      rename1 `krrel _ _ (r2,s2)` >> Cases_on `r2` >> simp[]));
-
-val krrel_ffi = Q.store_thm(
-  "krrel_ffi",
-  `krrel gmap (r1,s1) (r2,s2) ∧ r1 ≠ Rerr (Rabort Rtype_error) ⇒
-   s2.ffi = s1.ffi`,
-  Cases_on `r1` >> Cases_on`r2` >>
-  simp[krrel_def, ksrel_def, krrel_err_rw, ksrel_def] >> rw[])
-
-val krrel_arg2_typeerror = Q.store_thm(
-  "krrel_arg2_typeerror[simp]",
-  `krrel g (res1, s1) (Rerr (Rabort Rtype_error), s2) ⇔
-    res1 = Rerr (Rabort Rtype_error)`,
-  Cases_on `res1` >> simp[krrel_def, krrel_err_rw]);
-
-(* necesssary kvrel *)
-val kvrel_v_to_list = Q.store_thm(
-  "kvrel_v_to_list",
-  `∀g v1 v2 l1.
-     kvrel g v1 v2 ∧ v_to_list v1 = SOME l1 ⇒
-     ∃l2. v_to_list v2 = SOME l2 ∧ LIST_REL (kvrel g) l1 l2`,
-  ho_match_mp_tac val_rel_ind >> simp[v_to_list_def, PULL_EXISTS] >>
-  rpt strip_tac >> rename1 `v_to_list (closSem$Block _ vs2)` >>
-  Cases_on `vs2` >> fs[v_to_list_def] >> rw[] >> fs[v_to_list_def] >>
-  rename1 `v_to_list (closSem$Block _ (_ :: vs2'))` >>
-  Cases_on `vs2'` >> fs[v_to_list_def] >> rw[] >> fs[v_to_list_def] >>
-  rename1 `v_to_list (closSem$Block _ (_ :: _ :: vs2''))` >>
-  Cases_on `vs2''` >> fs[v_to_list_def] >> rw[] >> fs[v_to_list_def] >>
-  fs[case_eq_thms] >> rveq >> simp[PULL_EXISTS] >> metis_tac[MEM]);
-
-val kvrel_do_eq0 = Q.prove(
-  `(∀u1 v1 u2 v2 b g.
-      kvrel g u1 u2 ∧ kvrel g v1 v2 ∧ do_eq u1 v1 = Eq_val b ⇒
-      do_eq u2 v2 = Eq_val b) ∧
-   (∀us1 vs1 us2 vs2 b g.
-      LIST_REL (kvrel g) us1 us2 ∧ LIST_REL (kvrel g) vs1 vs2 ∧
-      do_eq_list us1 vs1 = Eq_val b ⇒
-      do_eq_list us2 vs2 = Eq_val b)`,
-  ho_match_mp_tac do_eq_ind >> rpt conj_tac
-  >- (Cases >> Cases >> strip_tac >>
-      simp[SimpL ``$==>``, do_eq_def, v_case_eq, bool_case_eq, PULL_EXISTS] >>
-      fs[] >> simp[do_eq_def] >> rw[] >> fs[LIST_REL_EL_EQN] >> metis_tac[])
-  >- simp[]
-  >- (simp[PULL_EXISTS] >> rpt gen_tac >> strip_tac >>
-      ONCE_REWRITE_TAC [do_eq_def] >>
-      Cases_on `do_eq u1 v1` >> fs[] >> simp[bool_case_eq] >> dsimp[] >>
-      rename1 `do_eq u1 v1 = Eq_val b` >> Cases_on `b` >> simp[] >>
-      rpt strip_tac >> nailIHx strip_assume_tac >> simp[] >> metis_tac[])
-  >- (simp[PULL_EXISTS] >> ONCE_REWRITE_TAC[do_eq_def] >> simp[])
-  >- (simp[PULL_EXISTS] >> ONCE_REWRITE_TAC[do_eq_def] >> simp[]));
-
-val kvrel_do_eq = save_thm("kvrel_do_eq", kvrel_do_eq0 |> CONJUNCT1);
-
-val kvrel_list_to_v = Q.store_thm("kvrel_list_to_v",
-  `!xs1 xs2 ys1 ys2.
-     LIST_REL (kvrel g) xs1 xs2 /\
-     LIST_REL (kvrel g) ys1 ys2 /\
-     kvrel g (list_to_v xs1) (list_to_v xs2) /\
-     kvrel g (list_to_v ys1) (list_to_v ys2) ==>
-       kvrel g (list_to_v (xs1 ++ ys1)) (list_to_v (xs2 ++ ys2))`,
-  Induct >- rw [list_to_v_def] \\ gen_tac
-  \\ Induct \\ rw [list_to_v_def] \\ fs []);
-
-val kvrel_v2l_l2v = Q.store_thm("kvrel_v2l_l2v",
-  `!x y xs ys.
-     kvrel g x y /\
-     v_to_list x = SOME xs /\
-     v_to_list y = SOME ys ==>
-       kvrel g (list_to_v xs) (list_to_v ys)`,
-  ho_match_mp_tac v_to_list_ind \\ rw [v_to_list_def]
-  \\ fs [list_to_v_def] \\ rveq
-  \\ fs [v_to_list_def] \\ rveq
-  \\ fs [list_to_v_def, case_eq_thms] \\ rveq
-  \\ fs [list_to_v_def]
-  \\ res_tac);
-
-(* necessary(!) *)
-val kvrel_op_correct_Rval = Q.store_thm(
-  "kvrel_op_correct_Rval",
-  `LIST_REL (kvrel g) vs1 vs2 ∧ do_app opn vs1 s01 = Rval(v1,s1) ∧
-   ksrel g s01 s02 ⇒
-   ∃v2 s2. do_app opn vs2 s02 = Rval(v2,s2) ∧ ksrel g s1 s2 ∧
-           kvrel g v1 v2`,
-  Cases_on `opn` >> simp[do_app_def, case_eq_thms, bool_case_eq, PULL_EXISTS] >>
-  TRY (rw[] >> fs[LIST_REL_EL_EQN] >> NO_TAC) \\
-  TRY (rw[] >> fs[] >>
-       imp_res_tac ksrel_flookup_refs \\ fs[ksrel_def] >>
-       imp_res_tac fmap_rel_def \\ fs[] \\
-       rveq \\ fs[LIST_REL_EL_EQN] \\
-       TRY (CASE_TAC \\ fs[] \\ rveq \\ fs[]) \\
-       TRY (match_mp_tac fmap_rel_FUPDATE_same) \\ fs[]
-       \\ fs[LIST_REL_EL_EQN,OPTREL_def,LIST_REL_REPLICATE_same,EVERY2_LUPDATE_same]
-       \\ first_x_assum match_mp_tac \\ rw[] \\ fs[] \\ intLib.COOPER_TAC)
-  >- (csimp[get_global_def] >> simp[ksrel_def] >>
-      simp[LIST_REL_EL_EQN, OPTREL_def] >> rpt strip_tac >> rveq >>
-      res_tac >> fs[] >> rveq >> simp[])
-  >- (csimp[get_global_def, PULL_EXISTS] >> simp[ksrel_def] >> rw[] >>
-      fs[LIST_REL_EL_EQN] >> rfs[] >> res_tac >> fs[OPTREL_def] >> fs[] >>
-      simp[EL_LUPDATE, bool_case_eq] >> metis_tac[])
-  >- (
-    rw [] >>
-    fs [] >>
-    rw [] >>
-    imp_res_tac LIST_REL_LENGTH
-    >- intLib.ARITH_TAC
-    >- intLib.ARITH_TAC >>
-    irule EVERY2_APPEND_suff >>
-    simp [] >>
-    irule EVERY2_TAKE >>
-    irule EVERY2_DROP >>
-    simp [])
-  >- (rw[] >> fs[] >>
-      imp_res_tac kvrel_v_to_list >> fs[ksrel_def] \\ rfs[] >>
-      qpat_x_assum`_ = SOME wss`mp_tac >>
-      DEEP_INTRO_TAC some_intro \\ fs[] \\ strip_tac \\
-      DEEP_INTRO_TAC some_intro \\ fs[PULL_EXISTS] \\
-      map_every qexists_tac[`wss`] \\
-      reverse conj_asm2_tac >- (
-        fs[LIST_EQ_REWRITE,EL_MAP,LIST_REL_EL_EQN,fmap_rel_def,FLOOKUP_DEF] \\
-        rfs[EL_MAP] \\ rw[] \\ res_tac \\ res_tac \\ fs[] \\
-        Cases_on`s02.refs ' (EL x ps)` \\ fs[] >>
-        metis_tac[ref_rel_def,ref_11]) \\
-      ntac 2 strip_tac >>
-      imp_res_tac INJ_MAP_EQ \\ fs[INJ_DEF] \\
-      imp_res_tac INJ_MAP_EQ \\ fs[INJ_DEF] )
-  >-
-   (rw [] \\ fs [] \\ rw []
-    \\ imp_res_tac kvrel_v_to_list \\ fs [] \\ rfs [] \\ rw []
-    \\ match_mp_tac kvrel_list_to_v \\ fs []
-    \\ imp_res_tac kvrel_v2l_l2v \\ fs [])
-  >- (rw[] >> fs[] >> metis_tac[kvrel_v_to_list])
-  >- (
-    rw[] \\ fs[] \\
-    rpt(qpat_x_assum`$some _ = _`mp_tac) \\
-    rpt(DEEP_INTRO_TAC some_intro) \\ rw[] \\
-    spose_not_then strip_assume_tac \\
-    imp_res_tac kvrel_v_to_list \\
-    rfs[LIST_EQ_REWRITE,LIST_REL_EL_EQN,EL_MAP] \\ fs[EL_MAP] \\
-    rfs[LIST_EQ_REWRITE,LIST_REL_EL_EQN,EL_MAP] \\
-    fs[EVERY_MEM,EXISTS_MEM] \\
-    metis_tac[v_11,integerTheory.INT_INJ,EL_MAP,o_THM,ORD_BOUND] )
-  >- (rw[] >> fs[] >> rw[] >> metis_tac[kvrel_do_eq]));
-
-val do_app_EQ_Rerr = Q.store_thm(
-  "do_app_EQ_Rerr",
-  `closSem$do_app opn vs s0 = Rerr e ⇒ e = Rabort Rtype_error`,
-  Cases_on `opn` >> simp[do_app_def, case_eq_thms, bool_case_eq, pair_case_eq] >> rw[]);
-
-val kvrel_lookup_vars = Q.store_thm(
-  "kvrel_lookup_vars",
-  `∀env01 env02 vars env1.
-     LIST_REL (kvrel g) env01 env02 ∧ lookup_vars vars env01 = SOME env1 ⇒
-     ∃env2. lookup_vars vars env02 = SOME env2 ∧
-            LIST_REL (kvrel g) env1 env2`,
-  Induct_on `vars` >> simp[lookup_vars_def, case_eq_thms, PULL_EXISTS] >>
-  fs[LIST_REL_EL_EQN] >> metis_tac[]);
-
-val loptrel_def = Define`
-  loptrel fv numargs lopt1 lopt2 ⇔
-     lopt2 = lopt1 ∨
-     lopt1 = NONE ∧
-     case (fv,lopt2) of
-       | (Closure (SOME loc1) ae _ n bod, SOME loc2) =>
-            loc1 = loc2 ∧ n = numargs ∧ ae = []
-       | (Recclosure (SOME loc1) ae _ fns i, SOME loc2) =>
-         i < LENGTH fns ∧ loc2 = loc1 + 2 * i ∧ numargs = FST (EL i fns) ∧
-         ae = []
-       | _ => F
-`;
-
-val ksrel_find_code = Q.store_thm(
-  "ksrel_find_code",
-  `ksrel g s1 s2 ⇒ find_code l (vs1:closSem$v list) s1.code = NONE`,
-  simp[ksrel_def, find_code_def, case_eq_thms, pair_case_eq]);
-
-val kvrel_dest_closure_SOME_Partial = Q.store_thm(
-  "kvrel_dest_closure_SOME_Partial",
-  `dest_closure max_app lopt1 f1 vs1 = SOME (Partial_app v1) ∧ kvrel g f1 f2 ∧
-   LIST_REL (kvrel g) vs1 vs2 ∧ loptrel f2 n lopt1 lopt2 ∧ LENGTH vs2 = n ⇒
-   ∃v2. dest_closure max_app lopt2 f2 vs2 = SOME (Partial_app v2) ∧
-        kvrel g v1 v2`,
-  simp[dest_closure_def, case_eq_thms, v_case_eq] >> rpt strip_tac >> rveq >> fs[] >>
-  rpt strip_tac >> fs[case_eq_thms, bool_case_eq] >> rveq >> fs[loptrel_def] >> rveq
-  >- (simp[EVERY2_APPEND_suff] >> fs[LIST_REL_EL_EQN] >> metis_tac[])
-  >- (Cases_on `lopt2` >> simp[EVERY2_APPEND_suff] >> fs[LIST_REL_EL_EQN] >>
-      rename1 `option_CASE lll` >> Cases_on `lll` >> fs[LIST_REL_EL_EQN])
-  >- (rpt (pairarg_tac >> fs[]) >> fs[bool_case_eq] >>
-      simp[EVERY2_APPEND_suff] >>
-      rename1 `LIST_REL val_approx_val envapx env2` >> simp[PULL_EXISTS] >>
-      qexists_tac `envapx` >>
-      fs[LIST_REL_EL_EQN] >> rename1 `EL ii` >>
-      qpat_x_assum `∀n. _ ⇒ UNCURRY f x y` mp_tac >>
-      disch_then (qspec_then `ii` mp_tac) >> simp[] >> rw[] >> simp[])
-  >- (rpt (pairarg_tac >> fs[]) >> fs[bool_case_eq] >>
-      Cases_on `lopt2` >> fs[] >> rename1 `option_CASE lll` >>
-      Cases_on `lll` >> fs[] >> rveq >>
-      qpat_x_assum `LIST_REL (UNCURRY _) _ _` mp_tac >>
-      CONV_TAC (LAND_CONV (REWRITE_CONV [LIST_REL_EL_EQN])) >>
-      rename1 `EL ii` >>
-      disch_then (CONJUNCTS_THEN2 assume_tac (qspec_then `ii` mp_tac)) >>
-      strip_tac >> rfs[] >> fs[LIST_REL_EL_EQN]))
-
-val kvrel_dest_closure_SOME_Full = Q.store_thm(
-  "kvrel_dest_closure_SOME_Full",
-  `dest_closure max_app lopt1 f1 vs1 = SOME (Full_app e1 env1 args1) ∧
-   kvrel g f1 f2 ∧
-   LIST_REL (kvrel g) vs1 vs2 ∧ loptrel f2 n lopt1 lopt2 ∧ LENGTH vs2 = n ⇒
-   ∃eapx e2 env2 args2.
-      dest_closure max_app lopt2 f2 vs2 = SOME (Full_app e2 env2 args2) ∧
-      LIST_REL val_approx_val eapx env2 ∧
-      LIST_REL (kvrel g) env1 env2 ∧ LIST_REL (kvrel g) args1 args2 ∧
-      kerel eapx g e1 e2`,
-  simp[dest_closure_def, case_eq_thms, bool_case_eq] >>
-  csimp[revtakerev, revdroprev] >> dsimp[] >> rpt strip_tac >> rveq >>
-  fs[] >> rveq >> fs[]
-  >- (imp_res_tac LIST_REL_LENGTH >> simp[] >> fs[] >>
-      simp[EVERY2_APPEND_suff, EVERY2_DROP, EVERY2_TAKE] >>
-      fs[loptrel_def] >>
-      qexists_tac `REPLICATE num_args Other ++ eapx` >> simp[] >>
-      rpt conj_tac >>
-      TRY (irule EVERY2_APPEND_suff >> simp[] >>
-           simp[LIST_REL_EL_EQN, LENGTH_REPLICATE, EL_REPLICATE]) >>
-      Cases_on `lopt2` >> fs[] >>
-      rename1 `option_CASE lll` >> Cases_on `lll` >> fs[] >> rveq >>
-      fs[check_loc_def])
-  >- (rpt (pairarg_tac >> fs[]) >> imp_res_tac LIST_REL_LENGTH >> fs[] >>
-      fs[bool_case_eq] >> rveq >>
-      qpat_x_assum `LIST_REL (UNCURRY _) _ _`
-        (fn th => (mp_tac o SIMP_RULE (srw_ss()) [LIST_REL_EL_EQN]) th >>
-                  assume_tac th) >>
-      rename1 `EL ii` >> simp[] >>
-      disch_then (qspec_then `ii` mp_tac) >> simp[] >> strip_tac >> rveq >>
-      simp[EVERY2_TAKE] >> rename1 `REPLICATE nargs Other` >>
-      rename1 `GENLIST (option_CASE locc _ _)` >>
-      rename1 `LIST_REL (UNCURRY _) fns1 fns2` >>
-      rename1 `LIST_REL val_approx_val envapx _` >>
-      qexists_tac `REPLICATE nargs Other ++
-                   GENLIST (case locc of
-                              | NONE => K Other
-                              | SOME n => (λi. Clos (2*i + n) (FST (EL i fns1))))
-                           (LENGTH fns2) ++ envapx` >> simp[] >>
-      conj_tac
-      >- (fs[loptrel_def] >> Cases_on `lopt2` >> fs[] >>
-          rename1 `option_CASE lll` >> Cases_on `lll` >> fs[] >>
-          fs[check_loc_def]) >>
-      conj_tac >> rpt (irule EVERY2_APPEND_suff) >> simp[EVERY2_DROP]
-      >- simp[LIST_REL_EL_EQN, EL_REPLICATE, LENGTH_REPLICATE]
-      >- (simp[LIST_REL_GENLIST] >> Cases_on `locc` >> simp[] >>
-          fs[LIST_REL_EL_EQN, UNCURRY])
-      >- (simp[LIST_REL_GENLIST] >> rpt strip_tac >>
-          qexists_tac `envapx` >> simp[])))
-
-val kvrel_subspt = Q.store_thm(
-  "kvrel_subspt",
-  `∀g v1 v2 g'. kvrel g v1 v2 ∧ subspt g g' ⇒ kvrel g' v1 v2`,
-  ho_match_mp_tac val_rel_ind >> simp[PULL_EXISTS] >> rpt strip_tac
-  >- (irule EVERY2_MEM_MONO >> imp_res_tac LIST_REL_LENGTH >>
-      simp[FORALL_PROD, MEM_ZIP, PULL_EXISTS] >> qexists_tac `kvrel g` >>
-      simp[] >> metis_tac[MEM_EL])
-  >- (rename1 `LIST_REL val_approx_val envapx _` >> qexists_tac `envapx` >>
-      simp[] >> rpt conj_tac >>
-      TRY (irule EVERY2_MEM_MONO >> imp_res_tac LIST_REL_LENGTH >>
-           simp[FORALL_PROD, MEM_ZIP, PULL_EXISTS] >>
-           qexists_tac `kvrel g` >> simp[] >> metis_tac[MEM_EL]) >>
-      fs[exp_rel_def] >> metis_tac[subspt_trans])
-  >- (rename1 `LIST_REL val_approx_val envapx _` >> qexists_tac `envapx` >>
-      simp[] >> rpt conj_tac >>
-      TRY (irule EVERY2_MEM_MONO >> imp_res_tac LIST_REL_LENGTH >>
-           simp[FORALL_PROD, MEM_ZIP, PULL_EXISTS] >>
-           qexists_tac `kvrel g` >> simp[] >> metis_tac[MEM_EL]) >>
-      qpat_x_assum `LIST_REL (UNCURRY _) _ _` mp_tac >> simp[LIST_REL_EL_EQN] >>
-      rpt strip_tac >> fs[] >> rfs[] >> rpt (pairarg_tac >> fs[]) >>
-      rename1 `nn < LENGTH _` >> first_x_assum (qspec_then `nn` mp_tac) >>
-      simp[] >> simp[exp_rel_def] >> metis_tac[subspt_trans]))
-
-val kvrel_LIST_REL_subspt = Q.store_thm(
-  "kvrel_LIST_REL_subspt",
-  `∀vs1 vs2. LIST_REL (kvrel g) vs1 vs2 ⇒
-             ∀g'. subspt g g' ⇒ LIST_REL (kvrel g') vs1 vs2`,
-  Induct_on `LIST_REL` >> simp[] >> metis_tac[kvrel_subspt]);
-
-val ksrel_subspt = Q.store_thm(
-  "ksrel_subspt",
-  `ksrel g s1 s2 ∧ subspt g g' ⇒ ksrel g' s1 s2`,
-  simp[ksrel_def] >> rpt strip_tac
-  >- (irule EVERY2_mono >>
-      qexists_tac `OPTREL (kvrel g)` >> simp[] >> rpt strip_tac >>
-      irule OPTREL_MONO >> qexists_tac `kvrel g` >>
-      metis_tac[kvrel_subspt])
-  >- (irule fmap_rel_mono >> qexists_tac `ref_rel (kvrel g)` >> simp[] >>
-      Cases >> simp[PULL_EXISTS] >> metis_tac[kvrel_LIST_REL_subspt]));
-
-val krrel_better_subspt = Q.store_thm(
-  "krrel_better_subspt",
-  `krrel g (res1,s1) (res2,s2) ∧ subspt g g' ⇒ krrel g' (res1,s1) (res2,s2)`,
-  Cases_on `res1` >> simp[krrel_err_rw] >>
-  metis_tac[kvrel_LIST_REL_subspt, ksrel_subspt, kvrel_subspt]);
-
-val dest_closure_SOME_Full_app_args_nil = Q.store_thm(
-  "dest_closure_SOME_Full_app_args_nil",
-  `dest_closure max_app (SOME loc) f args = SOME (Full_app exp1 env args1) ⇒
-   args1 = []`,
-  simp[dest_closure_def, case_eq_thms, bool_case_eq, revtakerev] >> strip_tac >> rveq
-  >- (fs[check_loc_def] >> simp[DROP_LENGTH_NIL_rwt]) >>
-  pairarg_tac >> fs[bool_case_eq] >> rveq >> fs[check_loc_def] >> rveq >>
-  simp[DROP_LENGTH_NIL_rwt]);
-
-val eqtI_thm = EQ_CLAUSES |> SPEC_ALL |> CONJUNCTS |> el 2 |> GSYM
-
-val v_caseT = v_case_eq |> INST_TYPE [alpha |-> bool] |> Q.INST [`v` |-> `T`]
-                        |> REWRITE_RULE []
-val optcaset = ``option$option_CASE``
-val opt_caseT = case_eq_thms |> CONJUNCTS
-                    |> List.find (fn th => th |> concl |> lhs |> lhs
-                                              |> strip_comb
-                                              |> #1 |> same_const optcaset)
-                    |> valOf
-                    |> INST_TYPE [beta |-> bool]
-                    |> Q.INST [`v'` |-> `T`]
-                    |> SIMP_RULE (srw_ss()) []
-
-
-val loptrel_arg1_SOME = save_thm(
-  "loptrel_arg1_SOME",
-  loptrel_def |> SPEC_ALL |> Q.INST [`lopt1` |-> `SOME loc1`]
-              |> SIMP_RULE (srw_ss()) [opt_caseT, v_caseT])
-
-val loptrel_arg1_NONE = save_thm(
-  "loptrel_arg1_NONE",
-  loptrel_def |> SPEC_ALL |> Q.INST [`lopt1` |-> `NONE`]
-              |> SIMP_RULE (srw_ss()) [opt_caseT, v_caseT])
-
-val kvrel_dest_closure_every_Fn_vs_NONE = Q.store_thm(
-  "kvrel_dest_closure_every_Fn_vs_NONE",
-  `kvrel g f1 f2 ∧ dest_closure max_app locopt f1 args0 = SOME (Full_app e env args) ⇒
-   every_Fn_vs_NONE [e]`,
-  simp[dest_closure_def, case_eq_thms, bool_case_eq] >> strip_tac >> rveq >> fs[] >>
-  rveq >> simp[Once every_Fn_vs_NONE_EVERY] >> pairarg_tac >>
-  fs[bool_case_eq] >> rveq >> fs[EVERY_MEM, FORALL_PROD, NOT_LESS_EQUAL] >>
-  metis_tac[MEM_EL]);
-
-val known_correct0 = Q.prove(
-  `(∀a es env1 env2 (s01:('a,'b) closSem$state) s02 res1 s1 g0 g g' as ealist.
-      a = (es,env1,s01) ∧ evaluate (es, env1, s01) = (res1, s1) ∧
-      EVERY esgc_free es ∧ subspt g0 g ∧ subspt g g' ∧
-      LIST_REL val_approx_val as env1 ∧ EVERY vsgc_free env1 ∧
-      every_Fn_vs_NONE es ∧
-      LIST_REL (kvrel g') env1 env2 ∧ ksrel g' s01 s02 ∧
-      state_globals_approx s01 g' ∧ BAG_ALL_DISTINCT (elist_globals es) ∧
-      ssgc_free s01 ∧ known es as g0 = (ealist, g) ⇒
-      ∃res2 s2.
-        evaluate(MAP FST ealist, env2, s02) = (res2, s2) ∧
-        krrel g' (res1,s1) (res2,s2)) ∧
-   (∀lopt1 f1 args1 (s01:('a,'b) closSem$state) res1 s1 lopt2 f2 args2 s02 g.
-      evaluate_app lopt1 f1 args1 s01 = (res1,s1) ∧ ssgc_free s01 ∧
-      kvrel g f1 f2 ∧ LIST_REL (kvrel g) args1 args2 ∧
-      ksrel g s01 s02 ∧ state_globals_approx s01 g ∧ vsgc_free f1 ∧
-      EVERY vsgc_free args1 ∧ loptrel f2 (LENGTH args1) lopt1 lopt2 ⇒
-      ∃res2 s2.
-        evaluate_app lopt2 f2 args2 s02 = (res2,s2) ∧
-        krrel g (res1,s1) (res2,s2))`,
-  ho_match_mp_tac evaluate_ind >> rpt conj_tac
-  >- (say "nil" >> simp[evaluate_def, known_def])
-  >- (say "cons" >>
-      simp[evaluate_def, known_def, pair_case_eq, result_case_eq,
-           BAG_ALL_DISTINCT_BAG_UNION] >>
-      rpt strip_tac >> rveq >> rpt (pairarg_tac >> fs[]) >> rveq >> simp[] >>
-      first_x_assum (patresolve `known [_] _ _ = _` last) >>
-      disch_then (resolve_selected (el 4)) >> simp[] >>
-      patresolve `known [_] _ _ = _` hd subspt_known_elist_globals >> simp[] >>
-      disch_then (resolve_selected hd) >> simp[] >> strip_tac >>
-      disch_then (resolve_selected last) >> simp[] >>
-      (impl_keep_tac >- metis_tac[subspt_trans]) >>
-      rw[]
-      >- (imp_res_tac known_sing_EQ_E >> rveq >> fs[] >>
-          sel_ihpc last >> simp[] >> disch_then (resolve_selected (el 3)) >>
-          simp[] >> disch_then (resolve_selected hd) >> simp[] >> impl_tac
-          >- (conj_tac
-              >- (resolve_selected hd (GEN_ALL kca_sing_sga) >> simp[] >>
-                  disch_then (resolve_selected last) >> simp[] >>
-                  metis_tac[kvrel_LIST_REL_val_approx, kvrel_EVERY_vsgc_free,
-                            ksrel_sga, ksrel_ssgc_free]) >>
-              metis_tac[ssgc_free_preserved_SING']) >> rw[] >>
-          simp[Once evaluate_CONS] >> imp_res_tac evaluate_SING >> rveq >>
-          fs[])
-      >- (imp_res_tac known_sing_EQ_E >> rveq >> fs[] >> sel_ihpc last >>
-          simp[] >> disch_then (resolve_selected (el 3)) >> simp[] >>
-          disch_then (resolve_selected hd) >> simp[] >> impl_tac
-          >- (conj_tac
-              >- (resolve_selected hd (GEN_ALL kca_sing_sga) >> simp[] >>
-                  disch_then (resolve_selected last) >> simp[] >>
-                  metis_tac[kvrel_LIST_REL_val_approx, kvrel_EVERY_vsgc_free,
-                            ksrel_sga, ksrel_ssgc_free]) >>
-              metis_tac[ssgc_free_preserved_SING']) >> rw[] >>
-          simp[Once evaluate_CONS, result_case_eq] >> fs[krrel_err_rw] >>
-          dsimp[] >> metis_tac[result_CASES])
-      >- (imp_res_tac known_sing_EQ_E >> rveq >> fs[] >>
-          simp[Once evaluate_CONS, result_case_eq, pair_case_eq] >>
-          dsimp[] >> fs[krrel_err_rw] >> metis_tac[pair_CASES, result_CASES]))
-  >- (say "var" >>
-      simp[evaluate_def, bool_case_eq, known_def] >>
-      rpt strip_tac >> fs[LIST_REL_EL_EQN])
-  >- (say "if" >>
-      simp[evaluate_def, pair_case_eq, bool_case_eq, BAG_ALL_DISTINCT_BAG_UNION,
-           result_case_eq, known_def] >> rpt strip_tac >> rveq >> fs[] >>
-      rpt (pairarg_tac >> fs[]) >> rveq >> fs[] >> fixeqs >>
-      imp_res_tac known_sing_EQ_E >> rveq >> fs[] >> rveq >>
-      map_every rename1 [`ksrel g' s01 s02`, `subspt g g'`,
-                           `known [eb] as g2 = ([(eb',eapx)], g)`,
-                           `known [tb] as g1 = ([(tb',tapx)], g2)`,
-                           `known [gd] as g0 = ([(gd',gapx)], g1)`] >>
-      `known [gd;tb] as g0 = ([(gd',gapx); (tb',tapx)], g2)`
-        by simp[known_def] >>
-      resolve_selected hd (subspt_known_elist_globals)>> simp[] >>
-      disch_then (resolve_selected hd) >> simp[] >> strip_tac >>
-      patresolve `known [gd] _ _ = _` hd subspt_known_elist_globals >> simp[] >>
-      disch_then (resolve_selected hd) >> simp[] >> strip_tac
-      >- (first_x_assum (patresolve `state_globals_approx _ _` (el 6)) >>
-          rpt (disch_then (resolve_selected last) >> simp[]) >>
-          impl_keep_tac >- metis_tac[subspt_trans] >> rw[] >>
-          simp[evaluate_def] >> imp_res_tac evaluate_SING >> fs[] >> rveq >>
-          fs[] >> rveq >> sel_ihpc last >> simp[] >> disch_then irule >>
-          simp[]
-          >- metis_tac[ssgc_free_preserved_SING']
-          >- (patresolve `known [gd] _ _ = _` hd (GEN_ALL kca_sing_sga) >>
-              simp[] >> disch_then (resolve_selected last) >> simp[] >>
-              metis_tac[ksrel_sga, kvrel_LIST_REL_val_approx,
-                        kvrel_EVERY_vsgc_free, ksrel_ssgc_free])
-          >- metis_tac[subspt_trans])
-      >- (first_x_assum (patresolve `state_globals_approx _ _` (el 6)) >>
-          rpt (disch_then (resolve_selected last) >> simp[]) >>
-          impl_keep_tac >- metis_tac[subspt_trans] >> rw[] >>
-          simp[evaluate_def] >> imp_res_tac evaluate_SING >> fs[] >> rveq >>
-          fs[] >> rveq >> sel_ihpc last >> simp[] >> disch_then irule >>
-          simp[]
-          >- metis_tac[ssgc_free_preserved_SING']
-          >- (patresolve `known [gd] _ _ = _` hd (GEN_ALL kca_sing_sga) >>
-              simp[] >> disch_then (resolve_selected last) >> simp[] >>
-              metis_tac[ksrel_sga, kvrel_LIST_REL_val_approx,
-                        kvrel_EVERY_vsgc_free, ksrel_ssgc_free,
-                        state_approx_better_definedg, known_better_definedg]))
-      >- ((* guard doesn't evaluate to T or F *) sel_ihpc (el 6) >> simp[] >>
-          rpt (disch_then (resolve_selected last) >> simp[]) >>
-          impl_keep_tac >- metis_tac[subspt_trans] >> rw[] >>
-          simp[evaluate_def] >> imp_res_tac evaluate_SING >> fs[] >> rveq >>
-          fs[] >> rveq >> dsimp[bool_case_eq] >> rpt disj2_tac >>
-          rpt strip_tac >> rveq >> fs[])
-      >- ((* guard errors *) sel_ihpc (el 6) >> simp[] >>
-          rpt (disch_then (resolve_selected last) >> simp[]) >>
-          impl_keep_tac >- metis_tac[subspt_trans] >> rw[] >>
-          dsimp[evaluate_def, result_case_eq, bool_case_eq] >>
-          fs[krrel_err_rw] >> metis_tac[pair_CASES, result_CASES]))
-  >- (say "let" >>
-      simp[evaluate_def, pair_case_eq, result_case_eq] >>
-      rpt strip_tac >> rveq >> fs[known_def] >>
-      rpt (pairarg_tac >> fs[]) >> rveq >> fs[BAG_ALL_DISTINCT_BAG_UNION] >>
-      map_every rename1 [`known [bod] _ g1 = (_, g)`,
-                           `known _ _ g0 = (_, g1)`,
-                           `subspt g gg`] >>
-      patresolve `known _ _ g0 = _` hd subspt_known_elist_globals >> simp[] >>
-      disch_then (resolve_selected hd) >> simp[] >>
-      (impl_tac >- fs[BAG_DISJOINT, DISJOINT_SYM]) >> strip_tac >>
-      first_x_assum (patresolve `known _ _ g0 = _` last) >> simp[] >>
-      rpt (disch_then (resolve_selected last) >> simp[]) >>
-      (impl_keep_tac >- metis_tac[subspt_trans]) >> rw[] >>
-      simp[evaluate_def, result_case_eq]
-      >- (imp_res_tac known_sing_EQ_E >> rveq >> fs[] >>
-          rveq >> sel_ihpc last >> simp[] >> disch_then irule >> simp[]
-          >- metis_tac[ssgc_evaluate]
-          >- metis_tac[ssgc_evaluate,rsgc_free_def]
-          >- (resolve_selected last known_correct_approx >> simp[] >>
-              rpt (disch_then (resolve_selected hd) >> simp[]) >>
-              metis_tac[ksrel_sga, kvrel_EVERY_vsgc_free,
-                        kvrel_LIST_REL_val_approx, ksrel_ssgc_free])
-          >- simp[EVERY2_APPEND_suff]
-          >- (irule EVERY2_APPEND_suff >> simp[] >>
-              resolve_selected last known_correct_approx >> simp[] >>
-              rpt (disch_then (resolve_selected hd) >> simp[]) >>
-              metis_tac[ksrel_sga, kvrel_EVERY_vsgc_free,
-                        kvrel_LIST_REL_val_approx, ksrel_ssgc_free]))
-      >- (fs[krrel_err_rw, result_case_eq] >> dsimp[] >>
-          metis_tac[pair_CASES, result_CASES]))
-  >- (say "raise" >>
-      simp[evaluate_def, pair_case_eq, result_case_eq] >>
-      rpt strip_tac >> rveq >> fs[known_def] >> pairarg_tac >> fs[] >>
-      imp_res_tac known_sing_EQ_E >> fs[] >> rveq >> fs[] >>
-      simp[evaluate_def, pair_case_eq, result_case_eq] >>
-      nailIHx strip_assume_tac >> simp[] >> fs[]
-      >- (imp_res_tac evaluate_SING >> fs[])
-      >- (dsimp[] >> fs[krrel_err_rw] >> metis_tac[result_CASES]))
-  >- (say "handle" >>
-      simp[evaluate_def, pair_case_eq, result_case_eq,
-           BAG_ALL_DISTINCT_BAG_UNION, error_case_eq, known_def] >>
-      rpt strip_tac >> rveq >> fs[] >>
-      rpt (pairarg_tac >> fs[]) >> rveq >>
-      imp_res_tac known_sing_EQ_E >> rveq >> fs[] >> rveq >>
-      map_every rename1 [`known _ (_ :: _) g1 = (_, g)`,
-                           `known _ _ g0 = (_, g1)`,
-                           `subspt g gg`] >>
-      patresolve `known _ _ g0 = _` hd subspt_known_elist_globals >> simp[] >>
-      rpt (disch_then (resolve_selected hd) >> simp[]) >> strip_tac >>
-      first_x_assum (patresolve `state_globals_approx _ _`  (el 6)) >> simp[] >>
-      rpt (disch_then (resolve_selected last) >> simp[]) >>
-      (impl_keep_tac >- metis_tac[subspt_trans]) >> rw[] >>
-      simp[evaluate_def, pair_case_eq, result_case_eq, error_case_eq]
-      >- (dsimp[] >> fs[PULL_EXISTS] >> sel_ihpc last >> simp[] >>
-          fs[krrel_err_rw] >> disch_then irule >> simp[]
-          >- metis_tac[ssgc_free_preserved_SING']
-          >- first_assum
-               (mp_then (Pos last) (mp_tac >~ (simp[] >> NO_TAC)) ssgc_evaluate)
-          >- (patresolve `known _ _ g0 = _` hd (GEN_ALL kca_sing_sga) >>
-              simp[] >> disch_then (resolve_selected last) >> simp[] >>
-              metis_tac[ksrel_ssgc_free,kvrel_EVERY_vsgc_free,ksrel_sga,
-                        kvrel_LIST_REL_val_approx]))
-      >- (fs[krrel_err_rw, result_case_eq, error_case_eq] >> dsimp[] >>
-          metis_tac[pair_CASES, result_CASES, error_CASES]))
-  >- (say "op" >>
-      simp[evaluate_def, pair_case_eq, result_case_eq, known_def,
-           BAG_ALL_DISTINCT_BAG_UNION] >>
-      rpt gen_tac >> strip_tac >> rpt gen_tac >>
-      Cases_on `op = Install` >- cheat >>
-      rpt (pairarg_tac >> fs[]) >>
-      rename[`isGlobal opn`, `gO_destApx apx`] >>
-      cheat (*
-      Cases_on `isGlobal opn ∧ gO_destApx apx ≠ gO_None`
-      >- (pop_assum strip_assume_tac >> simp[] >>
-          Cases_on `opn` >> fs[isGlobal_def] >>
-          Cases_on `apx` >> fs[gO_destApx_def] >> rveq >>
-          fs[known_op_def, NULL_EQ, bool_case_eq, case_eq_thms] >> rveq >>
-          imp_res_tac known_LENGTH_EQ_E >> fs[LENGTH_NIL_SYM] >> rveq >>
-          simp[evaluate_def] >>
-          rpt strip_tac >> rveq >> fs[evaluate_def, do_app_def, case_eq_thms] >>
-          fs[state_globals_approx_def, subspt_def] >> rveq >> simp[] >>
-          fs[known_def] >> rveq
-          >- (rename[`lookup n g0 = SOME (Tuple tg [])`,
-                     `kvrel g1 v (Block tg [])`] >>
-              `lookup n g1 = SOME (Tuple tg [])` by metis_tac[domain_lookup] >>
-              res_tac >> fs[] >> rveq >> fs[val_approx_val_def]) >>
-          (* TODO: clos_known$ is only necessary because of HOL issue #430 *)
-          rename[`lookup n g0 = SOME (clos_known$Int i)`, `kvrel g1 v (Number i)`] >>
-          `lookup n g1 = SOME (Int i)` by metis_tac[domain_lookup] >>
-          metis_tac[val_rel_def, val_approx_val_def, SOME_11]) >>
-      rename[`closLang$Op tr opn (MAP FST es)`,
-             `closSem$evaluate(MAP FST ealist,_,_)`] >>
-      rpt strip_tac >>
-      `ealist = [(Op tr opn (MAP FST es), apx)]`
-         by (Cases_on `isGlobal opn` >> fs[] >>
-             Cases_on `apx` >> fs[gO_destApx_def] >> every_case_tac >> fs[]) >>
-      pop_assum SUBST_ALL_TAC >> rveq >>
-      qpat_x_assum `¬(_ ∧ _)` kall_tac >> fs[] >>
-      dsimp[evaluate_def, result_case_eq, pair_case_eq] >>
-      sel_ihpc last >> simp[PULL_EXISTS] >>
-      rpt (disch_then (resolve_selected last) >> simp[]) >>
-      resolve_selected hd subspt_known_op_elist_globals >> simp[] >>
-      rpt (disch_then (resolve_selected hd) >> simp[]) >> strip_tac >>
-      (impl_keep_tac >- metis_tac[subspt_trans])
-      >- ((* args evaluate OK, do_app evaluates OK *)
-          metis_tac[kvrel_op_correct_Rval, EVERY2_REVERSE])
-      >- ((* args evaluate OK, do_app errors *)
-          rw[] >> imp_res_tac do_app_EQ_Rerr >> rw[] >>
-          metis_tac[result_CASES, pair_CASES])
-      >- ((* args error *) rw[] >> fs[krrel_err_rw] >>
-         metis_tac[result_CASES, pair_CASES]) *))
-  >- (say "fn" >>
-      simp[evaluate_def, pair_case_eq, result_case_eq,
-           known_def, bool_case_eq, case_eq_thms] >> rpt strip_tac >> rveq >> fs[] >>
-      rpt (pairarg_tac >> fs[]) >> rveq >> fs[] >>
-      imp_res_tac state_rel_max_app >> fs[] >>
-      dsimp[evaluate_def, case_eq_thms] >> imp_res_tac known_sing_EQ_E >> rveq >> fs[] >>
-      rveq >>
-      simp[exp_rel_def, PULL_EXISTS] >> metis_tac[kvrel_LIST_REL_val_approx])
-  >- (say "letrec" >>
-      simp[evaluate_def, pair_case_eq, result_case_eq, known_def, bool_case_eq,
-           case_eq_thms] >> rpt strip_tac >> rveq >> fs[letrec_case_eq] >>
-      rpt (pairarg_tac >> fs[]) >> rveq >> fs[] >>
-      fs[BAG_ALL_DISTINCT_BAG_UNION] >>
-      imp_res_tac state_rel_max_app >> fs[] >>
-      simp[evaluate_def, case_eq_thms, bool_case_eq] >> dsimp[] >>
-      simp[EVERY_MAP, EXISTS_MAP]
-      >- (disj1_tac >> simp[EVERY_MEM, FORALL_PROD] >>
-          imp_res_tac known_sing_EQ_E >> rveq >> fs[] >> rveq >>
-          sel_ihpc last >> simp[EVERY_GENLIST] >>
-          rpt (disch_then (resolve_selected last) >> simp[]) >>
-          rename1 `BAG_ALL_DISTINCT (elist_globals (MAP SND fns1))` >>
-          `∀n e. MEM (n,e) fns1 ⇒ n ≤ s02.max_app ∧ n ≠ 0`
-            by fs[EVERY_MEM, FORALL_PROD] >> simp[] >> strip_tac >>
-          simp[GSYM PULL_EXISTS] >> simp[Once EQ_SYM_EQ] >>
-          imp_res_tac LIST_REL_LENGTH >> fs[] >>
-          first_x_assum irule
-          >- (simp[LIST_REL_EL_EQN, EL_APPEND_EQN] >> qx_gen_tac `mm` >>
-              strip_tac >> rw[]
-              >- (fs[Once every_Fn_vs_NONE_EVERY] >>
-                  fs[EVERY_MAP] >> fs[EVERY_MEM, FORALL_PROD] >>
-                  metis_tac[])
-              >- (rename1 `LIST_REL val_approx_val apxs env1` >>
-                  qexists_tac `apxs` >> conj_tac
-                  >- metis_tac[kvrel_LIST_REL_val_approx] >>
-                  simp[LIST_REL_EL_EQN, EL_MAP] >>
-                  qx_gen_tac `nn` >> strip_tac >> pairarg_tac >>
-                  simp[] >> simp[exp_rel_def] >>
-                  map_every rename1 [`ksrel gg ss1 ss2`, `subspt g gg`,
-                                       `subspt g0 g`] >>
-                  ntac 2 (qexists_tac `g0`) >> simp[] >>
-                  rename1 `known [e1] env g0` >>
-                  Cases_on `known [e1] env g0` >>
-                  imp_res_tac known_sing_EQ_E >> fs[] >> rveq >>
-                  conj_tac >- metis_tac[subspt_trans] >>
-                  rename1 `known [subexp] env g0 = _` >>
-                  `elist_globals [subexp] = {||}`
-                    suffices_by metis_tac[known_emptySetGlobals_unchanged_g] >>
-                  fs[elglobals_EQ_EMPTY, MEM_MAP, PULL_EXISTS, FORALL_PROD] >>
-                  metis_tac[MEM_EL])
-              >- fs[LIST_REL_EL_EQN])
-          >- (irule EVERY2_APPEND_suff >> simp[] >>
-              simp[LIST_REL_GENLIST] >> qx_gen_tac `ii` >> strip_tac >>
-              rename1 `option_CASE lloc` >> Cases_on `lloc` >> simp[])) >>
-      disj2_tac >> fs[EXISTS_MEM, EXISTS_PROD] >> metis_tac[])
-  >- (say "app" >>
-      rpt gen_tac >> strip_tac >>
-      simp[evaluate_def, pair_case_eq, result_case_eq,
-           bool_case_eq, known_def, BAG_ALL_DISTINCT_BAG_UNION] >>
-      rpt strip_tac >> rveq >>
-      rpt (pairarg_tac >> fs[]) >> rveq >> fs[] >>
-      map_every imp_res_tac [known_sing_EQ_E, evaluate_SING] >> rveq >> fs[] >>
-      rveq
-      >- (map_every rename1 [
-            `known [fexp] apxs g1 = ([(fexp',fapx)], g)`,
-            `known args apxs g0 = (alist, g1)`,
-            `subspt g gg`] >>
-          patresolve `known [_] _ _ = _` (el 2) subspt_known_elist_globals >>
-          simp[] >> disch_then (resolve_selected (el 1)) >> simp[] >>
-          impl_tac >- fs[BAG_DISJOINT, DISJOINT_SYM] >> strip_tac >>
-          first_x_assum (patresolve `known args _ _ = _` last) >> simp[] >>
-          `subspt g1 gg` by metis_tac[subspt_trans] >>
-          rpt (disch_then (resolve_selected last) >> simp[]) >> rw[] >>
-          simp[evaluate_def] >> imp_res_tac known_LENGTH_EQ_E >> fs[] >>
-          first_x_assum (patresolve `known [_] _ _ = _` last) >> simp[] >>
-          disch_then (resolve_selected (el 2)) >> simp[] >>
-          disch_then (resolve_selected hd) >> simp[] >>
-          resolve_selected hd ssgc_evaluate >> simp[] >>
-          rpt (disch_then (resolve_selected hd) >> simp[]) >> strip_tac >>
-          impl_keep_tac
-          >- (patresolve `closSem$evaluate (MAP FST _, _, _) = _` last
-                         known_correct_approx >>
-              simp[] >> disch_then (resolve_selected hd) >> simp[] >>
-              metis_tac[ksrel_ssgc_free,kvrel_EVERY_vsgc_free,ksrel_sga,
-                        kvrel_LIST_REL_val_approx]) >>
-          rw[] >> simp[] >>
-          rename1 `evaluate_app loption1 v1 vs1 s21 = (result,ss1)` >>
-          `ssgc_free s21`
-            by metis_tac[ksrel_ssgc_free, ssgc_free_preserved_SING'] >> fs[] >>
-          first_x_assum (resolve_selected hd) >> simp[] >>
-          rpt (disch_then (resolve_selected hd) >> simp[]) >> strip_tac >>
-          `state_globals_approx s21 gg`
-            by (patresolve `known [_] _ _ = _` hd known_correct_approx >>
-                simp[] >> disch_then (resolve_selected last) >> simp[] >>
-                metis_tac[ksrel_ssgc_free,kvrel_EVERY_vsgc_free,ksrel_sga,
-                          kvrel_LIST_REL_val_approx]) >> fs[] >>
-          `vsgc_free v1`
-            by (patresolve `closSem$evaluate ([_],_,_) = (Rval [v1],_)` last
-                           ssgc_evaluate >> simp[]) >> fs[] >>
-          reverse (Cases_on `loption1`) >> simp[]
-          >- (first_x_assum irule >> simp[loptrel_def]) >>
-          rename1 `dest_Clos fapprox` >> Cases_on `dest_Clos fapprox` >>
-          simp[]
-          >- (first_x_assum irule >> simp[loptrel_def]) >>
-          rename1 `dest_Clos fapprox = SOME closapxvalue` >>
-          `∃clloc clarity. closapxvalue = (clloc, clarity)`
-            by metis_tac[pair_CASES] >> pop_assum SUBST_ALL_TAC >>
-          simp[] >> rename1 `LENGTH args > 0` >>
-          reverse (Cases_on `clarity = LENGTH args`) >> simp[]
-          >- (first_x_assum irule >> simp[loptrel_def]) >>
-          first_x_assum irule >> simp[loptrel_def] >>
-          qspecl_then [`[fexp]`, `apxs`, `g1`, `[(fexp',fapprox)]`, `g`]
-             mp_tac known_correct_approx >> simp[] >>
-          disch_then (resolve_selected last) >> simp[] >>
-          disch_then (qspec_then `gg` mp_tac) >> impl_tac
-          >- metis_tac[kvrel_LIST_REL_val_approx, ksrel_ssgc_free,
-                       kvrel_EVERY_vsgc_free, ksrel_sga] >>
-          fs[dest_Clos_eq_SOME] >> rveq >> rw[] >> simp[] >>
-          metis_tac[evaluate_length_imp])
-      >- (map_every rename1 [
-            `known [fexp] apxs g1 = ([(fexp',fapx)], g)`,
-            `known args apxs g0 = (alist, g1)`,
-            `subspt g gg`] >>
-          patresolve `known [_] _ _ = _` (el 2) subspt_known_elist_globals >>
-          simp[] >> disch_then (resolve_selected (el 1)) >> simp[] >>
-          impl_tac >- fs[BAG_DISJOINT, DISJOINT_SYM] >> strip_tac >>
-          first_x_assum (patresolve `known args _ _ = _` last) >> simp[] >>
-          `subspt g1 gg` by metis_tac[subspt_trans] >>
-          rpt (disch_then (resolve_selected last) >> simp[]) >> rw[] >>
-          simp[evaluate_def] >> imp_res_tac known_LENGTH_EQ_E >> fs[] >>
-          sel_ihpc last >> simp[] >>
-          disch_then (resolve_selected (el 2)) >> simp[] >>
-          disch_then (resolve_selected hd) >> simp[] >> reverse impl_tac
-          >- (rw[] >> simp[] >> fs[krrel_err_rw] >>
-              dsimp[result_case_eq] >> metis_tac[pair_CASES, result_CASES]) >>
-          conj_tac
-          >- (patresolve `closSem$evaluate (MAP FST _, _, _) = _` last
-                         known_correct_approx >>
-              simp[] >> disch_then (resolve_selected hd) >> simp[] >>
-              metis_tac[ksrel_ssgc_free,kvrel_EVERY_vsgc_free,ksrel_sga,
-                        kvrel_LIST_REL_val_approx]) >>
-          metis_tac [ssgc_evaluate])
-      >- (map_every rename1 [
-            `known [fexp] apxs g1 = ([(fexp',fapx)], g)`,
-            `known args apxs g0 = (alist, g1)`,
-            `subspt g gg`] >>
-          patresolve `known [_] _ _ = _` (el 2) subspt_known_elist_globals >>
-          simp[] >> disch_then (resolve_selected (el 1)) >> simp[] >>
-          impl_tac >- fs[BAG_DISJOINT, DISJOINT_SYM] >> strip_tac >>
-          first_x_assum (patresolve `known args _ _ = _` last) >> simp[] >>
-          `subspt g1 gg` by metis_tac[subspt_trans] >> strip_tac >>
-          nailIHx strip_assume_tac >>
-          simp[evaluate_def, bool_case_eq, result_case_eq, pair_case_eq] >>
-          imp_res_tac known_LENGTH_EQ_E >> rveq >> fs[] >>
-          fs[krrel_err_rw] >> dsimp[] >>
-          metis_tac[result_CASES,pair_CASES])
-      >- (map_every imp_res_tac [evaluate_IMP_LENGTH, known_LENGTH_EQ_E] >>
-          fs[] >> rw[] >> simp[evaluate_def]))
-  >- (say "tick" >> simp[dec_clock_def] >> rpt gen_tac >> strip_tac >>
-      simp[evaluate_def, bool_case_eq, known_def] >>
-      rename1 `(s0:('a,'b) closSem$state).clock = 0` >> Cases_on `s0.clock = 0` >>
-      fs[] >> rpt strip_tac >> rpt (pairarg_tac >> fs[]) >> rveq >> fs[] >>
-      simp[evaluate_def] >- fs[ksrel_def] >>
-      fs[dec_clock_def] >> fixeqs >> imp_res_tac known_sing_EQ_E >> rveq >>
-      fs[] >> rveq >>
-      map_every rename1 [
-        `known [exp1] apxs g0 = ([(exp2,apx)],g)`,
-        `evaluate([exp1],env1,s01 with clock := s01.clock - 1) = (res1,s1)`,
-        `ksrel gg s01 s02`] >>
-      sel_ihpc last >> simp[] >>
-      disch_then
-        (qspecl_then [`env2`, `s02 with clock := s02.clock - 1`, `gg`]
-                     mp_tac) >>
-      simp[] >> impl_keep_tac >- fs[ksrel_def] >>
-      `s02.clock = s01.clock` by fs[ksrel_def] >> simp[])
-  >- (say "call" >>
-      simp[evaluate_def, pair_case_eq, result_case_eq, case_eq_thms, bool_case_eq,
-           known_def] >> rw[]
-      >- (simp[] >> metis_tac[pair_CASES])
-      >- (rpt (pairarg_tac >> fs[]) >> rveq >> nailIHx strip_assume_tac >>
-          simp[evaluate_def] >> rw[] >>
-          imp_res_tac ksrel_find_code >> fs[])
-      >- (fixeqs >> rpt (pairarg_tac >> fs[]) >> rveq >> fs[] >>
-          nailIHx strip_assume_tac >>
-          imp_res_tac ksrel_find_code >> fs[])
-      >- (rpt (pairarg_tac >> fs[]) >> rveq >> fs[] >>
-          nailIHx strip_assume_tac >> simp[evaluate_def] >>
-          fs[krrel_err_rw] >>
-          dsimp[result_case_eq, case_eq_thms, pair_case_eq, bool_case_eq] >>
-          metis_tac[option_CASES, pair_CASES, result_CASES]))
-  >- (say "evaluate_app(nil)" >> simp[evaluate_def])
-  >- (say "evaluate_app(cons)" >> rpt gen_tac >> strip_tac >>
-      simp[evaluate_def, case_eq_thms, bool_case_eq, pair_case_eq, result_case_eq] >>
-      rpt strip_tac >> rveq >> fs[]
-      >- metis_tac[pair_CASES]
-      >- (simp[evaluate_def, case_eq_thms, bool_case_eq, pair_case_eq] >>
-          resolve_selected hd (GEN_ALL kvrel_dest_closure_SOME_Partial) >>
-          simp[PULL_EXISTS] >> imp_res_tac LIST_REL_LENGTH >> fs[] >>
-          rpt (disch_then (resolve_selected hd) >> simp[]) >>
-          strip_tac >> simp[] >> fs[ksrel_def])
-      >- (simp[evaluate_def, case_eq_thms, bool_case_eq, pair_case_eq] >>
-          resolve_selected hd (GEN_ALL kvrel_dest_closure_SOME_Partial) >>
-          simp[PULL_EXISTS] >> imp_res_tac LIST_REL_LENGTH >> fs[] >>
-          rpt (disch_then (resolve_selected hd) >> simp[]) >> strip_tac >>
-          simp[] >> fs[ksrel_def, dec_clock_def])
-      >- (simp[evaluate_def, case_eq_thms, bool_case_eq, pair_case_eq] >>
-          resolve_selected hd (GEN_ALL kvrel_dest_closure_SOME_Full) >>
-          simp[PULL_EXISTS] >> imp_res_tac LIST_REL_LENGTH >> fs[] >>
-          rpt (disch_then (resolve_selected hd) >> simp[]) >> strip_tac >>
-          simp[] >> imp_res_tac LIST_REL_LENGTH >> fs[ksrel_def])
-      >- (simp[evaluate_def, case_eq_thms, bool_case_eq, pair_case_eq] >>
-          resolve_selected hd (GEN_ALL kvrel_dest_closure_SOME_Full) >>
-          simp[PULL_EXISTS] >> imp_res_tac LIST_REL_LENGTH >> fs[] >>
-          rpt (disch_then (resolve_selected hd) >> simp[]) >> strip_tac >>
-          simp[] >> rename1 `ksrel g s01 s02` >>
-          `s02.clock = s01.clock` by fs[ksrel_def] >>
-          `s02.max_app = s01.max_app` by fs[ksrel_def] >>
-          imp_res_tac LIST_REL_LENGTH >> fs[] >> simp[PULL_EXISTS] >>
-          dsimp[] >> fs[PULL_EXISTS] >>
-          map_every rename1 [
-            `dest_closure _ lopt1 f1 (iarg1 :: iargs) =
-               SOME (Full_app exp1 env1 args1)`,
-            `evaluate([exp1],env1,dec_clock _ s01) = (Rval [v1], s11)`,
-            `kerel envapx gg exp1 exp2`] >> fs[exp_rel_def] >>
-          rpt disj1_tac >>
-          first_x_assum (patresolve `known [exp1] _ _ = _` last) >> simp[] >>
-          map_every rename1 [
-            `evaluate([exp1],env1,
-                      dec_clock (SUC (LENGTH iargs1) - LENGTH args2) s01)`,
-            `LIST_REL (kvrel gg) env1 env2`] >>
-          disch_then (qspecl_then [
-             `env2`,
-             `dec_clock (SUC (LENGTH iargs1) - LENGTH args2) s02`,
-             `gg`] mp_tac) >> simp[] >>
-          `set_globals exp1 = {||} ∧ EVERY vsgc_free env1 ∧
-           EVERY vsgc_free args1 ∧ esgc_free exp1`
-            by metis_tac[vsgc_free_Full_app_set_globals, EVERY_DEF,
-                         set_globals_empty_esgc_free] >> simp[] >>
-          qspec_then `[exp1]` mp_tac known_emptySetGlobals_unchanged_g >>
-          disch_then (resolve_selected hd) >> simp[] >>
-          disch_then SUBST_ALL_TAC >>
-          rename1 `LIST_REL val_approx_val envapx env1` >>
-          `LIST_REL val_approx_val envapx env1`
-            by metis_tac[kvrel_LIST_REL_val_approx] >>
-          `every_Fn_vs_NONE [exp1]`
-            by metis_tac[kvrel_dest_closure_every_Fn_vs_NONE] >>
-          impl_tac >- (simp[] >> fs[ksrel_def, dec_clock_def]) >> rw[] >>
-          simp[] >>
-          rename1 `loptrel f2 _ lopt1 lopt2` >>
-          reverse (Cases_on `lopt1`)
-          >- (fs[loptrel_arg1_SOME] >> rveq >>
-              imp_res_tac dest_closure_SOME_Full_app_args_nil >> fs[] >>
-              rveq >> simp[]) >>
-          qpat_x_assum `loptrel _ _ _ _` mp_tac >>
-          simp[loptrel_arg1_NONE] >> reverse strip_tac >> rveq
-          >- (imp_res_tac dest_closure_SOME_Full_app_args_nil >> fs[] >>
-              rveq >> simp[])
-          >- (imp_res_tac dest_closure_SOME_Full_app_args_nil >> fs[] >>
-              rveq >> simp[]) >>
-          first_x_assum irule >> simp[]
-          >- metis_tac[ssgc_free_preserved_SING', ssgc_free_dec_clock]
-          >- (patresolve `evaluate([exp1],_,_) = _` last ssgc_evaluate >>
-              simp[])
-          >- (patresolve `known [exp1] _ _ = _` hd known_correct_approx >>
-              simp[] >> disch_then (resolve_selected last) >> simp[] >>
-              metis_tac[ksrel_sga, ksrel_ssgc_free, kvrel_EVERY_vsgc_free])
-          >- simp[loptrel_def])
-      >- (imp_res_tac evaluate_SING >> fs[])
-      >- (simp[evaluate_def, case_eq_thms, bool_case_eq, pair_case_eq] >>
-          resolve_selected hd (GEN_ALL kvrel_dest_closure_SOME_Full) >>
-          simp[PULL_EXISTS] >> imp_res_tac LIST_REL_LENGTH >> fs[] >>
-          rpt (disch_then (resolve_selected hd) >> simp[]) >> strip_tac >>
-          simp[] >> rename1 `ksrel g s01 s02` >>
-          `s02.clock = s01.clock` by fs[ksrel_def] >>
-          imp_res_tac LIST_REL_LENGTH >> fs[] >> simp[PULL_EXISTS] >>
-          dsimp[] >>
-          map_every rename1 [
-            `dest_closure _ lopt1 f1 (iarg1 :: iargs) =
-               SOME (Full_app exp1 env1 args1)`,
-            `evaluate([exp1],env1,dec_clock _ s01) = (Rerr err1, s1)`,
-            `kerel envapx gg exp1 exp2`] >> fs[exp_rel_def] >>
-          first_x_assum (patresolve `known [exp1] _ _ = _` last) >> simp[] >>             map_every rename1 [
-            `evaluate([exp1],env1,
-                      dec_clock (SUC (LENGTH iargs1) - LENGTH args2) s01)`,
-            `LIST_REL (kvrel gg) env1 env2`] >>
-          disch_then (qspecl_then [
-             `env2`,
-             `dec_clock (SUC (LENGTH iargs1) - LENGTH args2) s02`,
-             `gg`] mp_tac) >> simp[] >>
-          `set_globals exp1 = {||} ∧ EVERY vsgc_free env1 ∧
-           EVERY vsgc_free args1 ∧ esgc_free exp1`
-            by metis_tac[vsgc_free_Full_app_set_globals, EVERY_DEF,
-                         set_globals_empty_esgc_free] >> simp[] >>
-          qspec_then `[exp1]` mp_tac known_emptySetGlobals_unchanged_g >>
-          disch_then (resolve_selected hd) >> simp[] >>
-          disch_then SUBST_ALL_TAC >>
-          rename1 `LIST_REL val_approx_val envapx env1` >>
-          `LIST_REL val_approx_val envapx env1`
-            by metis_tac[kvrel_LIST_REL_val_approx] >>
-          `every_Fn_vs_NONE [exp1]`
-            by metis_tac[kvrel_dest_closure_every_Fn_vs_NONE] >>
-          impl_tac >- (simp[] >> fs[ksrel_def, dec_clock_def]) >> rw[] >>
-          imp_res_tac state_rel_max_app >>
-          simp[] >> fs[krrel_err_rw] >>
-          rename1 `evaluate([exp2],_,_) = (res2,_)` >>
-          Cases_on `res2`
-          >- (imp_res_tac evaluate_SING >> simp[] >> metis_tac[pair_CASES]) >>
-          simp[])))
-
-val known_correct = save_thm(
-  "known_correct",
-  known_correct0 |> SIMP_RULE (srw_ss()) []);
-
-val known_preserves_every_Fn_NONE = Q.store_thm(
-  "known_preserves_every_Fn_NONE",
-  `∀es as g0 alist g.
-     known es as g0 = (alist,g) ∧ every_Fn_vs_NONE es ⇒
-     every_Fn_vs_NONE (MAP FST alist)`,
-  ho_match_mp_tac known_ind >> simp[known_def] >> rpt strip_tac >>
-  rpt (pairarg_tac >> fs[]) >> rveq >> fs[] >>
-  imp_res_tac known_sing_EQ_E >> rveq >> fs[] >> rveq
-  >- (simp[Once every_Fn_vs_NONE_EVERY] >> simp[GSYM every_Fn_vs_NONE_EVERY])
-  >- (every_case_tac >> simp[Once every_Fn_vs_NONE_EVERY])
-  >- (simp[Once every_Fn_vs_NONE_EVERY] >>
-      simp[EVERY_MEM, MEM_MAP, PULL_EXISTS, FORALL_PROD] >> rpt strip_tac >>
-      sel_ihpc hd >> rename1 `known[bod] env g0` >>
-      Cases_on `known[bod] env g0` >> simp[] >> imp_res_tac known_sing_EQ_E >>
-      rveq >> fs[] >> rveq >> disch_then irule >>
-      fs[Once every_Fn_vs_NONE_EVERY] >>
-      fs[EVERY_MEM, MEM_MAP, PULL_EXISTS, FORALL_PROD] >> metis_tac[]));
-
-val known_preserves_every_Fn_SOME = Q.store_thm(
-  "known_preserves_every_Fn_SOME",
-  `∀es as g0 alist g.
-     known es as g0 = (alist,g) ∧ every_Fn_SOME es ⇒
-     every_Fn_SOME (MAP FST alist)`,
-  ho_match_mp_tac known_ind >> simp[known_def] >> rpt strip_tac >>
-  rpt (pairarg_tac >> fs[]) >> rveq >> fs[] >>
-  imp_res_tac known_sing_EQ_E >> rveq >> fs[] >> rveq
-  >- (simp[Once every_Fn_SOME_EVERY]>>simp[GSYM every_Fn_SOME_EVERY])
-  >- (every_case_tac >> simp[Once every_Fn_SOME_EVERY])
-  >- (simp[Once every_Fn_SOME_EVERY] >>
-      simp[EVERY_MEM, MEM_MAP, PULL_EXISTS, FORALL_PROD] >> rpt strip_tac >>
-      sel_ihpc hd >> rename1 `known[bod] env g0` >>
-      Cases_on `known[bod] env g0` >> simp[] >> imp_res_tac known_sing_EQ_E >>
-      rveq >> fs[] >> rveq >> disch_then irule >>
-      fs[Once every_Fn_SOME_EVERY] >>
-      fs[EVERY_MEM, MEM_MAP, PULL_EXISTS, FORALL_PROD] >> metis_tac[]));
-
-fun abbrevify (asl,g) =
-  let val (l,r) = dest_imp g
-      fun abc t = if is_forall t then REWR_CONV (GSYM markerTheory.Abbrev_def) t
-                  else ALL_CONV t
-  in
-    if is_forall r then
-      CONV_TAC (LAND_CONV (EVERY_CONJ_CONV abc)) >> strip_tac
-    else ALL_TAC
-  end (asl,g)
-
-val unabbrevify = RULE_ASSUM_TAC (REWRITE_RULE [markerTheory.Abbrev_def])
-
-val say = say0 "known_idem"
-val merge_subapprox_cong = Q.store_thm(
-  "merge_subapprox_cong",
-  `a1 ◁ a2 ∧ b1 ◁ b2 ⇒ merge a1 b1 ◁ merge a2 b2`,
-  simp[subapprox_def] >>
-  metis_tac[merge_comm, merge_assoc]);
-
-val known_op_increases_subspt_info = Q.store_thm(
-  "known_op_increases_subspt_info",
-  `∀opn as1 g0 a1 a2 g1 g2 as2 g.
-     known_op opn as1 g0 = (a1,g1) ∧ subspt g0 g1 ∧ subspt g1 g2 ∧
-     LIST_REL $◁ as2 as1 ∧ known_op opn as2 g2 = (a2,g)
-    ⇒
-     a2 ◁ a1 ∧ subspt g2 g`,
-  rpt gen_tac >> Cases_on `opn` >>
-  simp[known_op_def, case_eq_thms, va_case_eq, bool_case_eq, NULL_EQ] >>
-  disch_then strip_assume_tac >> rveq >> simp[] >> fs[]
-  >- (fs[subspt_def] >> metis_tac[domain_lookup, NOT_SOME_NONE])
-  >- (fs[subspt_def] >> metis_tac[domain_lookup, subapprox_refl, SOME_11])
-  >- fs[subspt_def, DISJ_IMP_THM, lookup_insert]
-  >- (fs[subspt_def, DISJ_IMP_THM, lookup_insert, FORALL_AND_THM] >> rveq >>
-      rw[] >> fs[subapprox_def, merge_comm])
-  >- fs[subspt_def, lookup_insert, DISJ_IMP_THM]
-  >- (fs[subspt_def, lookup_insert, DISJ_IMP_THM, FORALL_AND_THM] >> rveq >>
-      rw[] >> fs[subapprox_def] >> metis_tac[merge_comm, merge_assoc])
-  >- (fs[LIST_REL_EL_EQN] >>
-      metis_tac[integerTheory.INT_INJ, integerTheory.INT_OF_NUM,
-                integerTheory.INT_LT])
-  >- (fs[LIST_REL_EL_EQN] >> rfs[]))
-
-val known_increases_subspt_info = Q.store_thm(
-  "known_increases_subspt_info",
-  `∀es as1 g0 alist1 g1 g2 as2 alist2 g.
-      known es as1 g0 = (alist1,g1) ∧ BAG_ALL_DISTINCT (elist_globals es) ∧
-      subspt g0 g1 ∧ subspt g1 g2 ∧ LIST_REL $◁ as2 as1 ∧
-      known es as2 g2 = (alist2,g)
-     ⇒
-      subspt g2 g ∧
-      LIST_REL $◁ (MAP SND alist2) (MAP SND alist1)`,
-  ho_match_mp_tac known_ind >> rpt conj_tac >> rpt gen_tac >> abbrevify >>
-  fs[known_def, BAG_ALL_DISTINCT_BAG_UNION] >>
-  rpt (gen_tac ORELSE disch_then strip_assume_tac)
-  >- (rveq >> simp[])
-  >- (rpt (pairarg_tac >> fs[]) >> rveq >> fs[] >>
-      imp_res_tac known_sing_EQ_E >> rveq >> fs[] >> rveq >>
-      map_every rename1 [`LIST_REL _ (MAP SND alist2) (MAP SND alist1)`,
-                           `known (exp2::es) as1 g01 = (alist1, g1)`,
-                           `known [exp1] as1 g0 = ([(_,apx1)], g01)`,
-                           `known [exp1] as2 g2 = ([(_,apx2)], g21)`] >>
-      patresolve `known [_] _ g0 = _` hd subspt_known_elist_globals >> simp[] >>
-      rpt (disch_then (resolve_selected hd) >> simp[]) >> strip_tac >> fs[] >>
-      unabbrevify >>
-      `subspt g01 g2` by metis_tac[subspt_trans] >>
-      first_x_assum (resolve_selected hd) >> simp[] >>
-      rpt (disch_then (resolve_selected hd) >> simp[]) >> strip_tac >>
-      `subspt g2 g21` by metis_tac[] >>
-      `subspt g1 g21` by metis_tac[subspt_trans] >>
-      `subspt g21 g` by metis_tac[] >> metis_tac[subspt_trans])
-  >- (say "var" >> rveq >> simp[any_el_ALT] >> fs[LIST_REL_EL_EQN] >> rw[])
-  >- (say "if" >>
-      rpt (pairarg_tac >> fs[]) >> rveq >> fs[] >>
-      imp_res_tac known_sing_EQ_E >> rveq >>
-      fs[PULL_EXISTS, EXISTS_PROD] >> rveq >>
-      map_every rename1 [
-        `merge apx2' apx3' ◁ merge apx2 apx3`,
-        `known [tb] as1 g01 = ([(_,apx2)], g02)`,
-        `known [tb] as2 g11 = ([(_,apx2')], g12)`,
-        `known [eb] as1 g02 = ([(_,apx3)], g1)`,
-        `known [ge] as1 g0 = ([(_,apx1)], g01)`] >>
-      `∃apxs. known [ge;tb] as1 g0 = (apxs, g02)` by simp[known_def] >>
-      resolve_selected hd subspt_known_elist_globals >> simp[] >>
-      rpt (disch_then (resolve_selected hd) >> simp[]) >> strip_tac >>
-      patresolve `known [ge] as1 g0 = _` hd subspt_known_elist_globals >>
-      simp[] >>
-      rpt (disch_then (resolve_selected hd) >> simp[]) >> strip_tac >> fs[] >>
-      unabbrevify >>
-      `subspt g01 g2` by metis_tac[subspt_trans] >>
-      first_x_assum (resolve_selected hd) >> simp[] >>
-      disch_then (resolve_selected last) >> simp[] >> strip_tac >>
-      first_x_assum (patresolve `known [tb] as2 _ = _` (el 3)) >> simp[] >>
-      impl_keep_tac
-      >- metis_tac[subspt_trans] >> strip_tac >>
-      first_x_assum (patresolve `known [eb] as2 _ = _` (el 3)) >> simp[] >>
-      impl_keep_tac
-      >- metis_tac[subspt_trans] >> strip_tac >>
-      conj_tac >- metis_tac[subspt_trans] >>
-      metis_tac[merge_subapprox_cong])
-  >- (say "let" >>
-      rpt (pairarg_tac >> fs[]) >> rveq >> fs[] >>
-      imp_res_tac known_sing_EQ_E >> rveq >> fs[] >> rveq >>
-      map_every rename1 [`apx' ◁ apx`,
-                           `known [bod] _ g01 = ([(_, apx)], g02)`,
-                           `known [bod] _ g21 = ([(_, apx')], g22)`,
-                           `known binds as1 g0 = (_, g01)`,
-                           `known binds as2 g2 = (_, g21)`] >>
-      patresolve `known binds as1 g0 = _` hd subspt_known_elist_globals >>
-      simp[] >>
-      rpt (disch_then (resolve_selected hd) >> simp[]) >> impl_tac
-      >- fs[BAG_DISJOINT, DISJOINT_SYM] >> strip_tac >> fs[] >> unabbrevify >>
-      first_x_assum (patresolve `known binds as2 _ = _` (el 3)) >> simp[] >>
-      impl_keep_tac >- metis_tac [subspt_trans] >> strip_tac >>
-      first_x_assum (patresolve `known [bod] _ g21 = _` (el 3)) >>
-      simp[EVERY2_APPEND_suff] >> impl_keep_tac >- metis_tac[subspt_trans] >>
-      metis_tac[subspt_trans])
-  >- (say "raise" >>
-      rpt (pairarg_tac >> fs[]) >> rveq >> fs[] >>
-      imp_res_tac known_sing_EQ_E >> rveq >> fs[] >> rveq >> unabbrevify >>
-      metis_tac[])
-  >- (say "tick" >>
-      rpt (pairarg_tac >> fs[]) >> rveq >> fs[] >>
-      imp_res_tac known_sing_EQ_E >> rveq >> fs[] >> rveq >> unabbrevify >>
-      fs[EXISTS_PROD] >> metis_tac[CONS_11, PAIR_EQ])
-  >- (say "handle" >>
-      rpt (pairarg_tac >> fs[]) >> rveq >> fs[] >>
-      imp_res_tac known_sing_EQ_E >> rveq >> fs[] >> rveq >>
-      map_every rename1 [
-        `merge apx1' apx2' ◁ merge apx1 apx2`,
-        `known [exp1] as1 g0 = ([(_,apx1)], g01)`,
-        `known [exp1] as2 g2 = ([(_,apx1')], g21)`,
-        `known [hndlr] (Other::as1) g01 = ([(_,apx2)], g1)`,
-        `known [hndlr] (Other::as2) g21 = ([(_,apx2')], gg)`] >>
-      patresolve `known [exp1] as1 g0 = _` hd subspt_known_elist_globals >>
-      simp[] >> disch_then (resolve_selected hd) >> simp[] >> strip_tac >>
-      fs[] >> unabbrevify >>
-      first_x_assum (patresolve `known [exp1] _ g2 = _` last) >> simp[] >>
-      impl_keep_tac >- metis_tac[subspt_trans] >> strip_tac >>
-      fs[PULL_EXISTS, EXISTS_PROD] >>
-      first_x_assum (patresolve `known [hndlr] _ g21 = _` last) >> simp[] >>
-      impl_keep_tac >- metis_tac[subspt_trans] >>
-      metis_tac[merge_subapprox_cong, subspt_trans])
-  >- (say "call" >>
-      rpt (pairarg_tac >> fs[]) >> rveq >> fs[] >> unabbrevify >> metis_tac[])
-  >- (say "op" >>
-      rpt (pairarg_tac >> fs[]) >> rveq >> fs[] >>
-      map_every rename1 [`apx' ◁ apx`,
-                           `known_op opn _ g01 = (apx,g1)`,
-                           `known_op opn _ g21 = (apx',gg)`] >>
-      patresolve `known_op _ _ g01 = _` (el 2) subspt_known_op_elist_globals >>
-      simp[] >> disch_then (resolve_selected hd) >> simp[] >> strip_tac >>
-      fs[] >> unabbrevify >>
-      first_x_assum (patresolve `known _ _ g2 = _` last) >> simp[] >>
-      impl_keep_tac >- metis_tac[subspt_trans] >> strip_tac >>
-      patresolve `known_op _ _ g01 = _` hd known_op_increases_subspt_info >>
-      simp[] >>
-      disch_then (patresolve `known_op _ _ g21 = _` last) >>
-      simp[LIST_REL_REVERSE_EQ] >> metis_tac[subspt_trans])
-  >- (say "app" >>
-      rpt (pairarg_tac >> fs[]) >> rveq >> fs[] >>
-      imp_res_tac known_sing_EQ_E >> rveq >> fs[] >> rveq >>
-      map_every rename1 [`subspt g2 gg`, `subspt g1 g2`,
-                           `known args as2 g2 = (_, g21)`,
-                           `known [f] as1 g11 = (_, g1)`] >>
-      patresolve `known _ _ _ = (_, g11)` hd subspt_known_elist_globals >>
-      simp[] >>
-      disch_then (resolve_selected hd) >> simp[] >> impl_keep_tac
-      >- fs[BAG_DISJOINT, DISJOINT_SYM] >> strip_tac >> fs[] >> unabbrevify >>
-      first_x_assum (patresolve `known _ _ g2 = _` last) >> simp[] >>
-      impl_keep_tac >- metis_tac[subspt_trans] >> strip_tac >>
-      first_x_assum (patresolve `known _ _ g21 = _` last) >> simp[] >>
-      metis_tac[subspt_trans])
-  >- (say "fn" >>
-      rpt (pairarg_tac >> fs[]) >> rveq >> fs[] >> rveq >> unabbrevify >>
-      rename1 `subspt gg2 gg` >>
-      first_x_assum (patresolve `known _ _ gg2 = _` last) >>
-      simp[] >> reverse impl_tac >- metis_tac[subspt_trans] >>
-      simp[LIST_REL_REPLICATE_same, EVERY2_APPEND_suff])
-  >- (say "letrec" >>
-      rpt (pairarg_tac >> fs[]) >> rveq >> fs[letrec_case_eq] >> rveq >>
-      imp_res_tac known_sing_EQ_E >> rveq >> fs[] >> rveq >>
-      map_every rename1 [`apx1' ◁ apx1`,
-                           `known [bod] _ g0 = ([(_,apx1)], g1)`,
-                           `known [bod] _ g2 = ([(_,apx1')], g)`] >>
-      unabbrevify >>
-      first_x_assum (patresolve `subspt g1 _` hd) >> simp[] >>
-      disch_then (first_assum o mp_then (Pos last) mp_tac) >> simp[] >>
-      disch_then irule >> irule EVERY2_APPEND_suff >> simp[] >>
-      simp[LIST_REL_GENLIST]))
-
-val sga_subspt = Q.store_thm(
-  "sga_subspt",
-  `state_globals_approx s g0 ∧ subspt g0 g ⇒ state_globals_approx s g`,
-  simp[state_globals_approx_def, subspt_def] >> rw[] >> fs[get_global_def] >>
-  nailIHx strip_assume_tac >> metis_tac[domain_lookup]);
-
-val state_globals_LN = Q.store_thm(
-  "state_globals_LN",
-  `state_globals_approx s LN ⇔ ∀n v. get_global n s.globals ≠ SOME (SOME v)`,
-  simp[state_globals_approx_def] >> simp[lookup_def]);
-
-(* Optionally applied state relation and result relation*)
-val opt_state_rel_def = Define`
-  opt_state_rel b g s1 s2 ⇔
-  if b then state_rel g s1 s2
-       else s1 = s2`
-
-val opt_res_rel_def = Define`
-  opt_res_rel b g r1 r2 ⇔
-  if b then res_rel g r1 r2
-        else r1 = r2`
-
-(* Some assumptions can be removed if b = F *)
-val compile_correct = Q.store_thm(
-  "compile_correct",
-  `compile b e0 = e ∧ evaluate ([e0], [], s01) = (res1, s1) ∧
-   esgc_free e0 ∧ every_Fn_vs_NONE [e0] ∧
-   opt_state_rel b LN s01 s02 ∧
-   state_globals_approx s01 LN ∧ BAG_ALL_DISTINCT (set_globals e0) ∧
-   ssgc_free s01
-    ⇒
-   ∃res2 s2 g.
-     evaluate([e], [], s02) = (res2, s2) ∧
-     opt_res_rel b g (res1,s1) (res2,s2)`,
-  reverse (Cases_on`b`)>>
-  simp[compile_def,opt_state_rel_def,opt_res_rel_def] >- metis_tac[]>>
-  rpt (pairarg_tac >> simp[]) >>
-  map_every rename1 [`known [e0] [] LN = (alist0, g1)`,
-                       `known [e0] [] g1 = (alist, g)`] >>
-  imp_res_tac known_sing_EQ_E >> rveq >> fs[] >> rw[] >>
-  patresolve `known _ _ LN = _` hd known_increases_subspt_info >> simp[] >>
-  disch_then (patresolve `known _ _ g1 = _` (el 2)) >> simp[] >> strip_tac >>
-  patresolve `known _ _ g1 = _` last (CONJUNCT1 known_correct) >> simp[] >>
-  disch_then (resolve_selected hd) >> simp[] >>
-  `ksrel g s01 s02` by metis_tac[ksrel_subspt, subspt_LN] >>
-  disch_then (resolve_selected (el 2)) >> simp[] >>
-  metis_tac[sga_subspt, subspt_LN])
-
-val known_code_locs = Q.store_thm("known_code_locs",
-  `∀xs vs g.
-   code_locs (MAP FST (FST (known xs vs g))) = code_locs xs`,
-  ho_match_mp_tac known_ind
-  \\ rw[known_def]
-  \\ rpt(pairarg_tac \\ fs[])
-  \\ rw[code_locs_append]
-  \\ fs[code_locs_def]
-  \\ imp_res_tac known_sing_EQ_E \\ fs[]
-  >- (every_case_tac >> simp[code_locs_def] >>
-      rename[`isGlobal opn`, `gO_destApx apx`] >>
-      Cases_on `opn` >> fs[isGlobal_def] >> Cases_on `apx` >>
-      fs[gO_destApx_def, known_op_def, bool_case_eq, NULL_EQ, case_eq_thms] >> rveq >>
-      imp_res_tac known_LENGTH_EQ_E >> fs[LENGTH_NIL_SYM, code_locs_def])
-  \\ fs[code_locs_map]
-  \\ AP_TERM_TAC
-  \\ simp[MAP_MAP_o,MAP_EQ_f,FORALL_PROD]
-  \\ rw[]
-  \\ first_x_assum drule
-  \\ qmatch_goalsub_abbrev_tac`FST p`
-  \\ Cases_on`p` \\ fs[markerTheory.Abbrev_def]
-  \\ pop_assum(assume_tac o SYM)
-  \\ imp_res_tac known_sing_EQ_E \\ fs[]);
-
-val compile_code_locs = Q.store_thm("compile_code_locs",
-  `code_locs [compile b e] = code_locs [e]`,
-  Cases_on`b` \\ rw[compile_def]
-  \\ rpt(pairarg_tac \\ fs[])
-  \\ pop_assum mp_tac
-  \\ specl_args_of_then``known``known_code_locs mp_tac
-  \\ rw[] \\ fs[]
-  \\ pop_assum mp_tac
-  \\ specl_args_of_then``known``known_code_locs mp_tac
-  \\ rw[] \\ fs[]
-  \\ imp_res_tac known_sing_EQ_E \\ fs[]);
-
-(*
-vsgc_free_def
-ssgc_free_def
-esgc_free_def
-set_globals_def
-compile_correct
-state_globals_approx_def
-clos_knownTheory.compile_def
-val_rel_def
-*)
-
-*)
+         (drule dest_closure_SOME_IMP \\ strip_tac \\ rveq
+          \\ fs [v_rel_app_def] \\ rveq \\ fs []
+          \\ fs [dest_closure_def] \\ rveq
+          \\ imp_res_tac LIST_REL_LENGTH
+          THEN1
+           (IF_CASES_TAC \\ fs [] \\ rveq
+            \\ qpat_abbrev_tac `loc_is_ok = check_loc _ lopt2 _ _ _ _`
+            \\ `loc_is_ok` by (fs [Abbr `loc_is_ok`, loptrel_def, check_loc_def]
+                             \\ TRY (Cases_on `lopt2` \\ fs [])
+                             \\ TRY (Cases_on `loc` \\ fs [] \\ rveq)
+                             \\ fs [check_loc_def])
+            \\ simp [Abbr `loc_is_ok`]
+            \\ fs [pair_case_eq]
+            \\ first_x_assum drule
+            \\ fs [exp_rel_def]
+            \\ rename1 `known _ _ _ g0 = (_, g1)`
+            \\ `g0 = g1` by (match_mp_tac known_unchanged_globals
+                             \\ asm_exists_tac \\ simp [])
+            \\ disch_then drule
+            \\ simp [v_rel_upd_inline_factor, state_rel_upd_inline_factor]
+            \\ qmatch_asmsub_abbrev_tac `evaluate (_, fullenv1, state1)`
+            \\ qmatch_goalsub_abbrev_tac `evaluate (_, fullenv2, state2)`
+            \\ `LIST_REL (v_rel c g) fullenv1 fullenv2`
+               by (simp [Abbr `fullenv1`, Abbr `fullenv2`]
+                   \\ rpt (irule EVERY2_APPEND_suff \\ simp [])
+                   \\ irule EVERY2_TAKE
+                   \\ irule EVERY2_APPEND_suff \\ simp [])
+            \\ disch_then drule \\ simp []
+            \\ `num_args = LENGTH ys + 1` by fs [DROP_NIL]
+            \\ `state_rel c g state1 state2`
+               by (fs [Abbr `state1`, Abbr `state2`, state_rel_def, DROP_NIL])
+            \\ disch_then drule \\ simp []
+            \\ simp [set_globals_empty_esgc_free]
+            \\ simp [EVERY_REVERSE, EVERY_TAKE]
+            \\ simp [set_globals_empty_unique_set_globals]
+            \\ impl_tac
+            THEN1
+             (rpt conj_tac
+              THEN1 cheat
+              THEN1 cheat
+              THEN1 (unabbrev_all_tac \\ rveq \\ fs []
+                     \\ simp [TAKE_LENGTH_ID_rwt]
+                     \\ irule EVERY2_APPEND_suff \\ simp [])
+              THEN1 cheat
+              THEN1 fs [result_case_eq])
+            \\ strip_tac
+            \\ fs [result_case_eq] \\ rveq \\ fs []
+            \\ imp_res_tac evaluate_SING \\ fs [] \\ rveq
+            \\ simp [DROP_LENGTH_TOO_LONG])
+          THEN1
+           (rpt (pairarg_tac \\ fs [])
+            \\ fs [bool_case_eq] \\ rveq
+            \\ rename1 `LIST_REL (f_rel _ _ _) funs1 funs2`
+            \\ rename1 `EL i funs1 = (num_args1, exp1)`
+            \\ rename1 `EL i funs2 = (num_args2, exp2)`
+            \\ `num_args1 = num_args2`
+               by (fs [NOT_LESS_EQUAL, LIST_REL_EL_EQN]
+                   \\ first_x_assum (qpat_assum `i < _` o mp_then (Pos hd) mp_tac)
+                   \\ simp [f_rel_def])
+            \\ qpat_abbrev_tac `loc_is_ok = check_loc _ lopt2 _ _ _ _`
+            \\ `loc_is_ok`
+               by (fs [Abbr `loc_is_ok`, loptrel_def]
+                   \\ TRY (Cases_on `lopt2` \\ fs [])
+                   \\ TRY (Cases_on `loc` \\ fs [] \\ rveq)
+                   \\ fs [check_loc_def, DROP_NIL])
+            \\ simp [Abbr `loc_is_ok`]
+            \\ fs [pair_case_eq]
+            \\ first_x_assum drule
+            \\ qmatch_asmsub_abbrev_tac `f_rel _ aenvcase`
+            \\ `f_rel c aenvcase g (EL i funs1) (EL i funs2)` by fs [LIST_REL_EL_EQN]
+            \\ rfs [] \\ fs [f_rel_def, exp_rel_def]
+            \\ rename1 `known _ _ _ g0 = (_, g1)`
+            \\ `MEM (EL i funs1) funs1` by simp [EL_MEM]
+            \\ pop_assum mp_tac \\ simp [] \\ strip_tac
+            \\ `g0 = g1` by (match_mp_tac known_unchanged_globals
+                             \\ asm_exists_tac \\ simp []
+                             \\ fs [elglobals_EQ_EMPTY]
+                             \\ first_x_assum irule
+                             \\ simp [MEM_MAP]
+                             \\ qexists_tac `EL i funs1` \\ simp [])
+            \\ rveq
+            \\ disch_then drule
+            \\ simp [v_rel_upd_inline_factor, state_rel_upd_inline_factor]
+            \\ qmatch_asmsub_abbrev_tac `evaluate (_, fullenv1, state1)`
+            \\ qmatch_goalsub_abbrev_tac `evaluate (_, fullenv2, state2)`
+            \\ `LIST_REL (v_rel c g) fullenv1 fullenv2`
+               by (simp [Abbr `fullenv1`, Abbr `fullenv2`]
+                   \\ rpt (irule EVERY2_APPEND_suff \\ simp [])
+                   THEN1 (irule EVERY2_TAKE
+                          \\ irule EVERY2_APPEND_suff \\ simp [])
+                   \\ fs [LIST_REL_GENLIST] \\ rw []
+                   \\ asm_exists_tac \\ simp [])
+            \\ disch_then drule \\ simp []
+            \\ `state_rel c g state1 state2`
+               by (fs [Abbr `state1`, Abbr `state2`, state_rel_def]
+                   \\ fs [CONV_RULE (LHS_CONV SYM_CONV) REVERSE_EQ_NIL, DROP_NIL])
+            \\ disch_then drule \\ simp []
+            \\ simp [EVERY_REVERSE, EVERY_TAKE, EVERY_GENLIST]
+            \\ `set_globals exp1 = {||}`
+               by (fs [elglobals_EQ_EMPTY]
+                   \\ first_x_assum irule \\ simp [MEM_MAP]
+                   \\ qexists_tac `EL i funs1` \\ simp [])
+            \\ simp [set_globals_empty_esgc_free]
+            \\ simp [set_globals_empty_unique_set_globals]
+            \\ impl_tac
+            THEN1
+             (rpt conj_tac
+              THEN1 (fs [EVERY_MEM, FORALL_PROD] \\ metis_tac [])
+              THEN1 cheat
+              THEN1 cheat
+              THEN1 (simp [Abbr `fullenv1`, Abbr `aenvcase`]
+                     \\ rpt (irule EVERY2_APPEND_suff \\ simp [])
+                     THEN1 simp [LIST_REL_EL_EQN, EL_REPLICATE]
+                     \\ Cases_on `loc` \\ simp []
+                     THEN1 simp [LIST_REL_EL_EQN, EL_REPLICATE]
+                     THEN1 simp [clos_gen_noinline_eq, LIST_REL_EL_EQN])
+              THEN1 cheat
+              THEN1 fs [result_case_eq])
+            \\ strip_tac
+            \\ fs [result_case_eq] \\ rveq \\ fs [] \\ rveq
+            \\ imp_res_tac evaluate_SING \\ rveq \\ fs [] \\ rveq \\ fs []           
+            \\ fs [CONV_RULE (LHS_CONV SYM_CONV) REVERSE_EQ_NIL, DROP_NIL]
+            \\ simp [DROP_LENGTH_TOO_LONG]))))
+
+);
 
 val _ = export_theory();
